adding more files to selftest 3

examples/machine-code/x64_compiler/x64_codegen_inputLib.sig
@@ -1,0 +1,67 @@
+signature x64_codegen_inputLib =
+sig
+
+  include Abbrev
+
+  datatype access_type =
+    ACCESS_WORD
+  | ACCESS_BYTE;
+
+  datatype assign_address_type =
+    ASSIGN_ADDRESS_REG of int
+  | ASSIGN_ADDRESS_OFFSET_ADD of int * Arbnum.num
+  | ASSIGN_ADDRESS_OFFSET_SUB of int * Arbnum.num;
+
+  datatype assign_monop_type =
+    ASSIGN_MONOP_NOT
+  | ASSIGN_MONOP_NEG;
+
+  datatype assign_binop_type =
+    ASSIGN_BINOP_ADD
+  | ASSIGN_BINOP_SUB
+  | ASSIGN_BINOP_MUL
+  | ASSIGN_BINOP_MOD
+  | ASSIGN_BINOP_DIV
+  | ASSIGN_BINOP_AND
+  | ASSIGN_BINOP_XOR
+  | ASSIGN_BINOP_OR;
+
+  datatype assign_x_type =
+    ASSIGN_X_REG of int          (* register number *)
+  | ASSIGN_X_CONST of Arbnum.num (* constant *);
+
+  datatype assign_exp_type =
+    ASSIGN_EXP_REG of int
+  | ASSIGN_EXP_CONST of Arbnum.num  (* constant *)
+  | ASSIGN_EXP_STACK of int         (* stack[offset] *)
+  | ASSIGN_EXP_BINOP of assign_x_type * assign_binop_type * assign_x_type
+  | ASSIGN_EXP_MONOP of assign_monop_type * assign_x_type
+  | ASSIGN_EXP_MEMORY of access_type * assign_address_type
+  | ASSIGN_EXP_SHIFT_LEFT of assign_x_type * int
+  | ASSIGN_EXP_SHIFT_RIGHT of assign_x_type * int
+  | ASSIGN_EXP_SHIFT_ARITHMETIC_RIGHT of assign_x_type * int
+
+  datatype assign_type =
+    ASSIGN_EXP of int * assign_exp_type        (* register := expression *)
+  | ASSIGN_STACK of int * assign_x_type        (* stack[offset] := x *)
+  | ASSIGN_MEMORY of access_type * assign_address_type * assign_x_type
+                                               (* mem[address] := register *)
+  | ASSIGN_OTHER of term * term                (* lhs := rhs *);
+
+  datatype guard_compare_type =
+    GUARD_COMPARE_LESS of bool       (* true: signed, false: unsigned *)
+  | GUARD_COMPARE_LESS_EQUAL of bool (* true: signed, false: unsigned *)
+  | GUARD_COMPARE_EQUAL;
+
+  datatype guard_type =
+    GUARD_NOT of guard_type
+  | GUARD_COMPARE of int * guard_compare_type * assign_x_type  (* reg, cmp, reg/const *)
+  | GUARD_EQUAL_BYTE of assign_address_type * Arbnum.num
+  | GUARD_TEST of int * assign_x_type
+  | GUARD_OTHER of term;
+
+  val term2guard      : Abbrev.term -> guard_type
+  val term2assign     : Abbrev.term -> Abbrev.term -> assign_type
+
+
+end
