examples/machine-code/multiword/multiwordScript.sml
@@ -5,7 +5,8 @@ val _ = set_trace "Unicode" 0;
 
 open pred_setTheory res_quanTheory arithmeticTheory wordsLib wordsTheory bitTheory;
 open pairTheory listTheory rich_listTheory relationTheory pairTheory integerTheory;
-open fcpTheory;
+open fcpTheory lcsymtacs;
+open ASCIInumbersTheory
 
 val _ = numLib.prefer_num();
 
@@ -102,6 +103,15 @@ val n2mw_SNOC = store_thm("n2mw_SNOC",
   \\ ONCE_REWRITE_TAC [n2mw_def] \\ ASM_REWRITE_TAC [SNOC]
   \\ SIMP_TAC bool_ss [dimwords_def,dimword_def,MULT,EXP_ADD,
        AC MULT_COMM MULT_ASSOC,DIV_DIV_DIV_MULT,EVAL ``0<2``,ZERO_LT_EXP,ZERO_LT_dimword]);
+
+val n2mw_mw2n = prove(
+  ``!xs. (n2mw (LENGTH xs) (mw2n xs) = xs)``,
+  Induct THEN1 EVAL_TAC
+  \\ FULL_SIMP_TAC std_ss [LENGTH,mw2n_def,n2mw_def,CONS_11]
+  \\ FULL_SIMP_TAC (srw_ss()) []
+  \\ Cases \\ FULL_SIMP_TAC (srw_ss()) []
+  \\ ONCE_REWRITE_TAC [ADD_COMM] \\ ONCE_REWRITE_TAC [MULT_COMM]
+  \\ FULL_SIMP_TAC std_ss [MOD_MULT,DIV_MULT]);
 
 val LENGTH_n2mw = store_thm("LENGTH_n2mw",
   ``!k n. LENGTH (n2mw k n) = k``,Induct \\ ASM_REWRITE_TAC [n2mw_def,LENGTH]);
@@ -386,6 +396,10 @@ val mw_trailing_NIL = store_thm("mw_trailing_NIL",
   \\ `0 < dimwords (LENGTH xs) (:'a)` by METIS_TAC [ZERO_LT_dimwords] \\ DISJ2_TAC
   \\ REPEAT STRIP_TAC THEN1 DECIDE_TAC \\ Cases_on `x`
   \\ FULL_SIMP_TAC std_ss [n2w_11,w2n_n2w,ZERO_LT_dimword]);
+
+val mw_trailing_LENGTH_ZERO = prove(
+  ``!xs. (LENGTH (mw_trailing xs) = 0) = (mw2n xs = 0)``,
+  FULL_SIMP_TAC std_ss [LENGTH_NIL,mw_trailing_NIL]);
 
 
 (* add/sub *)
@@ -727,6 +741,11 @@ val mwi_mul_def = Define `
       let (xs,ys) = (if LENGTH xs < LENGTH ys then (xs,ys) else (ys,xs)) in
         (~(s = t), mw_trailing (mw_mul xs ys (MAP (\x.0w) ys)))`;
 
+val mwi_mul_simple_def = Define `
+  mwi_mul_simple (s,xs) (t,ys) =
+    if (xs = []) \/ (ys = []) then (F,[]) else
+      (~(s = t), mw_trailing (mw_mul xs ys (MAP (\x.0w) ys)))`;
+
 val single_mul_thm = prove(
   ``!(x:'a word) y k z l.
       (single_mul x y k = (z,l)) ==>
@@ -807,6 +826,25 @@ val NUM_EXISTS = prove(
 val mwi_mul_thm = store_thm("mwi_mul_thm",
   ``!i j. mwi_mul (i2mw i) (i2mw j) = i2mw (i * j)``,
   REPEAT STRIP_TAC \\ SIMP_TAC std_ss [i2mw_def,mwi_mul_def,mw_NIL,Num_ABS_EQ_0]
+  \\ ONCE_REWRITE_TAC [EQ_SYM_EQ]
+  \\ Cases_on `i = 0`
+  THEN1 ASM_SIMP_TAC std_ss [mw_NIL,Num_ABS_EQ_0,INT_MUL_REDUCE,INT_LT_REFL]
+  \\ Cases_on `j = 0`
+  THEN1 ASM_SIMP_TAC std_ss [mw_NIL,Num_ABS_EQ_0,INT_MUL_REDUCE,INT_LT_REFL]
+  \\ `i * j < 0 = ~(i < 0 = j < 0)` by
+        (SIMP_TAC std_ss [INT_MUL_SIGN_CASES] \\ intLib.COOPER_TAC)
+  \\ ASM_SIMP_TAC std_ss [] \\ SRW_TAC [] [] \\ ONCE_REWRITE_TAC [EQ_SYM_EQ]
+  \\ MATCH_MP_TAC IMP_EQ_mw \\ ASM_SIMP_TAC std_ss [mw_ok_mw_trailing]
+  \\ ASM_SIMP_TAC std_ss [mw2n_mw_trailing,LENGTH_MAP,mw_mul_thm,mw2n_mw,
+       RW [APPEND,mw2n_def] (Q.SPEC `[]` mw2n_MAP_ZERO),GSYM INT_ABS_MUL]
+  \\ STRIP_ASSUME_TAC (Q.SPEC `i` NUM_EXISTS)
+  \\ STRIP_ASSUME_TAC (Q.SPEC `j` NUM_EXISTS)
+  \\ ASM_SIMP_TAC std_ss [INT_MUL,NUM_OF_INT,AC MULT_COMM MULT_ASSOC]);
+
+val mwi_mul_simple_thm = store_thm("mwi_mul_simple_thm",
+  ``!i j. mwi_mul_simple (i2mw i) (i2mw j) = i2mw (i * j)``,
+  REPEAT STRIP_TAC
+  \\ SIMP_TAC std_ss [i2mw_def,mwi_mul_simple_def,mw_NIL,Num_ABS_EQ_0]
   \\ ONCE_REWRITE_TAC [EQ_SYM_EQ]
   \\ Cases_on `i = 0`
   THEN1 ASM_SIMP_TAC std_ss [mw_NIL,Num_ABS_EQ_0,INT_MUL_REDUCE,INT_LT_REFL]
@@ -974,5 +1012,1850 @@ val mw_subv_NOT_NIL = store_thm("mw_subv_NOT_NIL",
   \\ POP_ASSUM MP_TAC \\ ASM_SIMP_TAC std_ss [mw2n_def] \\ DECIDE_TAC);
 
 
-val _ = export_theory();
+(* Division *)
 
+(* Following will be a definition of a division algorithm miming that
+   described by Donald E. Knuth in "The Art of Computer
+   Programming". (Found in "Volume II: Seminumerical Algorithms", on
+   pages 270-273 in the most recent edition (3rd edition, 1997)).
+
+   It is meant to compute the quotient of a word list x_{1}...x_{m+n}
+   by a word list y_{1}...y{n} where n and m are natural numbers, and
+   the words have arbitrary dimension b = 2 ^ k, for some given
+   natural k.
+
+   For this section, the digits of the word-list inputs are ordered in
+   reverse - that is, with the most significant bit as head *)
+
+(* General Definitions *)
+
+val mw_mul_by_single_def = Define `
+  mw_mul_by_single (x:'a word) (ys:'a word list) =
+    mw_mul_pass x ys (n2mw (LENGTH ys) 0) 0w`;
+
+val PULL_CONJ = METIS_PROVE [] ``!a b c.( a ==> b /\ c) ==>(a ==> b) /\ (a ==> c)``
+
+(*   Two theorems and corresponding tactics for handling equations
+     in a more "high-level" way, compared with the ones I know.          *)
+
+val EQ_M_R_S_i =
+  GEN_ALL (CONJUNCT2
+   (MP (Q.SPECL [`m*n < p*n`,`0<n`,`m<p`] PULL_CONJ)
+        ((fn (x,y) => x) (EQ_IMP_RULE (SPEC_ALL LT_MULT_RCANCEL)))))
+
+val EQT_M_R_S_i = fn x => (MATCH_MP_TAC (Q.SPECL [`xxx`,x,`yyy`] EQ_M_R_S_i))
+
+val EQ_A_S_R_2 = store_thm ("EQ_A_S_R_2",
+  ``!c d a b. d <= c /\ a + c < b + d ==> a < b``,
+  REPEAT strip_tac  >> RW_TAC arith_ss[]);
+
+val EQT_A_S_R_2 =
+  (* If the goal is `a < b` and `c <= d` is an assumption, transforms current goal into `a + c < b + d` *)
+  fn (c,d) =>
+    (MATCH_MP_TAC
+    (Q.SPECL [c,d,`xxx`,`yyy`] EQ_A_S_R_2)
+    >> strip_tac THEN1 METIS_TAC[]);
+
+(* division arithmetic lemmas*)
+
+val DIV_thm2 = store_thm( "DIV_thm2",
+  ``0 < b /\ a < c * b ==> a DIV b < c``,
+  strip_tac >> METIS_TAC[DIV_LT_X]);
+
+val DIV_thm3 = store_thm( "DIV_thm3",
+  ``!a b. 0 < b ==> (a DIV b * b <= a)``,
+  REPEAT strip_tac >> IMP_RES_TAC DIVISION >> METIS_TAC[LESS_EQ_ADD]);
+
+val DIV_thm4 = store_thm( "DIV_thm4",
+  ``!a b. 0 < b ==> (a - a DIV b * b < b)``,
+  REPEAT strip_tac >> IMP_RES_TAC DIVISION >>
+  METIS_TAC[MOD_LESS_EQ,DIV_thm3,CANCEL_SUB,ADD_SUB,ADD_COMM]);
+
+val DIV_thm4_bis = store_thm( "DIV_thm4_bis",
+  ``!a b. 0 < b ==> a < b + a DIV b * b``, strip_tac >>
+  METIS_TAC[DIV_EQ_X,MULT,ADD_COMM]);
+
+val DIV_thm1 = store_thm( "DIV_thm1",
+  ``0 < b /\ b <= c ==> a DIV c <= a DIV b`` ,
+  strip_tac >> qsuff_tac `a < (a DIV b + 1) * c` THEN1 (
+  strip_tac >> METIS_TAC[LESS_LESS_EQ_TRANS,DIV_LE_X]) >>
+  MATCH_MP_TAC LESS_LESS_EQ_TRANS >> EXISTS_TAC ``(a DIV b + 1)*b`` >> strip_tac THEN1
+  METIS_TAC[DIV_thm4_bis,RIGHT_ADD_DISTRIB,MULT_LEFT_1,ADD_COMM] >>
+  METIS_TAC[MULT_COMM,LESS_MONO_MULT]);
+
+val DIV_thm5 = store_thm( "DIV_thm5",
+  ``0 < b /\ a - q*b < b ==> (q >= a DIV b)``,
+  rw[GREATER_EQ] >> rw[DIV_LE_X] >> srw_tac[ARITH_ss][]);
+
+(* lists *)
+
+val NOT_NIL_EQ_LENGTH_NOT_0 = store_thm ( "NOT_NIL_EQ_LENGTH_NOT_0",
+  ``x <> [] <=> (0 < LENGTH x)``,
+  Cases_on `x` >> lrw[]);
+
+val HD_REVERSE = store_thm ("HD_REVERSE",
+  ``!x. x <> [] ==> (HD (REVERSE x) = LAST x)``,
+  REPEAT strip_tac >>
+  Induct_on `x` THEN1 fs[] >>
+  rw[LAST_DEF] >>
+  Cases_on `REVERSE x` THEN1 fs[] >>
+  fs[]);
+
+(* word & multiWord general *)
+
+val NOT_0w_bis = store_thm("NOT_0w_bis",
+  ``w <> 0w ==> 0 < w2n w``,
+  Cases_on `w`>> fs [] >> DECIDE_TAC);
+
+val dimwords_dimword = store_thm("dimwords_dimword",
+  ``!n. dimwords n (:'a) = dimword(:'a) ** n``,
+  rw[dimwords_def,dimword_def,Once MULT_COMM] >>
+  Induct_on `n` THEN1 rw[] >>
+  METIS_TAC[MULT_COMM,MULT,EXP,EXP_ADD]);
+
+val mw2n_msf = store_thm ("mw2n_msf" ,
+  ``!(x:'a word) xs. mw2n (xs++[x]) = mw2n xs + dimwords (LENGTH xs) (:'a) * w2n x``,
+  Induct_on `xs` >>
+  lrw[mw2n_def, EXP,dimwords_def,dimword_def,LEFT_ADD_DISTRIB] >>
+  REWRITE_TAC[MULT,DECIDE ``z * dimindex (:'a) = dimindex (:'a) * z``] >>
+  METIS_TAC[MULT_ASSOC,EXP_ADD,ADD_COMM]);
+
+val mw2n_msf_NIL = store_thm ("mw2n_msf_NIL",
+  ``!(xs:'a word list). (xs <> []) /\
+                        (mw2n xs < dimwords (LENGTH (FRONT xs)) (:'a)) ==>
+                        (mw2n xs = mw2n (FRONT xs))``,
+  REPEAT strip_tac >>
+  `mw2n xs = mw2n (FRONT xs ++ [LAST xs])` by METIS_TAC[APPEND_FRONT_LAST] >>
+  POP_ASSUM (fn x => FULL_SIMP_TAC std_ss [x,mw2n_msf]) >>
+  METIS_TAC[LESS_EQ_ADD,ADD_COMM,LESS_EQ_LESS_TRANS,LT_MULT_CANCEL_RBARE]);
+
+val mw2n_n2mw_0 = store_thm( "mw2n_n2mw_0",
+  ``!x. mw2n ((n2mw x 0):'a word list) = 0``,
+  Induct_on `x` THEN1 METIS_TAC[n2mw_def,mw2n_def] >>
+  `0 DIV dimword(:'a) = 0` by METIS_TAC[ZERO_LT_dimword,ZERO_DIV] >>
+  RW_TAC std_ss [word_0_n2w,n2mw_def,mw2n_def]);
+
+val mw_mul_by_single_lemma = store_thm( "mw_mul_by_single_lemma",
+  ``!(x:'a word) (ys:'a word list).
+    (mw2n (mw_mul_by_single x ys) = w2n x * mw2n ys) /\
+    (LENGTH (mw_mul_by_single x ys) = LENGTH ys + 1)``,
+  REPEAT strip_tac >>
+  REWRITE_TAC[mw_mul_by_single_def] >>
+  `LENGTH (ys:'a word list) = LENGTH ((n2mw (LENGTH ys) 0): 'a word list)`
+  by METIS_TAC[LENGTH_n2mw] >>
+  IMP_RES_TAC (SPEC_ALL mw_mul_pass_thm) >> lrw[mw2n_n2mw_0]);
+
+val word_reverse_lsl = prove(
+  ``!w n. word_reverse (w << n) = (word_reverse w >>> n):'a word``,
+  FULL_SIMP_TAC std_ss [word_reverse_def,word_lsl_def,word_lsr_def,
+    fcpTheory.CART_EQ,fcpTheory.FCP_BETA] THEN REPEAT STRIP_TAC
+  THEN `(dimindex (:'a) - 1 - i) < dimindex (:'a)` by DECIDE_TAC
+  THEN Cases_on `i + n < dimindex (:'a)`
+  THEN FULL_SIMP_TAC std_ss [fcpTheory.FCP_BETA]
+  THEN `i + n < dimindex (:'a) = n <= dimindex (:'a) - 1 - i` by DECIDE_TAC
+  THEN FULL_SIMP_TAC std_ss [fcpTheory.FCP_BETA,SUB_PLUS]);
+
+val word_reverse_EQ_ZERO = prove(
+  ``!w:'a word. (word_reverse w = 0w) = (w = 0w)``,
+  FULL_SIMP_TAC std_ss
+   [fcpTheory.CART_EQ,fcpTheory.FCP_BETA,word_reverse_def,word_0]
+  THEN REPEAT STRIP_TAC THEN EQ_TAC THEN REPEAT STRIP_TAC
+  THEN `dimindex (:'a) - 1 - i < dimindex (:'a)` by DECIDE_TAC THEN RES_TAC
+  THEN `dimindex (:'a) - 1 - (dimindex (:'a) - 1 - i) = i` by DECIDE_TAC
+  THEN FULL_SIMP_TAC std_ss []);
+
+val calc_d_def = tDefine "calc_d" `
+
+(* Following is an algorithm that computes the normalisation factor
+   (named d in Knuth's discussion) by which both xs and ys are multiplied
+   to ensure that the most significant figure of ys in greater or equal to
+   b / 2
+
+   Since we are working with word-size b = 2 ^ k for some natural k,
+   we produce the factor by multiplying the mentioned figure by 2
+   successively until b / 2 is reached.  *)
+
+  calc_d (v1:'a word, d:'a word) =
+    if (v1 = 0w) \/ word_msb(v1) then d else
+      calc_d (v1 * 2w, d * 2w)`
+  (WF_REL_TAC `measure (\(v1,d). w2n (word_reverse v1))`
+   THEN SIMP_TAC std_ss [WORD_MUL_LSL |> Q.SPECL [`w`,`1`] |>
+          SIMP_RULE std_ss [Once WORD_MULT_COMM] |> GSYM]
+   THEN FULL_SIMP_TAC std_ss [word_reverse_lsl,w2n_lsr]
+   THEN REPEAT STRIP_TAC
+   THEN `~(word_reverse v1 = 0w)` by FULL_SIMP_TAC std_ss [word_reverse_EQ_ZERO]
+   THEN Cases_on `word_reverse v1`
+   THEN FULL_SIMP_TAC (srw_ss()) [DIV_LT_X] THEN DECIDE_TAC);
+
+val calc_d_ind = fetch "-" "calc_d_ind"
+
+(* Definition *)
+
+val single_div_def = Define `
+  (single_div (x1:'a word) (x2:'a word) (y:'a word) =
+  (n2w ((w2n x1 * dimword (:'a) + w2n x2) DIV w2n y): 'a word,
+   n2w ((w2n x1 * dimword (:'a) + w2n x2) MOD w2n y): 'a word))`;
+
+val mw_div_by_single_def = tDefine "mw_div_by_single" `
+
+(* This algorithm forms the quotient of a multi-word number
+   x_{1}x_{2}x_{3}...x_{n} by a single word y using the classic
+   Euclidean division algorithm *)
+
+  (mw_div_by_single [] (y:'a word) = [0w]:'a word list) /\
+  (mw_div_by_single ([x]:'a word list) (y:'a word) = (\(a,b).if w2n x < w2n y then [b] else a::[b]) (single_div 0w x y)) /\
+  (mw_div_by_single (x1::x2::xs:'a word list) (y:'a word) =
+    if (w2n x1 < w2n y) \/ (w2n y = 0)
+      then let (q,r) = single_div x1 x2 y in
+      q::(mw_div_by_single (r::xs) y)
+      else let (q,r) = single_div 0w x1 y in
+      q::(mw_div_by_single (r::x2::xs) y))`
+
+  (WF_REL_TAC`measure(\(xs,y). if w2n (HD xs) < w2n y
+                             then 2 * LENGTH xs
+                             else 2 * LENGTH xs + 1)` >>
+   lrw[single_div_def] >>
+   Cases_on `y = 0w` THEN1 METIS_TAC[] >>
+   `0 < w2n y` by METIS_TAC[w2n_eq_0,NOT_ZERO_LT_ZERO] >>
+   METIS_TAC[MOD_LESS,MOD_LESS_EQ,ZERO_LT_dimword,LESS_EQ_LESS_TRANS])
+
+val mw_div_by_single_ind = fetch "-" "mw_div_by_single_ind"
+
+val mw_simple_div_def = Define `
+  (mw_simple_div x [] y = ([],x,T)) /\
+  (mw_simple_div x (x1::xs) y =
+     let c1 = x <+ y in
+     let (q,r) = single_div x x1 y in
+     let (qs,r,c) = mw_simple_div r xs y in
+       (q::qs,r,c /\ c1))`;
+
+val mw_div_test_def = tDefine "mw_div_test" `
+
+(* This function encloses the 3rd step "D3" of Knuth's algorithm.  It
+   is meant to take input q = u_{1}u_{2} / v_{1}, and either outputs Q
+   or Q + 1, where Q = U / V, U = u_{1}u_{2}u_{3}...u_{n+1},
+   V = v_{1}v_{2}...v_{n} are word lists with word-size b for some
+   n > 1, and Q < b.
+
+   Both if statements rephrase Knuth's tests, replacing the value of
+   the remainder r of the division u1u2 / v1 by r = u1u2 - u1u2 / v1,
+   and adding values on both sides of each equation to avoid
+   substractions.  *)
+
+  mw_div_test (q:'a word) (u1:'a word) (u2:'a word) (u3:'a word) (v1:'a word) (v2:'a word)  =
+    if (mw_cmp [u3;u2;u1] (mw_mul_by_single q [v2;v1])) = SOME T
+    then let q2 = n2w (w2n q - 1) in
+         let s = single_mul q2 v1 0w in
+          if (mw_cmp [u2;u1] (FST (mw_add [FST s; SND s] [0w;1w] F))) = SOME T
+          then mw_div_test q2 u1 u2 u3 v1 v2
+          else q2
+    else q`
+
+  (WF_REL_TAC `measure (\(q,u1,u2,u3,v1,v2). w2n q)` >>
+  REPEAT strip_tac >>
+  Cases_on `w2n q` THEN1 (
+  qsuff_tac `mw_cmp [u3; u2; u1] (mw_mul_by_single 0w [v2; v1]) <> SOME T` THEN1 fs[] >>
+  Q.PAT_ABBREV_TAC `x = mw_mul_by_single 0w [v2;v1]` >>
+  Q.PAT_ABBREV_TAC `u = [u3;u2;u1]` >>
+  `LENGTH x = LENGTH u` by fs[mw_mul_by_single_lemma,Abbr`x`,Abbr`u`] >>
+  `~(mw2n u < mw2n x)` by rw[mw_mul_by_single_lemma,Abbr`x`] >>
+  fs[mw_cmp_thm]) >>
+  rw[SUC_SUB1] >>
+  `n < dimword(:'a)` by METIS_TAC[w2n_lt,DECIDE ``n < SUC n``,LESS_TRANS] >>
+  rw[]);
+
+val mw_div_test_ind = fetch "-" "mw_div_test_ind"
+
+val mw_div_loop_def = tDefine "mw_div_loop"
+
+(* This algorithm encloses the steps between the 3rd "D3" and the
+   seventh "D7" which are repeated m + 1 times, where the initial
+   inputs are dividend xs = x_{1}...x_{m+n} and divisor ys =
+   y_{1}...y_{n}, and the normalised dividend is x_{1}...x_{m+n+1}. *)
+
+(*     Inputs are:
+
+       zs = x_{1}...{j+n+1}
+       us = x_{j}...x_{j+n+1}   ( j = m, m-1,..., 0 )
+       q = x1x2 / y1
+
+       q is then modified through mw_div_test.
+
+       if us < q * ys,   quotient digit is q - 1
+                         and input X becomes X - (q-1) * ys
+       else              quotient digit is q
+                         and input X's becomes X's - q * ys     *)
+
+ `mw_div_loop (zs:'a word list) (ys:'a word list) =
+
+  if LENGTH ys < LENGTH zs
+  then let (us:'a word list) = TAKE (SUC(LENGTH ys)) zs in
+       let q = if w2n (HD us) < w2n (HD ys)
+               then FST (single_div (HD us) (HD (TL us)) (HD ys))
+               else (n2w (dimword(:'a) - 1):'a word) in
+       let q2 = mw_div_test q (HD us) (HD (TL us)) (HD (TL (TL us))) (HD ys) (HD (TL ys)) in
+       let q2ys = mw_mul_by_single q2 (REVERSE ys) in
+
+       if mw_cmp (REVERSE us) q2ys = SOME T
+       then let q3 = (n2w (w2n q2 - 1):'a word) in
+            let q3ys = mw_mul_by_single q3 (REVERSE ys) in
+            let zs2 = (REVERSE (FRONT (FST(mw_sub (REVERSE us) q3ys T)))) ++ DROP (SUC(LENGTH ys)) zs in
+            q3::(mw_div_loop zs2 ys)
+       else let zs2 = (REVERSE (FRONT (FST(mw_sub (REVERSE us) q2ys T)))) ++ DROP (SUC(LENGTH ys)) zs in
+            q2::(mw_div_loop zs2 ys)
+  else zs`
+
+(WF_REL_TAC `measure (LENGTH o FST)` >>
+ REPEAT strip_tac >>
+ Q.PAT_ABBREV_TAC `us = (TAKE (SUC (LENGTH ys)) zs)` >>
+ Q.PAT_ABBREV_TAC `q = (if w2n (HD us) < w2n (HD ys) then
+                          FST (single_div (HD us) (HD (TL us)) (HD ys))
+                        else
+                          n2w (dimword (:'a) - 1))` >>
+ Q.PAT_ABBREV_TAC `q2 =(mw_div_test q (HD us) (HD (TL us))
+                       (HD (TL (TL us))) (HD ys) (HD (TL ys)))` >>
+  `LENGTH us = SUC (LENGTH ys)` by METIS_TAC[LENGTH_TAKE,LESS_EQ] THENL [
+
+ Q.PAT_ABBREV_TAC `q3:'a word = n2w (w2n q2 - 1)` >>
+ Q.PAT_ABBREV_TAC `q3ys = (mw_mul_by_single q3 (REVERSE ys))` >>
+ `LENGTH (REVERSE us) = LENGTH q3ys` by METIS_TAC[LENGTH_REVERSE,Abbr`q3ys`,mw_mul_by_single_lemma,ADD1] >>
+ Q.PAT_ABBREV_TAC `ws = FST (mw_sub (REVERSE us) q3ys T)` ,
+
+ Q.PAT_ABBREV_TAC `q2ys = (mw_mul_by_single q2 (REVERSE ys))` >>
+ `LENGTH (REVERSE us) = LENGTH q2ys` by METIS_TAC[LENGTH_REVERSE,Abbr`q2ys`,mw_mul_by_single_lemma,ADD1] >>
+ Q.PAT_ABBREV_TAC `ws = FST (mw_sub (REVERSE us) q2ys T)` ] >>
+
+ `LENGTH ws = LENGTH (REVERSE us)` by METIS_TAC[PAIR,mw_sub_lemma,Abbr`ws`] >>
+ lrw[] >>
+ qsuff_tac `ws <> []` THEN1 METIS_TAC[rich_listTheory.LENGTH_BUTLAST,LENGTH_REVERSE,prim_recTheory.PRE,DECIDE ``n < SUC n``] THEN1
+ METIS_TAC[NULL,rich_listTheory.LENGTH_NOT_NULL,DECIDE ``0 < SUC n``,LENGTH_REVERSE] THEN1
+ METIS_TAC[rich_listTheory.LENGTH_BUTLAST,LENGTH_REVERSE,prim_recTheory.PRE,DECIDE ``n < SUC n``] >>
+ METIS_TAC[NULL,rich_listTheory.LENGTH_NOT_NULL,DECIDE ``0 < SUC n``,LENGTH_REVERSE])
+
+val mw_div_loop_ind = fetch "-" "mw_div_loop_ind"
+
+val mw_div_def = Define
+
+(* Division of xs = x_{1}...x_{m+n} by ys = y_{1}...y_{n} *)
+
+` mw_div (xs:'a word list) (ys:'a word list) =
+
+  let txs = mw_trailing xs in
+  let tys = mw_trailing ys in
+
+  if LENGTH txs < LENGTH tys
+  then ([]:'a word list,txs)
+
+  else if LENGTH tys = 1
+       then let rslt = mw_div_by_single (REVERSE txs) (LAST tys) in
+            (REVERSE (FRONT rslt), [LAST rslt])
+       else let d = calc_d ((LAST tys,1w)) in
+            let dxs = mw_mul_by_single d txs in
+            let dys = FRONT (mw_mul_by_single d tys) in
+
+(*  ensure: x_{m}...x_{m+n} DIV y_{1}...y_{n} < b  *)
+
+            if (mw_cmp (LASTN (LENGTH dys) dxs) dys = SOME T) /\ (LENGTH dys < LENGTH dxs)
+            then let rslt = mw_div_loop (REVERSE dxs) (REVERSE dys) in
+            (DROP (LENGTH dys) (REVERSE rslt), REVERSE (FRONT (mw_div_by_single (LASTN (LENGTH dys) rslt) d)))
+            else let rslt = mw_div_loop (REVERSE (SNOC 0w dxs)) (REVERSE dys) in
+            (DROP (LENGTH dys) (REVERSE rslt), REVERSE (FRONT (mw_div_by_single (LASTN (LENGTH dys) rslt) d))) `
+
+(* calc_d Lemmas  *)
+
+val d_word_msb = store_thm( "d_word_msb",
+``!(a:'a word). word_msb a <=> dimword(:'a) DIV 2 <= w2n a``,
+  Cases THEN `0 < dimindex (:'a)` by FULL_SIMP_TAC std_ss [DIMINDEX_GT_0]
+  THEN `(dimindex(:'a)) - 1 < (dimindex (:'a))` by DECIDE_TAC
+  THEN `2 ** SUC (dimindex(:'a) - 1) = dimword (:'a)` by
+         (FULL_SIMP_TAC std_ss [dimword_def] THEN DECIDE_TAC)
+  THEN FULL_SIMP_TAC std_ss [w2n_n2w,word_msb_def,word_index,bitTheory.BIT_def,
+         bitTheory.BITS_THM2,DIV_LE_X,DIV_EQ_X,GSYM EXP]
+  THEN FULL_SIMP_TAC std_ss [dimword_def] THEN Cases_on `dimindex (:'a)`
+  THEN FULL_SIMP_TAC std_ss [EXP] THEN DECIDE_TAC);
+
+val d_lemma1 = store_thm ("d_lemma1",
+``!(v1:'a word) (d:'a word) (x:'a word).
+   calc_d (FST(v1,d),SND(v1,d)*x) = calc_d(v1,d) * x``,
+  HO_MATCH_MP_TAC calc_d_ind >> REPEAT strip_tac >>
+  rw[Once calc_d_def] THEN1 rw[Once calc_d_def] THEN1 rw[Once calc_d_def] >>
+  fs[FST,SND] >>
+  `!(x1:'a word) (x2:'a word). x1 * x2 = x2 * x1` by rw[] >>
+  METIS_TAC[calc_d_def]);
+
+val d_lemma2 = store_thm ("d_lemma2",
+``!(v1:'a word) (d:'a word).
+  FST(v1,d) <> 0w ==>
+  dimword(:'a) DIV 2 <= w2n ((calc_d (FST(v1,d),1w:'a word)) * (FST (v1,d)))``,
+
+  HO_MATCH_MP_TAC calc_d_ind >> REPEAT strip_tac >>
+  rw[Once calc_d_def] THEN1 METIS_TAC[FST] THEN1 METIS_TAC[d_word_msb] >>
+  fs[FST] >>
+  `w2n d < dimword(:'a) DIV 2` by METIS_TAC[d_word_msb,NOT_LESS_EQUAL] >>
+  `0 < 2` by DECIDE_TAC >>
+  `(2 * w2n d) < dimword(:'a)` by METIS_TAC[MULT_COMM,DIV_thm3,LESS_LESS_EQ_TRANS,LT_MULT_RCANCEL] >>
+  Cases_on `dimword(:'a) = 2` THEN1 (`w2n d = 0` by DECIDE_TAC >> METIS_TAC[w2n_eq_0]) >>
+  ASSUME_TAC ONE_LT_dimword >> `2 < dimword(:'a)` by DECIDE_TAC >>
+  `2w * d <> 0w` by rw[word_mul_def] >>
+  `2w = 1w * 2w` by rw[] >>
+  `calc_d(2w *d, 2w) = calc_d(2w*d,1w) * 2w` by METIS_TAC[d_lemma1,FST,SND] >> POP_ASSUM (fn x => REWRITE_TAC[x]) >>
+  RES_TAC >>rw[]);
+
+val d_lemma2_bis = store_thm ( "d_lemma2_bis",
+``!(v1:'a word) (d:'a word).
+  FST(v1,d) <> 0w ==> calc_d (FST(v1,d),1w) <> 0w``,
+  REPEAT strip_tac >> IMP_RES_TAC d_lemma2 >>
+  `w2n (calc_d (FST (v1,d),1w)) = 0` by METIS_TAC[word_0_n2w] >>
+  fs[FST,word_mul_def] >>
+  METIS_TAC[TWO,LESS_EQ,ONE_LT_dimword,DECIDE``0<2``,prim_recTheory.LESS_NOT_EQ,DIV_GT0]);
+
+val d_lemma3 = store_thm ("d_lemma3",
+``!(v1:'a word) (d:'a word).
+  w2n (calc_d (FST(v1,d),1w:'a word)) * w2n (FST (v1,d)) < dimword(:'a)``,
+
+  HO_MATCH_MP_TAC calc_d_ind >> REPEAT strip_tac >>
+  rw[Once calc_d_def,w2n_lt] >>
+  ASSUME_TAC d_lemma1 >>
+  RES_TAC >> fs[FST,SND] >>
+  `2w = 1w*2w` by rw[] >>
+  `calc_d (2w * d,2w) = 2w * (calc_d (2w * d,1w))` by METIS_TAC[] >> POP_ASSUM (fn x => REWRITE_TAC[x]) >>
+  Q.PAT_ABBREV_TAC` X = calc_d (2w * d,1w)` >>
+  fs[word_mul_def] >>
+  Cases_on `dimword(:'a) = 2` THEN1 fs[] >>
+  ASSUME_TAC ONE_LT_dimword >>
+  `2 < dimword(:'a)` by DECIDE_TAC >>
+  `2 MOD dimword(:'a) = 2` by METIS_TAC[LESS_MOD] >>
+  POP_ASSUM (fn x => fs[x]) >>
+  `w2n d < dimword(:'a) DIV 2` by METIS_TAC[d_word_msb,NOT_LESS_EQUAL] >>
+  `0 < 2` by DECIDE_TAC >>
+  `(2 * w2n d) < dimword(:'a)` by METIS_TAC[MULT_COMM,DIV_thm3,LESS_LESS_EQ_TRANS,LT_MULT_RCANCEL] >>
+  `(2 * w2n d) MOD dimword(:'a) = (2 * w2n d)` by rw[LESS_MOD] >> POP_ASSUM (fn x => fs[x]) >>
+  `(2 * w2n X) * w2n d < dimword(:'a)` by RW_TAC arith_ss[] >>
+  METIS_TAC[MOD_LESS_EQ,ZERO_LT_dimword,LESS_EQ_LESS_TRANS,LESS_MONO_MULT]);
+
+val d_lemma4 = store_thm ("d_lemma4",
+``!(v1:'a word) (d:'a word).
+  ?n. w2n (calc_d (FST(v1,d),1w)) = 2 ** n``,
+
+  HO_MATCH_MP_TAC calc_d_ind >> REPEAT strip_tac >> rw[Once calc_d_def] >> RES_TAC >>
+  fs[FST] >>
+  `2w = 1w * 2w` by rw[] >>
+  `calc_d (2w * d,2w) = calc_d (2w * d,1w) * 2w` by METIS_TAC[d_lemma1,FST,SND] >>
+  POP_ASSUM (fn x => REWRITE_TAC[x]) >> rw[word_mul_def] >>
+  REWRITE_TAC[dimword_def] >> ASSUME_TAC dimword_def >>  Q.PAT_ABBREV_TAC `m = dimindex(:'a)` >> markerLib.RM_ABBREV_TAC "m" >>
+  Cases_on `m = 1` THEN1 (
+  `w2n d < 1` by METIS_TAC[d_word_msb,NOT_LESS_EQUAL,EVAL ``2 ** 1 DIV 2``] >>
+  `w2n d = 0` by DECIDE_TAC >>
+  METIS_TAC[w2n_eq_0]) >>
+  Cases_on `m` THEN1 METIS_TAC[EXP,ONE_LT_dimword,prim_recTheory.LESS_NOT_EQ] >>
+  `2 < dimword(:'a)` by rw[] THEN1(
+  Cases_on `n'` THEN1 DECIDE_TAC >>
+  rw[EXP] >> METIS_TAC[LE_MULT_CANCEL_LBARE,ZERO_LT_EXP,DECIDE ``0 < 2 /\ 1 < 2``, LESS_LESS_EQ_TRANS] ) >>
+  qpat_assum `dimword(:'a) = xxx` (fn x => REWRITE_TAC [GSYM x] THEN (ASSUME_TAC x)) >>
+  rw[LESS_MOD,DECIDE ``2 ** n * 2 = 2 * 2 ** n``,GSYM EXP] >>
+  `SUC n < SUC n'` by ASSUME_TAC (Q.SPECL [`(2w:'a word)*(d:'a word)`,`x`] d_lemma3) THEN1(
+  qpat_assum `2 < xxx` (fn x => fs[FST] THEN ASSUME_TAC x) >>
+  qsuff_tac `w2n (calc_d (2w * d, 1w)) < dimword(:'a) DIV 2` THEN1 (strip_tac >>
+  `dimword(:'a) DIV 2 = 2 ** SUC n' DIV 2 ** 1` by rw[] >>
+  `dimword(:'a) DIV 2 = 2 ** n'` by METIS_TAC[SUC_SUB1,EXP_SUB,DECIDE ``(0 < 2) /\ (1 <= SUC n')`` ] >>
+  ` 2 ** n < 2 ** n'` by METIS_TAC[] >> fs[]) >>
+  `w2n (2w * d) = 2 * w2n d` by rw[word_mul_def] THEN1 (
+  `w2n d < dimword(:'a) DIV 2` by METIS_TAC[d_word_msb,NOT_LESS_EQUAL] >>
+  `0 < 2` by DECIDE_TAC >>
+  METIS_TAC[MULT_COMM,DIV_thm3,LESS_LESS_EQ_TRANS,LT_MULT_RCANCEL]) >>
+  POP_ASSUM (fn x => fs[x,EXP]) >> POP_ASSUM (K ALL_TAC) >>
+  POP_ASSUM (fn x => ASSUME_TAC (RW [DECIDE ``a*(b*c) = a*c*b``] x)) >>
+  `0 < w2n d` by METIS_TAC[NOT_0w_bis] >>
+  ONCE_REWRITE_TAC[MULT_COMM] >> rw[MULT_DIV] >>
+  METIS_TAC[LE_MULT_CANCEL_LBARE,LESS_EQ_LESS_TRANS,MULT_COMM,EQ_M_R_S_i,EXP_BASE_LT_MONO,DECIDE ``1 < 2``]) >>
+  IMP_RES_TAC TWOEXP_MONO >> rw[LESS_MOD]);
+
+val d_lemma5 = store_thm ("d_lemma5",
+``!(v1:'a word) (d:'a word).
+  2 <= w2n (calc_d (FST(v1,d),1w:'a word)) ==>
+  w2n (calc_d (FST(v1,d),1w:'a word)) * SUC (w2n (FST (v1,d))) <= dimword(:'a)``,
+
+  REPEAT strip_tac >>
+  REWRITE_TAC[dimword_def] >> ASSUME_TAC dimword_def >>  Q.PAT_ABBREV_TAC `m = dimindex(:'a)` >> markerLib.RM_ABBREV_TAC "m" >>
+  ASSUME_TAC (Q.SPECL [`v1:'a word`, `d:'a word`] d_lemma4) >>
+  fs[] >>
+  `n < m` by METIS_TAC[EXP_BASE_LT_MONO,DECIDE ``1 < 2``,w2n_lt] >>
+  `?p. m = n + p` by METIS_TAC[LESS_EQ_EXISTS,LESS_IMP_LESS_OR_EQ] >>
+  `w2n v1 * 2 ** n < 2 ** p * 2 ** n` by METIS_TAC[d_lemma3,FST,EXP_ADD,MULT_COMM] >>
+  POP_ASSUM (fn x => ASSUME_TAC (MP (Q.SPECL [`2 ** p`,`2 ** n`,`w2n (v1:'a word)`] EQ_M_R_S_i) x)) >>
+  `2 ** p = 2 ** m DIV 2 ** n` by METIS_TAC[EXP_ADD,MULT_COMM,MULT_DIV,ZERO_LT_EXP,DECIDE ``0 < 2``] >>
+  METIS_TAC[ZERO_LT_EXP,DECIDE ``0<2``,ADD1,X_LT_DIV,MULT_COMM]);
+
+val d_clauses = store_thm( "d_clauses",
+``!(vs:'a word list) (v1:'a word).
+  (0 < w2n v1) ==>
+  (0 < w2n (calc_d (v1,1w))) /\
+  (mw2n (mw_mul_by_single (calc_d (v1,1w)) (REVERSE (v1::vs))) = mw2n (FRONT (mw_mul_by_single (calc_d (v1,1w)) (REVERSE (v1::vs))))) /\
+  (dimword(:'a) DIV 2 <= w2n (LAST (FRONT (mw_mul_by_single (calc_d (v1,1w)) (REVERSE (v1::vs))))))``,
+
+  REPEAT GEN_TAC >> strip_tac >>
+  qsuff_tac `0 < w2n (calc_d (v1,1w))`
+  THEN1( strip_tac >> strip_tac THEN1 DECIDE_TAC >>
+         Q.PAT_ABBREV_TAC `X = mw_mul_by_single (calc_d (v1,1w)) (REVERSE (v1::vs))` >>
+         `0 < mw2n X` by ALL_TAC
+         THEN1( markerLib.UNABBREV_TAC "X" >>
+                REWRITE_TAC[mw_mul_by_single_lemma] >>
+                MATCH_MP_TAC ((fn (x,y) => y) (EQ_IMP_RULE (SPEC_ALL (ZERO_LESS_MULT)))) >>
+                strip_tac THEN1 DECIDE_TAC >>
+                lrw[mw2n_msf] >>
+                METIS_TAC[ZERO_LT_EXP,ZERO_LT_dimword,ADD_COMM,LESS_EQ_ADD,LESS_LESS_EQ_TRANS,ZERO_LESS_MULT,dimwords_dimword]) >>
+         `X <> []` by METIS_TAC[mw2n_def,NOT_ZERO_LT_ZERO] >>
+         qsuff_tac `mw2n X = mw2n (FRONT X)`
+         THEN1( qsuff_tac `dimword(:'a) DIV 2 * dimwords (LENGTH vs) (:'a) <= mw2n X`
+                THEN1( REPEAT strip_tac THEN1 DECIDE_TAC >>
+                       FULL_SIMP_TAC std_ss [] >>
+                       `FRONT X <> []` by METIS_TAC[NOT_ZERO_LT_ZERO,mw2n_def] >>
+                       `mw2n (FRONT X) = mw2n (FRONT (FRONT X) ++  [LAST (FRONT X)])` by METIS_TAC[APPEND_FRONT_LAST] >>
+                       POP_ASSUM (fn x => FULL_SIMP_TAC std_ss [x,mw2n_msf]) >>
+                       `LENGTH (FRONT (FRONT X)) = LENGTH (vs:'a word list)` by METIS_TAC[rich_listTheory.LENGTH_BUTLAST,prim_recTheory.PRE,
+                        LENGTH,LENGTH_REVERSE,mw_mul_by_single_lemma,ADD1,Abbr`X`] >>
+                        POP_ASSUM (fn x => FULL_SIMP_TAC std_ss [x] THEN ASSUME_TAC x) >>
+                       `mw2n (FRONT (FRONT X)) < dimwords (LENGTH (vs:'a word list)) (:'a) ` by METIS_TAC[mw2n_lt]>>
+                       `mw2n (FRONT (FRONT X)) + dimwords (LENGTH vs) (:'a) * w2n (LAST (FRONT X))
+                        < dimwords (LENGTH vs) (:'a) * (1 + w2n (LAST (FRONT X)))`
+                        by METIS_TAC [LESS_MONO_ADD,MULT_RIGHT_1,LEFT_ADD_DISTRIB] >>
+                       `dimword(:'a) DIV 2 < SUC (w2n (LAST (FRONT X)))` by METIS_TAC[EQ_M_R_S_i,MULT_COMM,LESS_EQ_LESS_TRANS,ADD1,ADD_COMM] >>
+                       DECIDE_TAC) >>
+                `mw2n X = w2n (calc_d (v1,1w)) * mw2n (REVERSE (v1::vs))` by METIS_TAC[mw_mul_by_single_lemma,Abbr`X`] >>
+                POP_ASSUM (fn x => REWRITE_TAC[x]) >>
+                rw[mw2n_msf,LEFT_ADD_DISTRIB] >>
+                REWRITE_TAC[DECIDE ``a*b + a * (c * d) = a*d*c + a*b``] >>
+                `v1 <> 0w` by (Cases_on `v1 = 0w` >> fs[]) >>
+                `!(a:'a word) (b:'a word).w2n (a * b) <= w2n a * w2n b` by rw[word_mul_def,MOD_LESS_EQ] >>
+                METIS_TAC[d_lemma2,FST,LESS_MONO_MULT,LESS_EQ_ADD,LESS_EQ_TRANS]) >>
+         MATCH_MP_TAC mw2n_msf_NIL >> strip_tac THEN1 METIS_TAC[] >>
+         rw[rich_listTheory.LENGTH_BUTLAST] >>
+         markerLib.UNABBREV_TAC "X" >>
+         REWRITE_TAC[mw_mul_by_single_lemma,GSYM ADD1,prim_recTheory.PRE] >>
+         Q.PAT_ABBREV_TAC `Z = w2n (calc_d (v1,1w))` >>
+         Cases_on `Z = 1` THEN1 METIS_TAC[mw2n_lt,DECIDE``1*x = x``] >>
+         fs[mw2n_msf,LEFT_ADD_DISTRIB] >>
+         REWRITE_TAC[DECIDE ``x*y + x*(z*w) = x*w*z + x*y``,EXP] >>
+         Q.PAT_ABBREV_TAC `Y = Z * w2n v1 * dimwords (LENGTH vs) (:'a)` >>
+         Cases_on `v1 = 0w` THEN1 METIS_TAC[word_0_n2w,DECIDE ``~(0<0)``] >>
+         `0 < Z` by METIS_TAC[FST,d_lemma2_bis,NOT_0w_bis] >>
+         `2 <= Z` by DECIDE_TAC >>
+         MATCH_MP_TAC LESS_LESS_EQ_TRANS >>
+         EXISTS_TAC ``Y + Z * dimwords (LENGTH (vs:'a word list)) (:'a)`` >> strip_tac THEN1
+         METIS_TAC[LESS_MONO_ADD,ADD_COMM,MULT_COMM,mw2n_lt,LENGTH_REVERSE,LT_MULT_RCANCEL] >>
+         markerLib.UNABBREV_TAC "Y" >>
+         REWRITE_TAC[dimwords_SUC,DECIDE ``z*v*l + z*l = z*(v+1)*l``,DECIDE ``x * dimword(:'a) = dimword(:'a) * x``] >>
+         MATCH_MP_TAC LESS_MONO_MULT >> METIS_TAC[Abbr`Z`,ADD1,d_lemma5,FST,MULT_COMM]) >>
+  Cases_on `v1 = 0w` THEN1 fs[] >> METIS_TAC[d_lemma2_bis,FST,NOT_0w_bis])
+
+(* Single Division: x1x2 / y *)
+
+val single_div_lemma1 = store_thm ( "single_div_lemma1" ,
+`` w2n (x1:'a word) < w2n (y:'a word) ==>
+   (w2n (x2:'a word) +  dimword(:'a) * w2n x1) DIV w2n y < dimword(:'a)``,
+  strip_tac >> MATCH_MP_TAC DIV_thm2 >> strip_tac THEN1 DECIDE_TAC >>
+  `w2n x2 < dimword(:'a)` by METIS_TAC[w2n_lt] >>
+  `w2n x2 + dimword(:'a) * w2n x1 < dimword(:'a) * SUC (w2n x1)`
+  by METIS_TAC[LESS_MONO_ADD,MULT_RIGHT_1,LEFT_ADD_DISTRIB,ADD1,ADD_COMM] >>
+  METIS_TAC[LESS_EQ,LESS_LESS_EQ_TRANS,LESS_MONO_MULT,MULT_COMM] );
+
+val single_div_lemma2 = store_thm ( "single_div_lemma2",
+  ``y <> 0w ==> w2n (SND (single_div x1 x2 y)) < w2n y``,
+  lrw[single_div_def] >>
+  ` 0 < w2n y` by PROVE_TAC [NOT_0w_bis] >>
+  `0 < dimword(:'a)` by PROVE_TAC[ZERO_LT_dimword] >>
+  Q.PAT_ABBREV_TAC`x = w2n x2 + dimword (:'a) * w2n x1` >>
+  Q.PAT_ABBREV_TAC`z = x MOD w2n y` >>
+  `z < w2n y` by PROVE_TAC[MOD_LESS] >>
+  `z MOD dimword(:'a) <= z` by PROVE_TAC[MOD_LESS_EQ] >>
+  DECIDE_TAC);
+
+val single_div_thm = store_thm ( "single_div_thm",
+  ``!(x1:'a word) (x2:'a word) y q r. (single_div x1 x2 y = (q,r))
+    ==>(((w2n x1 * dimword(:'a) + w2n x2) DIV w2n y < dimword(:'a) /\
+          y <> 0w)
+    ==> ((w2n q = (w2n x1 * dimword(:'a) + w2n x2) DIV w2n y) /\
+         (w2n r = (w2n x1 * dimword(:'a) + w2n x2) MOD w2n y)))``,
+
+  lrw [single_div_def] >> fs [] >> lrw[w2n_n2w] >>
+  `!w. w <> 0w ==> 0 < w2n w` by (Cases_on `w`>> fs [] >> DECIDE_TAC) >>
+  `w2n y < dimword(:'a)` by lrw[w2n_lt] >>
+  METIS_TAC[MOD_LESS,LESS_TRANS] );
+
+val single_div_thm_bis = store_thm ( "single_div_thm_bis",
+  ``!(x1:'a word) (x2:'a word) y q r. (single_div x1 x2 y = (q,r)) /\
+    (w2n x1 < w2n y) ==>
+    (w2n q * w2n y + w2n r = w2n x1 * dimword(:'a) + w2n x2)``,
+
+    REPEAT strip_tac >> IMP_RES_TAC single_div_lemma1 >>
+    qpat_assum `!xs. xxx` (fn x => (ASSUME_TAC (RW [Once ADD_COMM,Once MULT_COMM] (SPEC ``x2:'a word`` x)))) >>
+    Cases_on `y = 0w` THEN1 fs[word_0_n2w] >>
+    IMP_RES_TAC single_div_thm >> `0 < w2n y` by DECIDE_TAC >>
+    METIS_TAC[DIVISION]);
+
+(* Division by single: x_{1}x_{2}...x_{n} / y  *)
+
+val mw_div_by_single_LENGTH = store_thm ("mw_div_by_single_LENGTH",
+``!x xs y. w2n x < w2n y ==>
+    (LENGTH (mw_div_by_single (x::xs) y) = SUC (LENGTH xs))``,
+
+  REPEAT GEN_TAC >>
+  completeInduct_on `LENGTH (x::xs)`>>
+  REPEAT STRIP_TAC >>
+  Cases_on `xs` THEN1 lrw[Once mw_div_by_single_def,single_div_def] >>
+  lrw[Once mw_div_by_single_def,single_div_def] >>
+  Q.PAT_ABBREV_TAC `w:'a word = n2w ((w2n h + dimword (:'a) * w2n x) MOD w2n y)` >>
+  `w2n w < w2n y` by ALL_TAC
+  THEN1 (markerLib.UNABBREV_TAC "w" >>
+         REWRITE_TAC[w2n_n2w] >>
+         METIS_TAC[DECIDE ``!a. 0 <= a``,LESS_EQ_LESS_TRANS,MOD_LESS_EQ,MOD_LESS,ZERO_LT_dimword]) >>
+  METIS_TAC[LENGTH, DECIDE ``n < SUC n``])
+
+val mw_div_by_single_thm = store_thm ( "mw_div_by_single_thm",
+``!xs y. 0 < w2n y ==> (mw2n (REVERSE xs) = mw2n (mw_mul_by_single y (REVERSE (FRONT (mw_div_by_single xs y)))) + w2n (LAST (mw_div_by_single xs y)))``,
+
+HO_MATCH_MP_TAC mw_div_by_single_ind >>
+REPEAT strip_tac
+THEN1 (rw[Once mw_div_by_single_def] >> rw[mw_div_by_single_def,mw_mul_by_single_def,mw_mul_pass_def,mw2n_def])
+THEN1 (rw[single_div_def,mw_mul_by_single_lemma,mw_div_by_single_def,mw2n_def] >>
+       METIS_TAC[MULT_COMM,DIVISION,w2n_lt,LESS_MOD,MOD_LESS_EQ,DIV_LESS_EQ,LESS_EQ_LESS_TRANS]) >>
+Cases_on `(w2n x1 < w2n y \/ (w2n y = 0))` >>
+Q.PAT_ABBREV_TAC `rxs = REVERSE (x1::x2::xs)` >>
+rw[Once mw_div_by_single_def]
+THENL [ALL_TAC,fs[],ALL_TAC]
+THEN1 (`(mw2n (REVERSE (r::xs)) = mw2n (mw_mul_by_single y (REVERSE (FRONT (mw_div_by_single (r::xs) y)))) + w2n (LAST (mw_div_by_single (r::xs) y)))` by METIS_TAC[] >>
+       REPEAT (qpat_assum `!q r. xxx` (K ALL_TAC)) >>
+       rw[Once mw_div_by_single_def] >>
+       `w2n r < w2n y` by ALL_TAC
+       THEN1 ( fs[single_div_def] >>
+             qpat_assum `xxx=r` (fn x => REWRITE_TAC[GSYM x]) >>
+             rw[w2n_n2w] >>
+             METIS_TAC[LESS_EQ_LESS_TRANS,MOD_LESS_EQ,MOD_LESS,ZERO_LT_dimword]) >>
+       `mw_div_by_single (r::xs) y <> []` by
+       METIS_TAC[mw_div_by_single_LENGTH,NOT_NIL_EQ_LENGTH_NOT_0,DECIDE ``0 < SUC n``] >>
+       rw[LAST_DEF,FRONT_DEF,mw2n_msf,mw_mul_by_single_lemma] >>
+       `mw2n rxs = mw2n (REVERSE (r::xs)) + w2n q * w2n y * dimwords (LENGTH xs) (:'a)` by ALL_TAC
+       THEN1(markerLib.UNABBREV_TAC "rxs" >>
+             qpat_assum `mw2n (REVERSE xx) = yy` (K ALL_TAC) >>
+             lrw[mw2n_msf] >>
+             REWRITE_TAC[dimwords_dimword] >>
+             REWRITE_TAC[GSYM ADD1, EXP,
+               DECIDE ``a1 * (d * l) + a2 * l = (a1 * d + a2)*l``,
+               DECIDE ``b * l + d * e * l = (d * e + b)*l``] >>
+             METIS_TAC[single_div_thm_bis]) >>
+       ASM_SIMP_TAC std_ss [mw_mul_by_single_lemma] >>
+       `LENGTH (FRONT (mw_div_by_single (r::xs) y)) = LENGTH xs` by
+       METIS_TAC[mw_div_by_single_LENGTH,DECIDE ``0 < SUC n``,NOT_NIL_EQ_LENGTH_NOT_0,rich_listTheory.LENGTH_BUTLAST,prim_recTheory.PRE] >>
+       RW_TAC arith_ss[]) >>
+`mw2n (REVERSE (r::x2::xs)) = mw2n (mw_mul_by_single y (REVERSE (FRONT (mw_div_by_single (r::x2::xs) y)))) + w2n (LAST (mw_div_by_single (r::x2::xs) y))` by METIS_TAC[] >>
+REPEAT (qpat_assum `!q r. xxx` (K ALL_TAC)) >>
+`mw2n rxs = mw2n (REVERSE (r::x2::xs)) + w2n q * w2n y * dimwords (SUC(LENGTH xs)) (:'a)` by ALL_TAC
+THEN1 (markerLib.UNABBREV_TAC "rxs" >>
+       qpat_assum `mw2n (REVERSE xx) = yy` (K ALL_TAC) >>
+       lrw[mw2n_msf,GSYM ADD1,EXP] >>
+       `w2n x1 = w2n r + w2n q * w2n y` by ALL_TAC
+       THEN1 (IMP_RES_TAC single_div_thm_bis >> ASSUME_TAC word_0_n2w >>
+              FULL_SIMP_TAC arith_ss []) >>
+RW_TAC arith_ss[]) >>
+`(mw_div_by_single (x1::x2::xs) y) = q::mw_div_by_single (r::x2::xs) y` by rw[Once mw_div_by_single_def] >>
+POP_ASSUM (fn x => REWRITE_TAC[x]) >>
+`w2n r < w2n y` by ALL_TAC
+THEN1 ( fs[single_div_def] >>
+      qpat_assum `xxx=r` (fn x => REWRITE_TAC[GSYM x]) >>
+      rw[w2n_n2w] >>
+      METIS_TAC[LESS_EQ_LESS_TRANS,MOD_LESS_EQ,MOD_LESS,ZERO_LT_dimword]) >>
+`mw_div_by_single (r::x2::xs) y <> []` by
+METIS_TAC[mw_div_by_single_LENGTH,NOT_NIL_EQ_LENGTH_NOT_0,DECIDE ``0 < SUC n``] >>
+lrw[mw_mul_by_single_lemma,FRONT_DEF,LAST_DEF,mw2n_msf] >>
+`LENGTH (FRONT (mw_div_by_single (r::x2::xs) y)) = SUC (LENGTH xs)` by
+METIS_TAC[mw_div_by_single_LENGTH,DECIDE ``0 < SUC n``,LENGTH,NOT_NIL_EQ_LENGTH_NOT_0,rich_listTheory.LENGTH_BUTLAST,prim_recTheory.PRE] >>
+RW_TAC arith_ss[])
+
+val mw_div_by_single_thm_bis = store_thm ("mw_div_by_single_thm_bis",
+``!xs y. 0 < w2n y ==>
+  (mw2n (REVERSE (FRONT (mw_div_by_single xs y))) = mw2n (REVERSE xs) DIV w2n y) /\
+  (w2n (LAST (mw_div_by_single xs y)) = mw2n (REVERSE xs) MOD w2n y)``,
+
+  qsuff_tac `! (xs:'a word list) (y:'a word). 0 < w2n y ==>
+               w2n (LAST (mw_div_by_single xs y)) < w2n y`
+  THEN1( REPEAT strip_tac >>
+         IMP_RES_TAC mw_div_by_single_thm >>
+         POP_ASSUM (fn x => ASSUME_TAC (Q.SPECL [`xs:'a word list`] x)) >>
+         FULL_SIMP_TAC std_ss [mw_mul_by_single_lemma] >>
+         ONCE_REWRITE_TAC[MULT_COMM] >>
+         rw[MOD_TIMES,ADD_DIV_ADD_DIV] >>
+         MATCH_MP_TAC ((fn (x,y) => y) (EQ_IMP_RULE (SPEC_ALL EQ_ADDL))) >>
+         MATCH_MP_TAC LESS_DIV_EQ_ZERO >> METIS_TAC[]) >>
+
+  HO_MATCH_MP_TAC mw_div_by_single_ind >>
+  REPEAT strip_tac
+   THEN1 lrw[mw_div_by_single_def]
+  THEN1( lrw[mw_div_by_single_def,single_div_def] >>
+         METIS_TAC[MOD_LESS,LESS_EQ_LESS_TRANS,MOD_LESS_EQ,ZERO_LT_dimword]) >>
+  rw[Once mw_div_by_single_def]
+  THENL[Q.PAT_ABBREV_TAC `w = r::xs`,METIS_TAC[word_0_n2w,NOT_ZERO_LT_ZERO],Q.PAT_ABBREV_TAC `w = r::x2::xs`] >>
+  `w2n r < w2n y` by
+         ( FULL_SIMP_TAC std_ss [single_div_def] >>
+           POP_ASSUM (fn x => REWRITE_TAC[GSYM x]) >>
+           rw[] >>
+           METIS_TAC[MOD_LESS,LESS_EQ_LESS_TRANS,MOD_LESS_EQ,ZERO_LT_dimword]) >>
+  `mw_div_by_single w y <> []` by METIS_TAC[DECIDE ``0 < SUC x``,NOT_NIL_EQ_LENGTH_NOT_0,mw_div_by_single_LENGTH] >>
+  markerLib.UNABBREV_TAC "w" >>
+  rw[listTheory.LAST_CONS_cond,word_0_n2w] >>
+  METIS_TAC[w2n_eq_0])
+
+val mw_simple_div_lemma = prove(
+  ``!xs x y qs (r:'a word) c.
+      (mw_simple_div x xs y = (qs,r,c)) /\ 0w <+ y /\ x <+ y ==>
+      (mw_div_by_single (x::xs) y = SNOC r qs) /\ c``,
+  Induct THEN1
+   (FULL_SIMP_TAC std_ss [mw_simple_div_def,mw_div_by_single_def,WORD_LO]
+    \\ REPEAT STRIP_TAC
+    \\ Cases_on `single_div 0x0w x y` \\ FULL_SIMP_TAC std_ss [SNOC,CONS_11]
+    \\ IMP_RES_TAC single_div_thm_bis
+    \\ FULL_SIMP_TAC (srw_ss()) [w2n_n2w]
+    \\ Cases_on `w2n q` \\ FULL_SIMP_TAC std_ss [MULT_CLAUSES]
+    \\ Cases_on `r` \\ Cases_on `x` \\ FULL_SIMP_TAC (srw_ss()) [w2n_n2w]
+    \\ DECIDE_TAC)
+  \\ SIMP_TAC std_ss [Once mw_simple_div_def,Once mw_div_by_single_def,WORD_LO]
+  \\ NTAC 5 STRIP_TAC
+  \\ Cases_on `single_div x h y` \\ SIMP_TAC std_ss [LET_DEF]
+  \\ `?qs r1 c1. mw_simple_div r' xs y = (qs,r1,c1)` by METIS_TAC [PAIR]
+  \\ ASM_REWRITE_TAC [] \\ SIMP_TAC std_ss [] \\ ONCE_REWRITE_TAC [EQ_SYM_EQ]
+  \\ SIMP_TAC std_ss [SNOC,CONS_11] \\ STRIP_TAC \\ ONCE_REWRITE_TAC [EQ_SYM_EQ]
+  \\ Q.PAT_ASSUM `!x.bb` MATCH_MP_TAC
+  \\ FULL_SIMP_TAC std_ss [WORD_LO]
+  \\ `y <> 0w` by (Cases_on `y` \\ FULL_SIMP_TAC (srw_ss()) [] \\ DECIDE_TAC)
+  \\ `(w2n x * dimword (:'a) + w2n h) DIV w2n y < dimword (:'a)` by ALL_TAC THEN1
+   (FULL_SIMP_TAC (srw_ss()) [DIV_LT_X]
+    \\ MATCH_MP_TAC LESS_LESS_EQ_TRANS
+    \\ Q.EXISTS_TAC `SUC (w2n x) * dimword (:'a)` \\ STRIP_TAC THEN1
+     (FULL_SIMP_TAC std_ss [MULT_CLAUSES] \\ Cases_on `h`
+      \\ FULL_SIMP_TAC (srw_ss()) [DIV_LT_X])
+    \\ SIMP_TAC std_ss [Once MULT_COMM]
+    \\ DECIDE_TAC)
+  \\ IMP_RES_TAC single_div_thm \\ FULL_SIMP_TAC (srw_ss()) []);
+
+val mw2n_SNOC_0 = prove(
+  ``!xs. mw2n (SNOC 0w xs) = mw2n xs``,
+  Induct \\ FULL_SIMP_TAC (srw_ss()) [mw2n_def,SNOC]);
+
+val mw_simple_div_thm = store_thm("mw_simple_div_thm",
+  ``!xs y qs (r:'a word) c.
+      (mw_simple_div 0w xs y = (qs,r,c)) /\ 0w <+ y ==>
+      (mw2n (REVERSE qs) = mw2n (REVERSE xs) DIV w2n y) /\
+      (w2n r = mw2n (REVERSE xs) MOD w2n y) /\ c``,
+  REPEAT STRIP_TAC \\ IMP_RES_TAC mw_simple_div_lemma
+  \\ FULL_SIMP_TAC (srw_ss()) [WORD_LO]
+  \\ IMP_RES_TAC mw_div_by_single_thm_bis
+  \\ REPEAT (Q.PAT_ASSUM `!xs.bbb` (MP_TAC o Q.SPEC `0w::xs`))
+  \\ FULL_SIMP_TAC (srw_ss()) []
+  \\ FULL_SIMP_TAC std_ss [GSYM SNOC_APPEND,FRONT_SNOC,mw2n_SNOC_0]);
+
+
+(* multiWord Division: x_{1}_x{2}...x_{m+n} / y_{1}...y_{n} *)
+
+(* Following the proof on p.271 *)
+
+val mw_div_range1 = store_thm("mw_div_range1",
+  ``! (u1:'a word) u2 us (v1:'a word) vs.
+    (LENGTH us = LENGTH vs) /\
+    0 < w2n v1 /\
+    mw2n (REVERSE (u1::u2::us)) DIV mw2n (REVERSE (v1::vs))
+    < dimword(:'a) ==>
+    MIN ((w2n u1 * dimword(:'a) + w2n u2) DIV w2n v1) (dimword(:'a)-1)
+    >= mw2n (REVERSE (u1::u2::us)) DIV mw2n (REVERSE (v1::vs))``,
+
+    REPEAT GEN_TAC >>
+    Q.PAT_ABBREV_TAC`Q = (w2n u1 * dimword (:'a) + w2n u2) DIV w2n v1` >>
+    Q.PAT_ABBREV_TAC`X = mw2n (REVERSE (u1::u2::us)) DIV mw2n (REVERSE (v1::vs))` >>
+    REPEAT strip_tac >>
+    Cases_on `Q < (dimword(:'a) - 1)` >> lrw[MIN_DEF] >>
+    markerLib.UNABBREV_TAC"X">>
+    `0 < mw2n (REVERSE (v1::vs))` by
+    (fs[mw2n_msf] >> METIS_TAC[dimwords_dimword,ZERO_LT_dimword,ZERO_LT_EXP,LE_MULT_CANCEL_LBARE,LESS_LESS_EQ_TRANS,ADD_COMM,LESS_EQ_ADD,LESS_EQ_TRANS]) >>
+    MATCH_MP_TAC DIV_thm5 >> strip_tac THEN1 DECIDE_TAC >>
+    markerLib.UNABBREV_TAC "Q" >>
+    Q.PAT_ABBREV_TAC`a=(w2n u1) * dimword(:'a) + w2n u2`>>
+    lrw[mw2n_msf,dimwords_dimword] >>
+    Q.PAT_ABBREV_TAC`V1= w2n v1` >>
+    Q.PAT_ABBREV_TAC`U1 = w2n u1` >>
+    Q.PAT_ABBREV_TAC`U2 = w2n u2` >>
+    fs[] >>
+    `a + 1 <= V1 + a DIV V1 * V1`
+    by METIS_TAC[DIV_thm4,LESS_MONO_ADD,DIV_thm3,SUB_ADD,LESS_EQ,ADD1] >>
+    Q.PAT_ABBREV_TAC`q=a DIV V1` >>
+    REWRITE_TAC[GSYM ADD1,EXP] >>
+    Q.PAT_ABBREV_TAC`offset= dimword(:'a) ** (LENGTH t)` >>
+    MATCH_MP_TAC (METIS_PROVE [ADD_COMM,LESS_EQ_ADD,LESS_LESS_EQ_TRANS] ``(a < b) ==> (a < c + b)``) >>
+    REWRITE_TAC[RIGHT_ADD_DISTRIB] >>
+    ONCE_REWRITE_TAC[METIS_PROVE [ADD_ASSOC,ADD_COMM] ``a + (b + c) = b + (a + c)``] >>
+    MATCH_MP_TAC (METIS_PROVE [ADD_COMM,LESS_EQ_ADD,LESS_LESS_EQ_TRANS] ``(a < b) ==> (a < c + b)``) >>
+    RW_TAC arith_ss [] >>
+    ONCE_REWRITE_TAC[DECIDE ``a*b*c = a*c*b``] >> REWRITE_TAC[GSYM RIGHT_ADD_DISTRIB] >>
+    `offset * (a + 1) <= offset * (V1 + q * V1)` by METIS_TAC[LESS_MONO_MULT,MULT_COMM] >>
+    MATCH_MP_TAC LESS_LESS_EQ_TRANS >>
+    EXISTS_TAC ``offset * (a + 1)`` >> lrw[] >>
+    `U2 + U1 * dimword(:'a) = a` by METIS_TAC[Abbr`a`,ADD_COMM] >>
+    ASM_REWRITE_TAC[] >> REWRITE_TAC[LEFT_ADD_DISTRIB] >> RW_TAC arith_ss[] >>
+    METIS_TAC[LENGTH_REVERSE,mw2n_lt,Abbr `offset`,dimwords_dimword]);
+
+(* Proof on p.271-272 *)
+
+val mw_div_range2 = store_thm( "mw_div_range2",
+  ``! (u1:'a word) u2 us (v1:'a word) vs.
+    (LENGTH us = LENGTH vs) /\
+    mw2n (REVERSE (u1::u2::us)) DIV mw2n (REVERSE (v1::vs))
+    < dimword(:'a) /\
+    dimword(:'a) DIV 2 <= w2n v1 ==>
+    MIN ((w2n u1 * dimword(:'a) + w2n u2) DIV w2n v1) (dimword(:'a)-1)
+    <= mw2n (REVERSE (u1::u2::us)) DIV mw2n (REVERSE (v1::vs)) + 2``,
+
+    REPEAT GEN_TAC >>
+    Q.PAT_ABBREV_TAC`V = mw2n (REVERSE (v1::vs))` >>
+    Q.PAT_ABBREV_TAC`U = mw2n (REVERSE (u1::u2::us))`>>
+    Q.PAT_ABBREV_TAC`q = U DIV V` >>
+    Q.PAT_ABBREV_TAC`q' = MIN ((w2n u1 * dimword(:'a) + w2n u2) DIV w2n v1) (dimword(:'a) - 1)` >>
+    Cases_on `V <= U`
+    THEN1( (MATCH_MP_TAC o (fn (x,y) => y)) (EQ_IMP_RULE MONO_NOT_EQ) >>
+           strip_tac >>
+           qpat_assum `~x` (ASSUME_TAC o (fn x => (MP ((fn (x,y)=>x) (EQ_IMP_RULE (Q.SPECL [`q'`,`q+2`] NOT_LESS_EQUAL)))  x))) >>
+           Cases_on `LENGTH us = LENGTH vs`
+           THEN1( Cases_on `q < dimword(:'a)`
+                  THEN1( rw[] >> REWRITE_TAC [NOT_LESS_EQUAL] >>
+                         `3 <= q' - q` by METIS_TAC[SUB_LEFT_LESS,ADD_COMM,LESS_EQ,DECIDE ``3 = SUC 2``] >>
+                         Q.PAT_ABBREV_TAC`b = dimword(:'a)` >> REWRITE_TAC[HD] >>
+                         Cases_on `0 < w2n v1`
+                         THEN1( Q.PAT_ABBREV_TAC`a = w2n v1` >>
+                                `0 < b ** LENGTH vs` by METIS_TAC[Abbr`b`,ZERO_LT_dimword,ZERO_LT_EXP] >>
+                                `0 < V` by (lrw[Abbr`V`,Abbr`a`,mw2n_msf,dimwords_dimword] >> METIS_TAC[ADD_COMM,MULT_COMM,LESS_EQ_ADD,LE_MULT_CANCEL_LBARE,LESS_EQ_TRANS,LESS_LESS_EQ_TRANS]) >>
+                                `b ** (LENGTH vs ) <= V` by (lrw[Abbr`V`,mw2n_msf,LENGTH_REVERSE,dimwords_dimword] >> METIS_TAC[LE_MULT_CANCEL_LBARE,LESS_EQ_ADD,ADD_COMM,LESS_EQ_TRANS]) >>
+                                Cases_on `V = b ** (LENGTH vs)`
+                                THEN1( `V = mw2n ((REVERSE vs)++[v1])` by fs[] >>
+                                       qpat_assum `V = mw2n xxx` (fn x => (ASSUME_TAC (RW [mw2n_msf,LENGTH_REVERSE,dimwords_dimword] x))) >>
+                                       `b ** LENGTH vs * w2n v1 <= V` by METIS_TAC[ADD_COMM,LESS_EQ_ADD] >>
+                                       `0 < b ** LENGTH vs` by METIS_TAC[ZERO_LT_EXP,Abbr`b`,ZERO_LT_dimword] >>
+                                       `a <= 1` by METIS_TAC[Abbr`a`,LE_MULT_CANCEL_RBARE,NOT_ZERO_LT_ZERO] >>
+                                       `a = 1` by DECIDE_TAC  >>
+                                       `U = mw2n (REVERSE us) + V*(w2n u2) + V*b*(w2n u1)` by fs[MULT_COMM,Abbr`b`,Abbr`U`,LENGTH_REVERSE,mw2n_msf,dimwords_dimword,GSYM ADD1,EXP] >>
+                                       qpat_assum `U = xxx` (fn x => ASSUME_TAC(RW[GSYM MULT_ASSOC,GSYM ADD_ASSOC,GSYM LEFT_ADD_DISTRIB] x)) >>
+                                       `mw2n (REVERSE us) < V` by METIS_TAC[mw2n_lt,dimwords_dimword,Abbr`b`,LENGTH_REVERSE] >>
+                                       `q = w2n u1 * b + w2n u2` by METIS_TAC[RIGHT_ADD_DISTRIB,DIV_MULT,ADD_COMM,MULT_COMM] >>
+                                       `q' = MIN (b-1) q` by fs[MIN_COMM] >>
+                                       `~(b - 1 < q)` by DECIDE_TAC >>
+                                       `q' = q` by fs[MIN_DEF] >>
+                                       RW_TAC arith_ss [] ) >>
+                                `b ** (LENGTH vs) < V` by DECIDE_TAC >>
+                                qpat_assum `xxx <> yyy` (fn x => ALL_TAC) >>
+                                `2 * V * (V - b ** (LENGTH vs)) <= U * b ** (LENGTH vs)` by ALL_TAC
+                                THEN1( Q.PAT_ABBREV_TAC`l = b ** LENGTH vs` >>
+                                       `l < V` by METIS_TAC[LE_MULT_CANCEL_LBARE,LESS_EQ_LESS_TRANS] >>
+                                       Q.PAT_ABBREV_TAC`X= V - l` >> `0 < X` by METIS_TAC[SUB_LESS_0] >>
+                                       `0 < l` by METIS_TAC[ZERO_LT_dimword,ZERO_LT_EXP] >>
+                                       `0 < q*V` by METIS_TAC[DIV_GT0,ZERO_LESS_MULT] >>
+                                       `U - V < q * V + V - V` by METIS_TAC[DIV_thm4,DIV_thm3,LESS_MONO_ADD,SUB_ADD,ADD_COMM,LT_SUB_RCANCEL,ADD_0] >>
+                                       qpat_assum `U - V < xxx` (fn x => ASSUME_TAC ( METIS_PROVE[x,ADD_SUB] ``U-V < q*V``)) >>
+                                       `q' <= (w2n u1 * b + w2n u2) DIV a` by lrw[Abbr`a`,Abbr`q'`] >>
+                                       `q' * (a * l) <= (w2n u1 * b + w2n u2) * l` by METIS_TAC[MULT_ASSOC,Abbr`a`,DIV_thm3,LESS_EQ_TRANS,LESS_MONO_MULT,Abbr`q'`] >>
+                                       `U = (w2n u1 * b + w2n u2) * l + mw2n (REVERSE us)` by lrw[Abbr`U`,Abbr`b`,Abbr`l`,mw2n_msf,dimwords_dimword,EXP,GSYM ADD1] >>
+                                       `q' * (a * l) <= U` by METIS_TAC[Abbr`a`,LESS_EQ_ADD,LESS_EQ_TRANS,Abbr`q'`] >>
+                                       Cases_on `U = 0` THEN1 fs[] >>
+                                       `q' * X < U` by ALL_TAC
+                                       THEN1( Cases_on `0 < q'`
+                                              THEN1( `V = a * l + mw2n(REVERSE vs)` by lrw[Abbr`V`,Abbr`l`,Abbr`a`,mw2n_msf,dimwords_dimword] >>
+                                                     `V < a * l + l` by (fs[Abbr`l`,Abbr`b`,Abbr`a`] >> METIS_TAC[mw2n_lt,LENGTH_REVERSE,dimwords_dimword]) >>
+                                                     `0 < a * l` by METIS_TAC[ZERO_LT_EXP,ZERO_LT_dimword, Abbr`a`,ZERO_LESS_MULT] >>
+                                                     `X < a * l` by fs[Abbr`X`,ADD_SUB,LT_SUB_RCANCEL,LT_ADDL,ADD_COMM] >>
+                                                     METIS_TAC[LT_MULT_RCANCEL,MULT_COMM,LESS_LESS_EQ_TRANS]) >>
+                                              DECIDE_TAC) >>
+                                       qpat_assum `q' <= xxx` (fn x => ALL_TAC)>>
+                                       REPEAT (qpat_assum `q' * (a * l) <= xxx` (fn x => ALL_TAC)) >>
+                                       `3 * (X * V) <= q' * (X * V) - q * (X * V) /\
+                                       (q' * (X * V) < U * V) /\
+                                       ((U - V) * X < q * (V * X))`
+                                       by METIS_TAC[LESS_MONO_MULT,RIGHT_SUB_DISTRIB,LT_MULT_RCANCEL,MULT_ASSOC] >>
+                                       `3 * (X * V) <= U * V - (U-V)*X` by DECIDE_TAC >>
+                                       markerLib.UNABBREV_TAC "X" >>
+                                       `3 * ((V-l)*V) <= U*V - ((U-V)*V - (U-V)*l)` by METIS_TAC[LEFT_SUB_DISTRIB] >>
+                                       `(U-V)*l <= (U-V)*V` by METIS_TAC[LESS_IMP_LESS_OR_EQ,LE_MULT_LCANCEL] >>
+                                       `3 * ((V-l)*V) <= U*V + (U-V)*l - (U-V)*V` by METIS_TAC[SUB_SUB] >>
+                                       `3 * ((V-l)*V) <= U*V + (U*l - V*l) - (U*V - V*V)` by METIS_TAC[RIGHT_SUB_DISTRIB]>>
+                                       `3 * ((V-l)*V) <= U*V + (U*l - V*l) + V*V - U*V`by METIS_TAC[LE_MULT_RCANCEL,SUB_SUB] >>
+                                       `3 * ((V-l)*V) <= U*l - V*l + V*V` by METIS_TAC[ADD_ASSOC,PROVE [ADD_COMM,ADD_ASSOC,ADD_SUB] ``a+b-a=b``]>>
+                                       `V*l <= U*l` by METIS_TAC[LESS_MONO_MULT] >>
+                                       `3*((V-l)*V) <= (V*V + U*l) - V*l` by METIS_TAC[ADD_COMM,LESS_MONO_MULT,LESS_EQ_ADD_SUB] >>
+                                       `3*((V-l)*V) <= U*l + V*(V-l)` by METIS_TAC[ADD_COMM,LEFT_SUB_DISTRIB,LESS_EQ_ADD_SUB,SUB_LESS_0,LESS_IMP_LESS_OR_EQ,LE_MULT_LCANCEL] >>
+                                       qpat_assum `xxx <= yyy + V*(V-l)` (fn x =>
+                                                   ASSUME_TAC (RW [DECIDE ``3 = 2 + 1``,RIGHT_ADD_DISTRIB,MULT_LEFT_1] x)) >>
+                                       `(V-l)*V <= V*V` by METIS_TAC[SUB_LESS_EQ,LESS_MONO_MULT] >>
+                                       REPEAT (qpat_assum `3*xxx <= yyy` (fn x => ALL_TAC)) >>
+                                       METIS_TAC[MULT_COMM,MULT_ASSOC,LESS_EQ_MONO_ADD_EQ]) >>
+                               `V = (a-1+1) * b ** LENGTH vs + mw2n(REVERSE vs)` by lrw[Abbr`V`,Abbr`a`,mw2n_msf,dimwords_dimword] >>
+                               qpat_assum `V = xxx` (fn x => (ASSUME_TAC (RW [RIGHT_ADD_DISTRIB,MULT_LEFT_1,Once (DECIDE ``a + b + c = a + c + b``)] x))) >>
+                               `(a - 1) * b ** (LENGTH vs) <= V - b ** (LENGTH vs)`  by METIS_TAC[ADD_SUB,LESS_EQ_ADD] >>
+                               `2 * V * ((a-1) * b ** LENGTH vs) <= 2 * V * (V - b ** LENGTH vs)` by fs[] >>
+                               `2 * V * ((a-1) * b ** LENGTH vs) <= U * b ** LENGTH vs` by METIS_TAC[LESS_EQ_TRANS] >>
+                               qpat_assum `xxx <= U * b ** LENGTH vs` (fn x => ASSUME_TAC (RW [MULT_ASSOC] x)) >>
+                               `b ** LENGTH vs <> 0` by METIS_TAC[ZERO_LT_EXP,Abbr`b`,ZERO_LT_dimword,NOT_ZERO_LT_ZERO] >>
+                               `2 * V * (a-1) <= U` by METIS_TAC[LE_MULT_RCANCEL] >>
+                               qpat_assum `2 * V * xxx <= U` (fn x => (ASSUME_TAC ( RW [Once (DECIDE ``a * b * c = a * c * b``)] x))) >>
+                               `2 * (a-1) <= q` by METIS_TAC[Abbr`q`,DIV_LE_MONOTONE,MULT_DIV] >>
+                               `q + 3 <= q'` by METIS_TAC [LESS_EQ, EVAL ``SUC 2``,ADD,ADD_COMM] >>
+                               `q <= (q' - 3)` by METIS_TAC[LE_SUB_RCANCEL,ADD_SUB,ADD_COMM,LESS_EQ_ADD] >>
+                               qpat_assum ` q + 3 <= q'` (fn x => ALL_TAC) >>
+                               `!xx yy.MIN xx yy <= yy` by rw[] >>
+                               `q' <= b - 1` by METIS_TAC[] >> qpat_assum `!xx yy. zzz` (fn x => ALL_TAC) >>
+                               `2 <= b - 2` by METIS_TAC[SUB_LESS_EQ,LESS_EQ_TRANS,LE_SUB_RCANCEL,DECIDE ``(3-1 = 2)/\(b - 1 - 1 = b - 2)``]  >>
+                               `2 <= 2 * a` by METIS_TAC[LE_MULT_CANCEL_LBARE,Abbr`a`] >>
+                               `q' - 3 <= b - 4` by  METIS_TAC[LE_SUB_RCANCEL,SUB_LESS_EQ,LESS_EQ_TRANS,DECIDE ``x - 1 - 3 = x - 4``] >>
+                               `2 * a <= b - 2` by RW_TAC arith_ss [] >>
+                               qpat_assum `2*a <= xxx` (ASSUME_TAC o (fn x => (METIS_PROVE [DIV_LE_MONOTONE, DECIDE ``0<2``, MULT_COMM,MULT_DIV,x] ``a <= (b - 2) DIV 2``))) >>
+                               `2 <= b` by METIS_TAC[SUB_LESS_EQ, LESS_EQ_TRANS] >>
+                               `a <= (b DIV 2 - 1)` by METIS_TAC[DECIDE ``0<2``,MULT_RIGHT_1,DIV_SUB] >>
+                               RW_TAC arith_ss [Abbr`b`,ZERO_LT_dimword] ) >>
+                       `w2n v1 = 0` by DECIDE_TAC >>
+                       METIS_TAC[DIV_GT0,DECIDE ``0<2``,ONE_LT_dimword,Abbr`b`,LESS_EQ,TWO]) >>
+               DECIDE_TAC)>>
+       DECIDE_TAC)>>
+  strip_tac >>
+  qpat_assum `~x` (fn x => ASSUME_TAC(MP ((fn (x,y) => x)(EQ_IMP_RULE (Q.SPECL [`V`,`U`] NOT_LESS_EQUAL))) x)) >>
+  `LENGTH ((REVERSE us) ++ [u2]) = SUC(LENGTH us)` by lrw[] >>
+  `U = mw2n (REVERSE us) + dimword(:'a) ** LENGTH us * w2n u2 + dimword(:'a) ** (LENGTH(REVERSE us ++ [u2])) * w2n u1` by fs[Abbr`U`,LENGTH_REVERSE,GSYM ADD1,mw2n_msf,dimwords_dimword] >>
+  `U = mw2n (REVERSE us) + dimword(:'a) ** LENGTH us * w2n u2 + dimword(:'a) ** (LENGTH us) * dimword(:'a) * w2n u1` by fs[EXP,MULT_COMM] >>
+  qpat_assum `U = xxx` (fn x => ASSUME_TAC(RW[GSYM MULT_ASSOC,GSYM ADD_ASSOC,GSYM LEFT_ADD_DISTRIB] x)) >>
+  `V = mw2n (REVERSE vs) + dimword(:'a) ** LENGTH vs * w2n v1` by fs[mw2n_msf,dimwords_dimword] >>
+  `V < dimword(:'a) ** LENGTH vs * SUC (w2n v1)` by METIS_TAC[mw2n_lt,LENGTH_REVERSE,LESS_MONO_ADD,MULT,ADD_COMM,MULT_COMM,dimwords_dimword] >>
+  `U < dimword(:'a) ** SUC(LENGTH us)` by METIS_TAC[mw2n_lt,LESS_TRANS,LENGTH_REVERSE,LENGTH,dimwords_dimword]>>
+  `w2n u2 + dimword(:'a) * w2n u1 <= w2n v1` by METIS_TAC[ADD_COMM,LESS_EQ_ADD,LESS_EQ_LESS_TRANS,LESS_TRANS,LT_MULT_LCANCEL,DECIDE ``a < SUC b ==> (a <= b)``] >>
+  `MIN a b <= a` by lrw[] >>
+  `q' <= (w2n u2 +  dimword(:'a)*w2n u1) DIV w2n v1` by fs[ADD_COMM,MULT_COMM,Abbr`q'`]>>
+  `0 < w2n v1` by METIS_TAC[DIV_GT0,DECIDE ``0<2``,ONE_LT_dimword,LESS_EQ,TWO,ONE,LESS_EQ_TRANS]  >>
+  `(w2n u2 +  dimword(:'a)*w2n u1) DIV w2n v1 <= 1` by (Cases_on `w2n u2 + dimword(:'a)*w2n u1 = w2n v1` THEN1 (RW_TAC arith_ss[]) >>
+  `(w2n u2 + dimword(:'a) * w2n u1) < w2n v1` by RW_TAC arith_ss[] >> METIS_TAC[LESS_DIV_EQ_ZERO, DECIDE ``0<=1``]) >>
+  lrw[]);
+
+val mw_div_test_lemma1 = store_thm( "mw_div_test_lemma1",
+``!q u1 u2 u3 v1 v2. w2n (mw_div_test q u1 u2 u3 v1 v2) <= w2n q``,
+    HO_MATCH_MP_TAC mw_div_test_ind >> REPEAT strip_tac >>
+    rw[Once mw_div_test_def] >>
+    `w2n q2 <= w2n q` by
+    METIS_TAC[Abbr`q2`,w2n_n2w,ZERO_LT_dimword,MOD_LESS_EQ,LESS_EQ_TRANS,DECIDE ``x - 1 <=x``] >>
+    Cases_on `mw_cmp [u2; u1] (FST (mw_add [FST s; SND s] [0w; 1w] F)) = SOME T`
+           >> fs[] >> METIS_TAC[LESS_EQ_TRANS])
+
+val mw_div_test_lemma2 = store_thm( "mw_div_test_lemma2",
+``!(us:'a word list) (vs:'a word list).
+  !q u1 u2 u3 v1 v2.
+   (0 < w2n v1) /\ (LENGTH us = LENGTH vs) /\
+   (mw2n (REVERSE (u1::u2::u3::us)) DIV mw2n (REVERSE (v1::v2::vs)) < dimword(:'a)) /\
+   (mw2n (REVERSE (u1::u2::u3::us)) DIV mw2n (REVERSE (v1::v2::vs)) <= w2n q) ==>
+   (mw2n (REVERSE (u1::u2::u3::us)) DIV mw2n (REVERSE (v1::v2::vs))
+    <= w2n (mw_div_test q u1 u2 u3 v1 v2))``,
+
+    GEN_TAC >> GEN_TAC >>
+    HO_MATCH_MP_TAC mw_div_test_ind >>
+    REPEAT strip_tac >>
+    Cases_on `(mw_cmp [u3; u2; u1] (mw_mul_by_single q [v2; v1]) = SOME T)`
+    THEN1( Q.PAT_ABBREV_TAC `u = u1::u2::u3::us` >>
+           Q.PAT_ABBREV_TAC` v = v1::v2::vs` >>
+           rw[Once mw_div_test_def] >>
+           qsuff_tac `mw2n (REVERSE (u:'a word list)) DIV mw2n (REVERSE (v:'a word list)) <= w2n (n2w (w2n (q:'a word) - 1):'a word)`
+           THEN1( strip_tac >>
+                  Cases_on `mw_cmp [u2; u1] (FST (mw_add [FST s; SND s] [0w; 1w] F)) = SOME T` >>
+                  METIS_TAC[Abbr`q2`]) >>
+           qpat_assum `!q'. xxx` (K ALL_TAC) >>
+           qsuff_tac `w2n u1 * dimword (:'a) * dimword (:'a) + w2n u2 * dimword (:'a) + w2n u3 < w2n q * (w2n v1 * dimword (:'a) + w2n v2)`
+           THEN1( strip_tac >>
+                  Cases_on `mw2n (REVERSE u) DIV mw2n (REVERSE v) = 0` THEN1 DECIDE_TAC >>
+                  `0 < w2n q` by DECIDE_TAC >>
+                  `w2n (n2w (w2n (q:'a word) - 1):'a word) = w2n q - 1` by METIS_TAC[w2n_n2w,LESS_MOD,DECIDE ``x - 1 <= x``,LESS_EQ_LESS_TRANS,w2n_lt] >>
+                  POP_ASSUM (fn x => REWRITE_TAC[x]) >>
+                  markerLib.UNABBREV_TAC "v" >>
+                  rw[mw2n_msf,EXP, GSYM ADD1,dimwords_dimword] >>
+                  `0 < w2n v1 * dimword(:'a) + w2n v2`
+                   by METIS_TAC[ZERO_LT_dimword,LE_MULT_CANCEL_LBARE,LESS_EQ_ADD,LESS_EQ_TRANS,LESS_LESS_EQ_TRANS] >>
+                   `0 < dimword(:'a) ** (LENGTH vs)` by  METIS_TAC[ZERO_LT_dimword,ZERO_LT_EXP]  >>
+                   Q.PAT_ABBREV_TAC `U = mw2n (REVERSE u)` >>
+                   qsuff_tac `U DIV ((w2n v1 * dimword(:'a) + w2n v2) * dimword(:'a)**(LENGTH vs)) <= w2n q - 1`
+                   THEN1( Q.PAT_ABBREV_TAC`X = (w2n v1 * dimword(:'a) + w2n v2) * dimword(:'a) ** (LENGTH vs)` >>
+                          Q.PAT_ABBREV_TAC`V = mw2n (REVERSE vs) + dimword (:'a) ** LENGTH vs * w2n v2 + dimword (:'a) * dimword (:'a) ** LENGTH vs * w2n v1` >>
+                          strip_tac >>
+                          `0 < X` by METIS_TAC[Abbr `X`,ZERO_LESS_MULT]>>
+                          `X <= V` by METIS_TAC[LESS_EQ_ADD,LESS_EQ_TRANS,DECIDE ``vs + l*v2 + b*l*v1 = (v1*b + v2)*l + vs``] >>
+                          METIS_TAC[DIV_thm1,LESS_EQ_TRANS]) >>
+                   Q.PAT_ABBREV_TAC`X1 = w2n v1 * dimword(:'a) + w2n v2` >>
+                   Q.PAT_ABBREV_TAC`X2 = dimword(:'a) ** LENGTH vs` >>
+                   `U DIV (X1 * X2) = U DIV X2 DIV X1` by METIS_TAC[MULT_COMM,DIV_DIV_DIV_MULT] >>
+                   qpat_assum `U DIV xxx = yyy` (fn x => REWRITE_TAC[x]) >>
+                   rw[Abbr`U`,Abbr`u`,mw2n_msf,dimwords_dimword,EXP, GSYM ADD1] >>
+                   REWRITE_TAC[DECIDE ``u + x2 * u3 + b * x2 * u2 + b * (b * x2) * u1 = (u3 + u2*b + u1*b*b)*x2 + u``] >>
+                   Q.PAT_ABBREV_TAC`A = (w2n u3 + w2n u2 * dimword (:'a) + w2n u1 * dimword (:'a) * dimword (:'a))` >>
+                   Q.PAT_ABBREV_TAC`B = mw2n (REVERSE us)` >>
+                   `(A * X2 + B) DIV X2 = A` by METIS_TAC[DIV_MULT,Abbr`X2`,Abbr`B`,mw2n_lt,dimwords_dimword,LENGTH_REVERSE] >>
+                   qpat_assum `xx DIV X2 = A` (fn x => REWRITE_TAC[x]) >>
+                   `A < w2n q * X1` by METIS_TAC[ADD_COMM,ADD_ASSOC] >>
+                   `A DIV X1 < w2n q` by METIS_TAC[DIV_thm2] >>
+                   Cases_on `w2n q` THEN1 fs[] >>
+                   METIS_TAC[SUC_SUB1,LESS_EQ,LESS_EQ_MONO]) >>
+            REWRITE_TAC[DECIDE ``a1 * d * d + a2 * d + a3 = a3 + d * (a2 + ( d * a1))``,
+                        DECIDE ``w * (b1 * d + b2) = w *( b2 + d * b1)``] >>
+            `(w2n u1 = mw2n [u1]) /\ (w2n v1 = mw2n [v1])` by lrw[mw2n_def] >>
+            POP_ASSUM (fn x => REWRITE_TAC[x]) >> POP_ASSUM (fn x => REWRITE_TAC[x]) >>
+            REWRITE_TAC[SPEC_ALL (GSYM (CONJUNCT2 mw2n_def)),GSYM (CONJUNCT1 (SPEC_ALL mw_mul_by_single_lemma))] >>
+            `LENGTH [u3;u2;u1] = LENGTH (mw_mul_by_single q [v2;v1])` by lrw[mw_mul_by_single_lemma] >>
+            FULL_SIMP_TAC std_ss [mw_cmp_thm]) >>
+fs[Once mw_div_test_def] )
+
+val q_thm = store_thm( "q_thm",
+``!(u1:'a word) u2 us (v1:'a word) vs.
+  (LENGTH us = LENGTH vs) /\ (0 < w2n v1) /\
+  (mw2n (REVERSE (u1::u2::us)) DIV mw2n (REVERSE (v1::vs)) < dimword(:'a)) ==>
+  w2n u1 * dimword(:'a) + w2n u2 < dimword(:'a) * (1 + w2n v1)``,
+
+    REPEAT GEN_TAC >>
+    Q.PAT_ABBREV_TAC`U = mw2n (REVERSE (u1::u2::us))` >>
+    Q.PAT_ABBREV_TAC`V = mw2n (REVERSE (v1::vs))` >>
+    strip_tac >>
+    EQT_M_R_S_i `dimword(:'a) ** LENGTH (us:'a word list)` >>
+    `0 < V` by (fs[Abbr`V`,mw2n_msf,dimwords_dimword,Once ADD_COMM,Once MULT_COMM]
+            >> METIS_TAC[ZERO_LT_dimword,ZERO_LT_EXP,LESS_EQ_ADD, LE_MULT_CANCEL_LBARE,
+               LESS_LESS_EQ_TRANS]) >>
+    `U < dimword(:'a) * V` by METIS_TAC[DIV_LT_X] >>
+    MATCH_MP_TAC LESS_EQ_LESS_TRANS >> EXISTS_TAC ``(U:num)`` >> strip_tac THEN1(
+    lrw[Abbr`U`,mw2n_msf,dimwords_dimword] >>
+    REWRITE_TAC[ DECIDE  ``(w2 + d * w1) * d ** l = w1 * (d * d ** l) + w2 * d ** l``,GSYM EXP, ADD1] >>
+    METIS_TAC[LESS_EQ_TRANS,LESS_EQ_ADD,ADD_COMM]) >>
+    MATCH_MP_TAC LESS_LESS_EQ_TRANS >> EXISTS_TAC ``dimword(:'a) * V`` >> strip_tac THEN1 DECIDE_TAC >>
+    ASM_REWRITE_TAC[] >>
+    qsuff_tac `V <= (1 + w2n v1) * dimword(:'a) ** LENGTH vs` THEN1 (
+    strip_tac >> METIS_TAC[MULT_COMM,LESS_MONO_MULT,MULT_ASSOC] ) >>
+    lrw[Abbr`V`,mw2n_msf,dimwords_dimword] >> REWRITE_TAC[RIGHT_ADD_DISTRIB,MULT_LEFT_1] >>
+    METIS_TAC[LENGTH_REVERSE,ADD_COMM,LESS_EQ_MONO_ADD_EQ,mw2n_lt,dimwords_dimword,LESS_IMP_LESS_OR_EQ] );
+
+val mw_div_test_thm = store_thm( "mw_div_test_thm",
+``!(u1:'a word) u2 u3 us (v1:'a word) v2 vs.
+  (LENGTH us = LENGTH vs) /\ (dimword(:'a) DIV 2 <= w2n v1) /\
+  (mw2n (REVERSE (u1::u2::u3::us)) DIV (mw2n (REVERSE (v1::v2::vs))) < dimword(:'a))  ==>
+  (let q = if w2n u1 < w2n v1 then FST (single_div u1 u2 v1) else (n2w (dimword(:'a) - 1):'a word) in
+  w2n (mw_div_test q u1 u2 u3 v1 v2) < dimword(:'a) /\ (
+  (w2n (mw_div_test q u1 u2 u3 v1 v2) =
+    mw2n (REVERSE (u1::u2::u3::us)) DIV mw2n (REVERSE (v1::v2::vs))) \/
+   (w2n (mw_div_test q u1 u2 u3 v1 v2) =
+    SUC (mw2n (REVERSE (u1::u2::u3::us)) DIV mw2n (REVERSE (v1::v2::vs))))))``,
+    REPEAT GEN_TAC >>
+    Q.PAT_ABBREV_TAC`U = mw2n (REVERSE (u1::u2::u3::us))` >>
+    Q.PAT_ABBREV_TAC`V = mw2n (REVERSE (v1::v2::vs))` >>
+    Q.PAT_ABBREV_TAC`Q =  U DIV V` >>
+    strip_tac >>
+    Q.PAT_ABBREV_TAC `q = if w2n u1 < w2n v1 then FST (single_div u1 u2 v1) else n2w (dimword (:'a) - 1)` >>
+    rw[] THEN1 METIS_TAC[w2n_lt] >>
+    `LENGTH (u3::us) = LENGTH (v2::vs)` by lrw[] >>
+    `0 < w2n v1` by METIS_TAC[ONE_LT_dimword,DECIDE ``0<2 /\ ((1<x)==>(2 <= x))``,DIV_GT0,LESS_LESS_EQ_TRANS] >>
+    `0 < V` by (fs[Abbr`V`,mw2n_msf,dimwords_dimword,Once ADD_COMM,Once MULT_COMM]
+            >> METIS_TAC[ZERO_LT_dimword,ZERO_LT_EXP,LESS_EQ_ADD, LE_MULT_CANCEL_LBARE,
+               LESS_LESS_EQ_TRANS]) >>
+    `w2n q = MIN ((w2n u1 * dimword (:'a) + w2n u2) DIV w2n v1) (dimword (:'a) - 1)` by ALL_TAC
+    THEN1( markerLib.UNABBREV_TAC "q" >>
+           rw[single_div_def]
+           THEN1( IMP_RES_TAC single_div_lemma1 >>
+                  POP_ASSUM (fn x => ASSUME_TAC (Q.SPECL [`u2:'a word`] x)) >>
+                  FULL_SIMP_TAC arith_ss[] >>
+                  `!a b. (a <= b) ==> (a = MIN a b)` by lrw[MIN_DEF] >>
+                  METIS_TAC[SUB_LESS_OR]) >>
+           `!a b. (a <= b) ==> (a = MIN b a)` by lrw[MIN_DEF,MIN_COMM] >>
+           POP_ASSUM(fn x => MATCH_MP_TAC x) >>
+           `!a b. a * w2n v1 <= b ==> (a <= b DIV w2n v1)` by METIS_TAC[X_LE_DIV] >>
+           POP_ASSUM(fn x => MATCH_MP_TAC x) >>
+           REWRITE_TAC[RIGHT_SUB_DISTRIB] >>
+           METIS_TAC[NOT_LESS,MULT_COMM,LESS_MONO_MULT,SUB_LESS_EQ,LESS_EQ_ADD,LESS_EQ_TRANS]) >>
+    markerLib.RM_ABBREV_TAC "q" >>
+    `dimword(:'a) - 1 < dimword(:'a)` by (Cases_on `dimword(:'a)` >> fs[ZERO_LT_dimword]) >>
+    `w2n q <= dimword(:'a)-1` by METIS_TAC[w2n_lt,SUB_LESS_OR]  >>
+    `w2n q>=Q` by METIS_TAC[Abbr`Q`,mw_div_range1,Abbr `U`, Abbr`V`] >>
+    qpat_assum `w2n q >= Q` (fn x => ASSUME_TAC(METIS_PROVE [x,GREATER_EQ] ``Q <= w2n q``)) >>
+    `Q <= w2n (mw_div_test q u1 u2 u3 v1 v2)` by METIS_TAC[mw_div_test_lemma2] >>
+    `w2n q <= Q + 2` by METIS_TAC[Abbr`Q`,mw_div_range2,Abbr `U`, Abbr`V`] >>
+    REV (Cases_on `w2n q = Q + 2`) THEN1
+      (`w2n q <= SUC Q` by DECIDE_TAC >>
+       Q.PAT_ABBREV_TAC`test = w2n (mw_div_test q u1 u2 u3 v1 v2)` >>
+       `test <> dimword(:'a)` by METIS_TAC[w2n_lt,prim_recTheory.LESS_NOT_EQ] >>
+       `test <= w2n q` by METIS_TAC[mw_div_test_lemma1] >>
+       DECIDE_TAC) >>
+    REV (`mw_cmp [u3; u2; u1] (mw_mul_by_single q [v2; v1]) = SOME T` by ALL_TAC)
+    THEN1 (Q.PAT_ABBREV_TAC`test = w2n (mw_div_test q u1 u2 u3 v1 v2)` >>
+           `test <= w2n q - 1` by ALL_TAC
+           THEN1( markerLib.UNABBREV_TAC "test" >>
+                  REPEAT (qpat_assum `w2n q = xxx` (K ALL_TAC)) >>
+                  rw[Once mw_div_test_def] >>
+                  `w2n q2 = w2n q - 1` by (markerLib.UNABBREV_TAC "q2" >> lrw[]) >>
+                  Cases_on `mw_cmp [u2; u1] (FST (mw_add [FST s; SND s] [0w; 1w] F)) = SOME T` >>
+                  rw[] THEN1 METIS_TAC[LESS_EQ_REFL,LESS_EQ_TRANS,mw_div_test_lemma1] >>
+                  DECIDE_TAC) >>
+           DECIDE_TAC) >>
+    REV (`w2n u1 * dimword(:'a) * dimword(:'a) + w2n u2 * dimword(:'a) + w2n u3 < w2n q * (w2n v1 * dimword(:'a) + w2n v2)` by ALL_TAC)
+    THEN1
+      (qsuff_tac `mw2n [u3;u2;u1] < mw2n (mw_mul_by_single q [v2;v1])`
+       THEN1( `LENGTH [u3;u2;u1] = LENGTH (mw_mul_by_single q [v2;v1])` by METIS_TAC[mw_mul_by_single_lemma,LENGTH,ADD1] >>
+       FULL_SIMP_TAC std_ss [mw_cmp_thm,prim_recTheory.LESS_NOT_EQ]) >>
+       REPEAT (qpat_assum `w2n q = xxx` (K ALL_TAC)) >>
+       FULL_SIMP_TAC arith_ss[mw2n_def,mw_mul_by_single_lemma,LEFT_ADD_DISTRIB]) >>
+    Q.PAT_ABBREV_TAC` b = dimword(:'a)` >>
+    Q.PAT_ABBREV_TAC`V1 = w2n v1` >>
+    Q.PAT_ABBREV_TAC`V2 = w2n v2` >>
+    Q.PAT_ABBREV_TAC`U1 = w2n u1` >>
+    Q.PAT_ABBREV_TAC`U2 = w2n u2` >>
+    Q.PAT_ABBREV_TAC`U3 = w2n u3` >>
+    EQT_M_R_S_i `b**(LENGTH (vs:'a word list))` >>
+    `w2n q * mw2n (REVERSE vs) <= mw2n (REVERSE (us:'a word list)) + mw2n (REVERSE (v1::v2::(vs:'a word list)))` by ALL_TAC
+    THEN1( MATCH_MP_TAC (GEN_ALL (Q.SPECL [`a1*a2`,`a4`,`a5+a4`] LESS_EQ_TRANS)) >>
+           REV strip_tac THEN1 METIS_TAC[LESS_EQ_ADD,ADD_COMM] >>
+           MATCH_MP_TAC LESS_EQ_TRANS >>
+           EXISTS_TAC ``(b:num) * b ** LENGTH (vs:'a word list)`` >>
+           strip_tac THEN1
+             (MATCH_MP_TAC LESS_MONO_MULT2 \\ STRIP_TAC
+              THEN1 (FULL_SIMP_TAC std_ss [])
+              \\ ONCE_REWRITE_TAC [GSYM LENGTH_REVERSE]
+              \\ Q.UNABBREV_TAC `b`
+              \\ FULL_SIMP_TAC std_ss [dimword_def,GSYM EXP_EXP_MULT]
+              \\ ONCE_REWRITE_TAC [MULT_COMM]
+              \\ FULL_SIMP_TAC std_ss [GSYM dimwords_def]
+              \\ MATCH_MP_TAC (DECIDE ``n < m ==> n <= m:num``)
+              \\ SIMP_TAC std_ss [mw2n_lt]) >>
+            markerLib.UNABBREV_TAC "V" >> lrw[mw2n_msf,dimwords_dimword,GSYM ADD1,GSYM EXP]>>
+            ONCE_REWRITE_TAC[DECIDE``a + (b + c) = b + (a + c):num``] >>
+            Cases_on `V1` THEN1 fs[] >>
+            Q.PAT_ABBREV_TAC`A = b ** SUC(LENGTH vs)`>>
+            Q.PAT_ABBREV_TAC`B = mw2n (REVERSE vs) + V2 * b ** LENGTH vs`>>
+            METIS_TAC[MULT,MULT_COMM,ADD_COMM,ADD_ASSOC,LESS_EQ_ADD])>>
+    EQT_A_S_R_2 (`mw2n (REVERSE (us:'a word list)) + mw2n (REVERSE (v1::v2::(vs:'a word list)))`,`w2n (q:'a word) * mw2n (REVERSE (vs:'a word list))`) >>
+    REWRITE_TAC [DECIDE ``(U1 * b * b + U2 * b + U3) * b**y + (u + V:num) =
+                    u + b**y * U3 + b * b**y * U2 + b * b * b**y * U1 + V``] >>
+    markerLib.UNABBREV_TAC "b" >>
+    markerLib.UNABBREV_TAC "U3" >> markerLib.UNABBREV_TAC "U2" >> markerLib.UNABBREV_TAC "U1" >>
+    qpat_assum `LENGTH us = xxx` (fn x => (ASSUME_TAC x THEN REWRITE_TAC[GSYM x])) >>
+    REWRITE_TAC[DECIDE ``b*b*b**c = (b:num)*(b*b**c)``,GSYM EXP, Once
+    (METIS_PROVE [ADD1,LENGTH_APPEND,LENGTH_REVERSE,EVAL ``LENGTH [x]``]``SUC(LENGTH us) = LENGTH ((REVERSE us)++[u3])``),
+    Once (METIS_PROVE [ADD1,LENGTH_APPEND,LENGTH_REVERSE,EVAL ``LENGTH [x]``] ``SUC(SUC(LENGTH us)) = LENGTH (((REVERSE us)++[u3])++[u2])``)] >>
+    REWRITE_TAC[Once (GSYM LENGTH_REVERSE),GSYM mw2n_msf,GSYM dimwords_dimword,METIS_PROVE [REVERSE,SNOC_APPEND] ``(REVERSE xs) ++ [x] = REVERSE (x::xs)``] >>
+    ASM_REWRITE_TAC[] >>
+    REWRITE_TAC[dimwords_dimword]>>
+    REWRITE_TAC[DECIDE``(A:num) * (V1 * b + V2) * b ** c + A * vs = A * (vs + b ** c * V2 + b * b ** c * V1)``,GSYM EXP,
+                  Once (METIS_PROVE [ADD1,LENGTH_APPEND,LENGTH_REVERSE,EVAL ``LENGTH [x]``]``SUC(LENGTH vs) = LENGTH ((REVERSE vs)++[v2])``)] >>
+    markerLib.UNABBREV_TAC"V2" >> markerLib.UNABBREV_TAC "V1" >>
+    REWRITE_TAC[Once (GSYM LENGTH_REVERSE),GSYM mw2n_msf,GSYM dimwords_dimword,METIS_PROVE [REVERSE,SNOC_APPEND] ``(REVERSE xs) ++ [x] = REVERSE (x::xs)``] >>
+    REWRITE_TAC[RIGHT_ADD_DISTRIB,DECIDE ``2 = 1+1:num``,MULT_LEFT_1,ADD_ASSOC] >>
+    MATCH_MP_TAC LESS_MONO_ADD >>
+    METIS_TAC[Abbr`Q`,Abbr`U`,Abbr`V`,DIV_thm4_bis,ADD_COMM,MULT_COMM]);
+
+val mw_div_loop_LENGTH = store_thm( "mw_div_loop_LENGTH",
+``!(zs:'a word list) (ys:'a word list).
+  dimword(:'a) DIV 2 <= w2n (HD ys) /\
+  LENGTH ys < LENGTH zs /\
+  1 < LENGTH ys  ==>
+  (LENGTH (mw_div_loop zs ys) = LENGTH zs)``,
+
+HO_MATCH_MP_TAC mw_div_loop_ind >>
+REPEAT strip_tac >>
+rw[Once mw_div_loop_def] >>
+Cases_on `mw_cmp (REVERSE us) q2ys = SOME T` >>
+rw[]
+THEN1 (qpat_assum `! us q q2. xxx` (K ALL_TAC) >>
+       qpat_assum `! us. xxx` (fn x => ASSUME_TAC (Q.SPECL [`us`,`q`,`q2`,`q2ys`,`q3`,`q3ys`,`zs2'`] x)) >>
+       `LENGTH zs = SUC (LENGTH zs2')` by ALL_TAC
+       THEN1(`LENGTH q3ys = LENGTH us` by METIS_TAC[Abbr`us`,Abbr`q3ys`,mw_mul_by_single_lemma,ADD1,LENGTH_TAKE,LESS_EQ,LENGTH_REVERSE] >>
+             markerLib.UNABBREV_TAC "zs2'" >>
+             REWRITE_TAC[LENGTH_APPEND,LENGTH_REVERSE,LENGTH_DROP] >>
+             Q.PAT_ABBREV_TAC `X = (FST (mw_sub (REVERSE us) q3ys T))` >>
+             `0 < LENGTH us /\ (LENGTH us = SUC(LENGTH ys))` by METIS_TAC[LENGTH_TAKE,LESS_EQ,DECIDE ``0 < SUC x``] >>
+             `X <> [] /\ (LENGTH X = SUC(LENGTH ys))` by METIS_TAC[mw_sub_lemma,PAIR,LENGTH_REVERSE,NOT_NIL_EQ_LENGTH_NOT_0] >>
+             rw[rich_listTheory.LENGTH_BUTLAST,prim_recTheory.PRE] >>
+             RW_TAC arith_ss[]) >>
+       Cases_on `LENGTH ys < LENGTH zs2'` THEN1 METIS_TAC[] >>
+       rw[Once mw_div_loop_def]) >>
+qpat_assum `! us. xxx` (fn x => ASSUME_TAC (Q.SPECL [`us`,`q`,`q2`,`q2ys`,`zs2`] x)) >>
+qpat_assum `! us q q2. xxx` (K ALL_TAC) >>
+`LENGTH zs = SUC (LENGTH zs2)` by ALL_TAC
+THEN1 (`LENGTH q2ys = LENGTH us` by METIS_TAC[Abbr`us`,Abbr`q2ys`,mw_mul_by_single_lemma,ADD1,LENGTH_TAKE,LESS_EQ,LENGTH_REVERSE] >>
+       markerLib.UNABBREV_TAC "zs2" >>
+       REWRITE_TAC[LENGTH_APPEND,LENGTH_REVERSE,LENGTH_DROP] >>
+       Q.PAT_ABBREV_TAC `X = (FST (mw_sub (REVERSE us) q2ys T))` >>
+       `0 < LENGTH us /\ (LENGTH us = SUC(LENGTH ys))` by METIS_TAC[LENGTH_TAKE,LESS_EQ,DECIDE ``0 < SUC x``] >>
+       `X <> [] /\ (LENGTH X = SUC(LENGTH ys))` by METIS_TAC[mw_sub_lemma,PAIR,LENGTH_REVERSE,NOT_NIL_EQ_LENGTH_NOT_0] >>
+       rw[rich_listTheory.LENGTH_BUTLAST,prim_recTheory.PRE] >>
+       RW_TAC arith_ss[]) >>
+Cases_on `LENGTH ys < LENGTH zs2` THEN1 METIS_TAC[] >>
+rw[Once mw_div_loop_def])
+
+val tac_div_loop_1 =
+      `mw2n (REVERSE (TAKE (SUC (LENGTH ys)) zs2)) DIV mw2n (REVERSE ys) < dimword (:'a)` by ALL_TAC
+      THEN1( `SUC (LENGTH ys) < LENGTH zs` by DECIDE_TAC >>
+              markerLib.UNABBREV_TAC "zs2" >>
+              `LENGTH (FRONT w) = LENGTH ys` by METIS_TAC[prim_recTheory.PRE,LENGTH_BUTLAST] >>
+              `LENGTH (REVERSE (FRONT w)) < SUC (LENGTH ys)` by METIS_TAC[LENGTH_REVERSE,DECIDE ``x < SUC x``] >>
+              rw[TAKE_APPEND2,REVERSE_APPEND,SUC_SUB] >>
+              `LENGTH (TAKE 1 (DROP (SUC (LENGTH ys)) zs)) = 1` by METIS_TAC[LENGTH_TAKE,LENGTH_DROP,LESS_EQ,SUB_LESS_0,ONE] >>
+              rw[mw2n_APPEND,dimwords_dimword] >>
+              `!a b. (a < b * mw2n (REVERSE ys) ==> a DIV mw2n (REVERSE ys) < b)` by METIS_TAC[DIV_LT_X] >>
+              POP_ASSUM (fn x => MATCH_MP_TAC x) >>
+              MATCH_MP_TAC LESS_LESS_EQ_TRANS >> EXISTS_TAC ``dimword(:'a) * SUC (mw2n (REVERSE (us:'a word list)) - mw2n (q3ys:'a word list))`` >>
+              strip_tac
+              THEN1( REWRITE_TAC[METIS_PROVE [MULT,MULT_COMM,ADD_COMM] ``a * SUC b = a + a * b``] >>
+                     `!(x:num). x ** 1 = x` by
+                     (GEN_TAC >> REWRITE_TAC[ONE,Q.SPECL [`x`,`0`] (CONJUNCT2 EXP)] >>
+                     RW_TAC arith_ss[]) >>
+                     MATCH_MP_TAC LESS_MONO_ADD >>
+                     METIS_TAC[LESS_MONO_ADD,mw2n_lt,dimwords_dimword,LENGTH_REVERSE]) >>
+              markerLib.UNABBREV_TAC "q3ys" >>
+              ASM_REWRITE_TAC[mw_mul_by_single_lemma] >>
+              METIS_TAC[LESS_MONO_MULT,MULT_COMM,DIV_thm4,LESS_EQ]) >>
+      `mw2n (REVERSE (BUTLASTN (LENGTH ys) (mw_div_loop zs2 ys))) *
+      mw2n (REVERSE ys) + mw2n (REVERSE (LASTN (LENGTH ys) (mw_div_loop zs2 ys))) =
+      mw2n (REVERSE zs2)` by METIS_TAC[] >>
+      qpat_assum ` xx /\ (us = us) /\ yyy ==> zz` (K ALL_TAC) >>
+      `LENGTH ys <= LENGTH (mw_div_loop zs2 ys) /\ (LENGTH (mw_div_loop zs2 ys) = LENGTH zs2)` by METIS_TAC[mw_div_loop_LENGTH,LESS_IMP_LESS_OR_EQ] >>
+      rw[rich_listTheory.LASTN_CONS,rich_listTheory.BUTLASTN_CONS,mw2n_msf,dimwords_dimword,rich_listTheory.LENGTH_BUTLASTN] >>
+      REWRITE_TAC[DECIDE ``(a + b)* c + d = a*c + d + b*c``] >>
+      qpat_assum `xxx = mw2n (REVERSE zs2)` (fn x => REWRITE_TAC[x]) >>
+      markerLib.UNABBREV_TAC "zs2" >> REWRITE_TAC[REVERSE_APPEND,REVERSE_REVERSE,mw2n_APPEND] >>
+      qpat_assum `mw2n (FRONT xx) = mw2n xx` (fn x => REWRITE_TAC[x]) >>
+      REWRITE_TAC[LENGTH_REVERSE,LENGTH_APPEND,LENGTH_DROP] >>
+      fs[rich_listTheory.LENGTH_BUTLAST] >>
+      markerLib.UNABBREV_TAC "q3ys" >>
+      fs[mw_mul_by_single_lemma] >>
+      `zs = us ++ (DROP (SUC(LENGTH ys)) zs)` by METIS_TAC[Abbr`us`,TAKE_DROP] >>
+      POP_ASSUM (fn x => CONV_TAC (RAND_CONV (ONCE_REWRITE_CONV [x]))) >>
+      REWRITE_TAC[REVERSE_APPEND,mw2n_APPEND,dimwords_dimword,LENGTH_DROP,LENGTH_REVERSE] >>
+      REWRITE_TAC[DECIDE ``a + b*c + b*d*e = a + b*(c +d*e)``] >>
+      METIS_TAC[DIV_thm3,SUB_ADD];
+
+val tac_div_loop_2 =
+        rw[Once mw_div_loop_def] >>
+        rw[Once mw_div_loop_def] >> POP_ASSUM (K ALL_TAC) >>
+        `LENGTH zs2 = LENGTH ys` by DECIDE_TAC   >>
+        `LENGTH ys <= LENGTH (q3::zs2)` by METIS_TAC[LENGTH,DECIDE ``n <= SUC n``] >>
+        rw[rich_listTheory.BUTLASTN_CONS,rich_listTheory.LASTN_CONS,mw2n_msf,dimwords_dimword] >>
+        `(BUTLASTN (LENGTH ys) zs2 = []) /\
+         (LASTN (LENGTH ys) zs2 = zs2)` by METIS_TAC[rich_listTheory.BUTLASTN_LENGTH_NIL,rich_listTheory.LASTN_LENGTH_ID] >>
+        POP_ASSUM (fn x => REWRITE_TAC[x]) >>    POP_ASSUM (fn x => REWRITE_TAC[x]) >>
+        RW_TAC arith_ss[LENGTH,REVERSE,mw2n_def] >>
+        markerLib.UNABBREV_TAC "zs2">>
+        ASM_REWRITE_TAC[REVERSE_REVERSE,REVERSE_APPEND,mw2n_APPEND,dimwords_dimword]>>
+        markerLib.UNABBREV_TAC "q3ys" >> rw[mw_mul_by_single_lemma] >>
+        RW_TAC arith_ss[] >>
+        ONCE_REWRITE_TAC[GSYM ADD_ASSOC] >>
+        Q.PAT_ABBREV_TAC `x = mw2n (REVERSE ys) * (mw2n (REVERSE us) DIV mw2n (REVERSE ys))` >>
+        `mw2n (REVERSE us) - x + x = mw2n (REVERSE us)` by METIS_TAC[MULT_COMM,DIV_thm3,SUB_ADD,Abbr`x`] >>
+        POP_ASSUM (fn x => REWRITE_TAC[x]) >>
+        markerLib.UNABBREV_TAC "us" >>
+        `SUC(LENGTH ys) = LENGTH zs` by DECIDE_TAC >> POP_ASSUM (fn x => REWRITE_TAC[x]) >>
+        rw[rich_listTheory.BUTFIRSTN_LENGTH_NIL,listTheory.TAKE_LENGTH_ID,mw2n_def];
+
+val tac_div_loop_test =
+       Cases_on `us` THEN1 fs[] >> Cases_on `t` THEN1 fs[] >> Cases_on `t'` THEN1 fs[] >>
+       Cases_on `ys` THEN1 fs[] >> Cases_on `t'` THEN1 fs[] >>
+       FULL_SIMP_TAC std_ss[HD,TL,LENGTH] >>
+       METIS_TAC[mw_div_test_thm];
+
+val mw_div_loop_thm = store_thm( "mw_div_loop_thm",
+``!(zs:'a word list) (ys:'a word list).
+  dimword(:'a) DIV 2 <= w2n (HD ys) /\
+  LENGTH ys < LENGTH zs /\ 1 < LENGTH ys /\
+  ((mw2n (REVERSE (TAKE (SUC (LENGTH ys)) zs)) DIV mw2n (REVERSE ys)) < dimword(:'a) ) ==>
+  (let rslt = mw_div_loop zs ys in
+   mw2n (REVERSE( BUTLASTN (LENGTH ys) rslt)) * mw2n (REVERSE ys) + mw2n (REVERSE (LASTN (LENGTH ys) rslt)) =
+   mw2n (REVERSE zs))``,
+
+  HO_MATCH_MP_TAC mw_div_loop_ind >> REPEAT strip_tac >>
+  rw[Once mw_div_loop_def] >>
+  markerLib.UNABBREV_TAC "rslt" >>
+  Cases_on `mw_cmp (REVERSE us) q2ys = SOME T` >>
+  rw[]
+
+THENL[qpat_assum `!us. xxx` (K ALL_TAC) >>
+      qpat_assum `!us. xxx` (fn x => ASSUME_TAC (Q.SPECL [`us`,`q`,`q2`,`q2ys`,`q3`,`q3ys`,`zs2'`] x)),
+      qpat_assum `!us. xxx` (fn x => ASSUME_TAC (Q.SPECL [`us`,`q`,`q2`,`q2ys`,`zs2`] x)) >>
+      qpat_assum `!us. xxx` (K ALL_TAC)]
+THENL[ALL_TAC,markerLib.UNABBREV_TAC "q3" >> markerLib.UNABBREV_TAC "q2" >>
+      Q.PAT_ABBREV_TAC `q3 = mw_div_test q (HD us) (HD (TL us)) (HD (TL (TL us))) (HD ys) (HD (TL ys))`] >>
+markerLib.UNABBREV_TAC "zs2" >>
+markerLib.UNABBREV_TAC "zs2'" >>
+markerLib.UNABBREV_TAC "q2ys" >>
+markerLib.UNABBREV_TAC "q3ys" >>
+Q.PAT_ABBREV_TAC `q3ys = (mw_mul_by_single q3 (REVERSE ys))` >>
+Q.PAT_ABBREV_TAC `w = FST (mw_sub (REVERSE us) q3ys T)` >>
+Q.PAT_ABBREV_TAC `zs2 = (REVERSE (FRONT w) ++ DROP (SUC (LENGTH ys)) zs)` >>
+`LENGTH q3ys = LENGTH us` by METIS_TAC[Abbr`us`,Abbr`q3ys`,mw_mul_by_single_lemma,ADD1,LENGTH_TAKE,LESS_EQ,LENGTH_REVERSE] >>
+`0 < LENGTH us /\ (LENGTH us = SUC(LENGTH ys))` by METIS_TAC[LENGTH_TAKE,LESS_EQ,DECIDE ``0 < SUC x``] >>
+`0 < mw2n (REVERSE ys)` by
+        (`ys <> []` by METIS_TAC[NOT_NIL_EQ_LENGTH_NOT_0,DECIDE ``0<1``,LESS_TRANS] >>
+         `?h t. ys = h::t` by METIS_TAC[list_CASES] >>
+         FULL_SIMP_TAC std_ss[HD] >>
+         POP_ASSUM (fn x => lrw[x,mw2n_msf,dimwords_dimword]) >>
+         `0 < dimword(:'a) DIV 2` by METIS_TAC[TWO,DIV_GT0,DECIDE``0<2``,TWO,LESS_EQ,ONE_LT_dimword] >>
+         METIS_TAC[LESS_LESS_EQ_TRANS,ZERO_LT_EXP,ZERO_LT_dimword,LESS_EQ_ADD,ZERO_LESS_MULT,ADD_COMM]) >>
+`w2n q3 = mw2n (REVERSE us) DIV mw2n (REVERSE ys)` by ALL_TAC
+THENL[`(w2n q2 = mw2n (REVERSE us) DIV mw2n (REVERSE ys)) \/(w2n q2 = SUC (mw2n (REVERSE us) DIV mw2n (REVERSE ys)))` by tac_div_loop_test
+       THEN1(`mw2n (REVERSE us) < mw2n (mw_mul_by_single q2 (REVERSE ys))` by FULL_SIMP_TAC std_ss[ADD1,LENGTH,LENGTH_REVERSE,mw_mul_by_single_lemma,mw_cmp_thm] >>
+            POP_ASSUM (fn x => ASSUME_TAC (RW [mw_mul_by_single_lemma] x)) >>
+            qpat_assum `w2n q2 = xxx` (fn x => FULL_SIMP_TAC std_ss [x]) >>
+            METIS_TAC[NOT_LESS,DIV_thm3]) >>
+       METIS_TAC[SUC_SUB1,w2n_n2w,w2n_lt,LESS_MOD,DECIDE ``x < SUC x``,LESS_TRANS,Abbr`q3`],
+      ALL_TAC,
+      `(w2n q3 = mw2n (REVERSE us) DIV mw2n (REVERSE ys)) \/(w2n q3 = SUC (mw2n (REVERSE us) DIV mw2n (REVERSE ys)))` by tac_div_loop_test >>
+      `LENGTH q3ys = LENGTH (REVERSE us)` by METIS_TAC[ADD1,LENGTH,LENGTH_REVERSE,mw_mul_by_single_lemma,Abbr`q3ys`] >>
+      `mw2n q3ys <= mw2n (REVERSE us)` by FULL_SIMP_TAC std_ss[mw_cmp_thm,NOT_LESS] >>
+      markerLib.UNABBREV_TAC "q3ys" >>
+      POP_ASSUM (fn x => ASSUME_TAC (RW [mw_mul_by_single_lemma] x)) >>
+      qpat_assum `w2n q3 = xxx` (fn x => FULL_SIMP_TAC std_ss [x]) >>
+      METIS_TAC[X_LE_DIV,NOT_LESS,DECIDE ``z < SUC z``],
+      ALL_TAC] >>
+`w <> [] /\ (LENGTH w = SUC(LENGTH ys))` by METIS_TAC[mw_sub_lemma,PAIR,LENGTH_REVERSE,NOT_NIL_EQ_LENGTH_NOT_0] >>
+`LENGTH zs = SUC (LENGTH zs2)` by (
+      markerLib.UNABBREV_TAC "zs2" >>
+      REWRITE_TAC[LENGTH_APPEND,LENGTH_REVERSE,LENGTH_DROP] >>
+      rw[rich_listTheory.LENGTH_BUTLAST,prim_recTheory.PRE] >>
+      RW_TAC arith_ss[]) >>
+`mw2n q3ys <= mw2n (REVERSE us)` by METIS_TAC[Abbr`q3ys`,mw_mul_by_single_lemma,DIV_thm3] >>
+`mw2n w = mw2n (REVERSE us) - mw2n q3ys` by METIS_TAC[LENGTH_REVERSE,mw_sub_thm] >>
+`mw2n (FRONT w) = mw2n w` by(
+       `mw2n w < dimword(:'a) ** LENGTH (FRONT w)` by (
+                qpat_assum `mw2n xx = mw2n yy - mw2n zz` (K ALL_TAC) >>
+                rw[rich_listTheory.LENGTH_BUTLAST,prim_recTheory.PRE] >>
+                `mw2n w = mw2n (REVERSE us) - mw2n q3ys` by METIS_TAC[LENGTH_REVERSE,mw_sub_thm] >>
+                POP_ASSUM (fn x => REWRITE_TAC[x]) >>
+                markerLib.UNABBREV_TAC "q3ys" >>
+                ASM_REWRITE_TAC[mw_mul_by_single_lemma] >>
+                METIS_TAC[DIV_thm4,LESS_TRANS,mw2n_lt,dimwords_dimword,LENGTH_REVERSE]) >>
+       METIS_TAC[mw2n_msf_NIL,dimwords_dimword]) >>
+Cases_on `LENGTH ys < LENGTH zs2`
+THENL[tac_div_loop_1,tac_div_loop_2,tac_div_loop_1,tac_div_loop_2]);
+
+val tac_div_loop_bis_1 =
+    `0 < LENGTH zs2` by DECIDE_TAC >>
+    `LENGTH ys <= LENGTH (mw_div_loop zs2 ys)` by METIS_TAC[NOT_NIL_EQ_LENGTH_NOT_0,mw_div_loop_LENGTH,LESS_IMP_LESS_OR_EQ] >>
+    rw[LASTN_CONS] >>
+    `mw2n (REVERSE (TAKE (SUC (LENGTH ys)) zs2)) DIV mw2n (REVERSE ys) < dimword (:'a)` by ALL_TAC
+    THEN1(    `SUC (LENGTH ys) < LENGTH zs` by DECIDE_TAC >>
+              markerLib.UNABBREV_TAC "zs2" >>
+              `LENGTH (FRONT w) = LENGTH ys` by METIS_TAC[prim_recTheory.PRE,LENGTH_BUTLAST] >>
+              `LENGTH (REVERSE (FRONT w)) < SUC (LENGTH ys)` by METIS_TAC[LENGTH_REVERSE,DECIDE ``x < SUC x``] >>
+              rw[TAKE_APPEND2,REVERSE_APPEND,SUC_SUB] >>
+              `LENGTH (TAKE 1 (DROP (SUC (LENGTH ys)) zs)) = 1` by METIS_TAC[LENGTH_TAKE,LENGTH_DROP,LESS_EQ,SUB_LESS_0,ONE] >>
+              rw[mw2n_APPEND,dimwords_dimword] >>
+              `!a b. (a < b * mw2n (REVERSE ys) ==> a DIV mw2n (REVERSE ys) < b)` by METIS_TAC[DIV_LT_X] >>
+              POP_ASSUM (fn x => MATCH_MP_TAC x) >>
+              MATCH_MP_TAC LESS_LESS_EQ_TRANS >> EXISTS_TAC ``dimword(:'a) * SUC (mw2n (REVERSE (us:'a word list)) - mw2n (q3ys:'a word list))`` >>
+              strip_tac
+              THEN1( REWRITE_TAC[METIS_PROVE [MULT,MULT_COMM,ADD_COMM] ``a * SUC b = a + a * b``] >>
+                      `!(x:num). x ** 1 = x` by
+                     (GEN_TAC >> REWRITE_TAC[ONE,Q.SPECL [`x`,`0`] (CONJUNCT2 EXP)] >>
+                     RW_TAC arith_ss[]) >>
+                     MATCH_MP_TAC LESS_MONO_ADD >>
+                     METIS_TAC[LESS_MONO_ADD,mw2n_lt,dimwords_dimword,LENGTH_REVERSE]) >>
+              markerLib.UNABBREV_TAC "q3ys" >>
+              ASM_REWRITE_TAC[mw_mul_by_single_lemma] >>
+              METIS_TAC[LESS_MONO_MULT,MULT_COMM,DIV_thm4,LESS_EQ]) >>
+     METIS_TAC[];
+
+val tac_div_loop_bis_2 =
+rw[Once mw_div_loop_def] >>
+lrw[rich_listTheory.LASTN_CONS,rich_listTheory.LASTN_LENGTH_ID] >>
+markerLib.UNABBREV_TAC "zs2" >>
+`SUC (LENGTH ys) = LENGTH zs` by DECIDE_TAC >>
+POP_ASSUM (fn x => REWRITE_TAC[x]) >>
+REWRITE_TAC[REVERSE_APPEND,REVERSE_REVERSE,rich_listTheory.BUTFIRSTN_LENGTH_NIL,REVERSE,APPEND_NIL] >>
+`LENGTH (REVERSE (FRONT w)) = LENGTH ys` by METIS_TAC[rich_listTheory.LENGTH_BUTLAST,prim_recTheory.PRE,LENGTH_REVERSE] >>
+POP_ASSUM (fn x => ASM_REWRITE_TAC[GSYM x,LASTN_LENGTH_ID,REVERSE_REVERSE]) >>
+markerLib.UNABBREV_TAC "q3ys" >>
+ASM_REWRITE_TAC[mw_mul_by_single_lemma] >>
+METIS_TAC[DIV_thm4];
+
+val mw_div_loop_thm_bis = store_thm ("mw_div_loop_thm_bis",
+``!(zs:'a word list) (ys:'a word list).
+  dimword(:'a) DIV 2 <= w2n (HD ys) /\
+  LENGTH ys < LENGTH zs /\ 1 < LENGTH ys /\
+  ((mw2n (REVERSE (TAKE (SUC (LENGTH ys)) zs)) DIV mw2n (REVERSE ys)) < dimword(:'a) ) ==>
+  (let rslt = mw_div_loop zs ys in
+   (mw2n (REVERSE( BUTLASTN (LENGTH ys) rslt)) = mw2n (REVERSE zs) DIV mw2n (REVERSE ys)) /\
+   (mw2n (REVERSE (LASTN (LENGTH ys) rslt)) = mw2n (REVERSE zs) MOD mw2n (REVERSE ys)))``,
+
+qsuff_tac `!(zs:'a word list) (ys:'a word list).
+           dimword(:'a) DIV 2 <= w2n (HD ys) /\
+           LENGTH ys < LENGTH zs /\ 1 < LENGTH ys /\
+           ((mw2n (REVERSE (TAKE (SUC (LENGTH ys)) zs)) DIV mw2n (REVERSE ys)) < dimword(:'a) ) ==>
+           (mw2n (REVERSE (LASTN (LENGTH ys) (mw_div_loop zs ys))) < mw2n (REVERSE ys))`
+THEN1(REPEAT strip_tac >>
+      rw[] >>
+      IMP_RES_TAC mw_div_loop_thm >>
+      `mw2n (REVERSE zs) = mw2n (REVERSE (BUTLASTN (LENGTH ys) rslt)) * mw2n (REVERSE ys) +
+       mw2n (REVERSE (LASTN (LENGTH ys) rslt))` by METIS_TAC[] >>
+      POP_ASSUM (fn x => REWRITE_TAC[x]) >>
+      `0 < mw2n (REVERSE ys)` by
+        (`ys <> []` by METIS_TAC[NOT_NIL_EQ_LENGTH_NOT_0,DECIDE ``0<1``,LESS_TRANS] >>
+         `?h t. ys = h::t` by METIS_TAC[list_CASES] >>
+         FULL_SIMP_TAC std_ss[HD] >>
+         POP_ASSUM (fn x => lrw[x,mw2n_msf,dimwords_dimword]) >>
+         `0 < dimword(:'a) DIV 2` by METIS_TAC[TWO,DIV_GT0,DECIDE``0<2``,TWO,LESS_EQ,ONE_LT_dimword] >>
+         METIS_TAC[LESS_LESS_EQ_TRANS,ZERO_LT_EXP,ZERO_LT_dimword,LESS_EQ_ADD,ZERO_LESS_MULT,ADD_COMM]) >>
+      rw[MOD_TIMES,ADD_DIV_ADD_DIV,Abbr`rslt`] >>
+      MATCH_MP_TAC ((fn (x,y) => y) (EQ_IMP_RULE (SPEC_ALL EQ_ADDL))) >>
+      MATCH_MP_TAC LESS_DIV_EQ_ZERO >> METIS_TAC[]) >>
+
+HO_MATCH_MP_TAC mw_div_loop_ind >>
+REPEAT strip_tac >>
+rw[Once mw_div_loop_def] >>
+Cases_on `mw_cmp (REVERSE us) q2ys = SOME T` >>
+markerLib.UNABBREV_TAC "q3"
+THENL[Q.PAT_ABBREV_TAC`(q3:'a word) = n2w (w2n q2 - 1)`,markerLib.UNABBREV_TAC "q2" >>
+      Q.PAT_ABBREV_TAC `q3 = mw_div_test q (HD us) (HD (TL us)) (HD (TL (TL us))) (HD ys) (HD (TL ys))`] >>
+markerLib.UNABBREV_TAC "zs2" >>
+markerLib.UNABBREV_TAC "zs2'" >>
+markerLib.UNABBREV_TAC "q2ys" >>
+markerLib.UNABBREV_TAC "q3ys" >>
+Q.PAT_ABBREV_TAC `q3ys = (mw_mul_by_single q3 (REVERSE ys))` >>
+Q.PAT_ABBREV_TAC `w = FST (mw_sub (REVERSE us) q3ys T)` >>
+Q.PAT_ABBREV_TAC `zs2 = (REVERSE (FRONT w) ++ DROP (SUC (LENGTH ys)) zs)` >>
+rw[] >>
+`0 < LENGTH us /\ (LENGTH us = SUC(LENGTH ys))` by METIS_TAC[LENGTH_TAKE,LESS_EQ,DECIDE ``0 < SUC x``] >>
+`LENGTH q3ys = LENGTH us` by METIS_TAC[Abbr`us`,Abbr`q3ys`,mw_mul_by_single_lemma,ADD1,LENGTH_TAKE,LESS_EQ,LENGTH_REVERSE] >>
+`0 < mw2n (REVERSE ys)` by
+        (`ys <> []` by METIS_TAC[NOT_NIL_EQ_LENGTH_NOT_0,DECIDE ``0<1``,LESS_TRANS] >>
+         `?h t. ys = h::t` by METIS_TAC[list_CASES] >>
+         FULL_SIMP_TAC std_ss[HD] >>
+         POP_ASSUM (fn x => lrw[x,mw2n_msf,dimwords_dimword]) >>
+         `0 < dimword(:'a) DIV 2` by METIS_TAC[TWO,DIV_GT0,DECIDE``0<2``,TWO,LESS_EQ,ONE_LT_dimword] >>
+         METIS_TAC[LESS_LESS_EQ_TRANS,ZERO_LT_EXP,ZERO_LT_dimword,LESS_EQ_ADD,ZERO_LESS_MULT,ADD_COMM]) >>
+`w2n q3 = mw2n (REVERSE us) DIV mw2n (REVERSE ys)` by ALL_TAC
+THENL[`(w2n q2 = mw2n (REVERSE us) DIV mw2n (REVERSE ys)) \/(w2n q2 = SUC (mw2n (REVERSE us) DIV mw2n (REVERSE ys)))` by tac_div_loop_test
+       THEN1(`mw2n (REVERSE us) < mw2n (mw_mul_by_single q2 (REVERSE ys))` by FULL_SIMP_TAC std_ss[ADD1,LENGTH,LENGTH_REVERSE,mw_mul_by_single_lemma,mw_cmp_thm] >>
+            POP_ASSUM (fn x => ASSUME_TAC (RW [mw_mul_by_single_lemma] x)) >>
+            qpat_assum `w2n q2 = xxx` (fn x => FULL_SIMP_TAC std_ss [x]) >>
+            METIS_TAC[NOT_LESS,DIV_thm3]) >>
+       METIS_TAC[SUC_SUB1,w2n_n2w,w2n_lt,LESS_MOD,DECIDE ``x < SUC x``,LESS_TRANS,Abbr`q3`],
+      ALL_TAC,
+      `(w2n q3 = mw2n (REVERSE us) DIV mw2n (REVERSE ys)) \/(w2n q3 = SUC (mw2n (REVERSE us) DIV mw2n (REVERSE ys)))` by tac_div_loop_test >>
+      `LENGTH q3ys = LENGTH (REVERSE us)` by METIS_TAC[ADD1,LENGTH,LENGTH_REVERSE,mw_mul_by_single_lemma,Abbr`q3ys`] >>
+      `mw2n q3ys <= mw2n (REVERSE us)` by FULL_SIMP_TAC std_ss[mw_cmp_thm,NOT_LESS] >>
+      markerLib.UNABBREV_TAC "q3ys" >>
+      POP_ASSUM (fn x => ASSUME_TAC (RW [mw_mul_by_single_lemma] x)) >>
+      qpat_assum `w2n q3 = xxx` (fn x => FULL_SIMP_TAC std_ss [x]) >>
+      METIS_TAC[X_LE_DIV,NOT_LESS,DECIDE ``z < SUC z``],
+      ALL_TAC] >>
+`mw2n q3ys <= mw2n (REVERSE us)` by METIS_TAC[Abbr`q3ys`,mw_mul_by_single_lemma,DIV_thm3] >>
+`w <> [] /\ (LENGTH w = SUC(LENGTH ys))` by METIS_TAC[mw_sub_lemma,PAIR,LENGTH_REVERSE,NOT_NIL_EQ_LENGTH_NOT_0] >>
+`mw2n w = mw2n (REVERSE us) - mw2n q3ys` by METIS_TAC[Abbr`w`,LENGTH_REVERSE,mw_sub_thm] >>
+`mw2n (FRONT w) = mw2n w` by (
+       `mw2n w < dimword(:'a) ** LENGTH (FRONT w)` by (
+                qpat_assum `mw2n xx = mw2n yy - mw2n zz` (fn x => (
+                    rw[rich_listTheory.LENGTH_BUTLAST,prim_recTheory.PRE] >>
+                    ASSUME_TAC x)) >>
+                POP_ASSUM (fn x => REWRITE_TAC[x]) >>
+                markerLib.UNABBREV_TAC "q3ys" >>
+                ASM_REWRITE_TAC[mw_mul_by_single_lemma] >>
+                METIS_TAC[DIV_thm4,LESS_TRANS,mw2n_lt,dimwords_dimword,LENGTH_REVERSE]) >>
+       METIS_TAC[mw2n_msf_NIL,dimwords_dimword]) >>
+`LENGTH zs = SUC (LENGTH zs2)` by (
+      markerLib.UNABBREV_TAC "zs2" >>
+      REWRITE_TAC[LENGTH_APPEND,LENGTH_REVERSE,LENGTH_DROP] >>
+      rw[rich_listTheory.LENGTH_BUTLAST,prim_recTheory.PRE] >>
+      RW_TAC arith_ss[]) >>
+Cases_on `LENGTH ys < LENGTH zs2`
+THENL[tac_div_loop_bis_1,tac_div_loop_bis_2,tac_div_loop_bis_1,tac_div_loop_bis_2]);
+
+val mw_div_thm = store_thm ("mw_div_thm" ,
+``!(xs: 'a word list) ys.
+   (0 < mw2n ys) ==> (let rslt = (mw_div xs ys) in
+   (mw2n xs = mw2n (FST rslt) * mw2n ys + mw2n (SND rslt)) /\
+    mw2n (SND rslt) < mw2n ys)``,
+
+rw[]
+THEN1(  markerLib.UNABBREV_TAC "rslt" >>
+        rw[mw_div_def] >>
+        markerLib.UNABBREV_TAC "dxs'" >>
+        markerLib.UNABBREV_TAC "rslt'''" >>
+        markerLib.UNABBREV_TAC "rslt''''" >>
+        markerLib.UNABBREV_TAC "rslt'''''" >>
+        markerLib.UNABBREV_TAC "dxs" >>
+        Q.PAT_ABBREV_TAC `dxs = mw_mul_by_single d txs` >>
+        markerLib.UNABBREV_TAC "rslt" >>
+        Q.PAT_ABBREV_TAC `rslt = mw_div_by_single (REVERSE tyxs) (LAST tys)` >>
+        markerLib.UNABBREV_TAC "rslt''" >>
+        Q.PAT_ABBREV_TAC `rslt'' = mw_div_loop (REVERSE dxs) (REVERSE dys)` >>
+        markerLib.UNABBREV_TAC "rslt'" >>
+        Q.PAT_ABBREV_TAC `rslt'''= (mw_div_loop (REVERSE (SNOC 0w dxs)) (REVERSE dys))` >>
+        rw[]
+        THEN1 METIS_TAC[mw2n_def,mw2n_mw_trailing,DECIDE ``0*a + b = b``]
+        THEN1( markerLib.UNABBREV_TAC "rslt" >> markerLib.UNABBREV_TAC "rslt'''" >>
+               qsuff_tac `0 < w2n (LAST tys) /\ (mw2n ys = w2n (LAST tys))`
+               THEN1 (lrw[mw2n_def] >> markerLib.UNABBREV_TAC "txs" >>
+                     IMP_RES_TAC mw_div_by_single_thm >>
+                     POP_ASSUM (fn x => ASSUME_TAC (Q.SPECL [`REVERSE (mw_trailing (xs:'a word list))`] x)) >>
+                     FULL_SIMP_TAC std_ss [REVERSE_REVERSE,mw2n_mw_trailing,mw_mul_by_single_lemma] >>
+                     RW_TAC arith_ss[]) >>
+               strip_tac THEN1 METIS_TAC[mw_ok_def,NOT_0w_bis,mw_ok_mw_trailing,Abbr`tys`,NOT_NIL_EQ_LENGTH_NOT_0, DECIDE ``0 < 1``] >>
+               markerLib.UNABBREV_TAC "tys" >> REWRITE_TAC[Once (GSYM mw2n_mw_trailing)] >>
+               Cases_on `mw_trailing ys` THEN1 fs[] >> Cases_on `t` THEN1 METIS_TAC[mw2n_def,DECIDE ``a + b*0 = a``,LAST_CONS] >>
+               fs[]) >>
+        `1 < LENGTH tys` by
+             (Cases_on `LENGTH tys = 0` THEN1 METIS_TAC[mw2n_mw_trailing,Abbr`tys`,NOT_ZERO_LT_ZERO,LENGTH_NIL,mw2n_def] >>
+              DECIDE_TAC) >>
+        `tys <> []` by METIS_TAC[mw2n_mw_trailing,Abbr`tys`,mw2n_def,DECIDE ``~(0<0)``] >>
+        `0 < w2n (LAST tys)` by METIS_TAC[mw_ok_mw_trailing,Abbr`tys`,mw_ok_def,NOT_0w_bis] >>
+        `LENGTH dys = LENGTH tys` by
+              (markerLib.UNABBREV_TAC "dys" >>
+              `(mw_mul_by_single d tys <> []) /\ (LENGTH (mw_mul_by_single d tys) = SUC(LENGTH tys))` by METIS_TAC[mw_mul_by_single_lemma,DECIDE ``0<1 /\ (n < SUC n)``,LESS_TRANS,NOT_NIL_EQ_LENGTH_NOT_0,ADD1] >>
+               rw[rich_listTheory.LENGTH_BUTLAST,prim_recTheory.PRE])>>
+        `(dimword(:'a) DIV 2 <= w2n (HD (REVERSE dys))) /\
+         (mw2n dys = mw2n (mw_mul_by_single d tys))` by
+              (`dys <> []` by METIS_TAC[NOT_NIL_EQ_LENGTH_NOT_0] >>
+              markerLib.UNABBREV_TAC "dys" >>
+              `REVERSE tys = (LAST tys)::(REVERSE (FRONT tys))` by ALL_TAC
+              THEN1(`tys = FRONT tys ++ [LAST tys]` by METIS_TAC[APPEND_FRONT_LAST] >>
+                    POP_ASSUM (fn x => CONV_TAC (RATOR_CONV (REWRITE_CONV [Once x]))) >>
+                    lrw[]) >>
+              METIS_TAC[d_clauses,REVERSE_REVERSE,Abbr`d`,HD_REVERSE]) >>
+        markerLib.UNABBREV_TAC "rslt''" >>
+        markerLib.UNABBREV_TAC "rslt'''" >>
+        markerLib.UNABBREV_TAC "dxs"
+        THENL[Q.PAT_ABBREV_TAC `dxs = mw_mul_by_single d txs`, Q.PAT_ABBREV_TAC `dxs = SNOC 0w (mw_mul_by_single d txs)`] >>
+        Q.PAT_ABBREV_TAC`rslt'' = mw_div_loop (REVERSE dxs) (REVERSE dys)` >>
+        `0 < w2n d` by METIS_TAC[NOT_0w_bis,d_lemma2_bis,FST,Abbr`d`]
+        THENL[`mw2n (REVERSE (TAKE (SUC (LENGTH (dys:'a word list))) (REVERSE dxs))) DIV mw2n dys < dimword (:'a)` by
+              (`SUC (LENGTH dys) <= LENGTH dxs` by METIS_TAC[LESS_EQ] >>
+              qpat_assum `mw2n dys = xxx` (K ALL_TAC) >>
+              rw[REVERSE_REVERSE,rich_listTheory.FIRSTN_REVERSE] >>
+              `mw2n (LASTN (LENGTH dys) dxs) < mw2n dys` by FULL_SIMP_TAC std_ss [LESS_IMP_LESS_OR_EQ,LENGTH_LASTN,mw_cmp_thm] >>
+              `dxs = BUTLASTN (LENGTH dys) dxs ++ LASTN (LENGTH dys) dxs` by METIS_TAC[APPEND_BUTLASTN_LASTN,LESS_IMP_LESS_OR_EQ] >>
+              POP_ASSUM (fn x => ONCE_REWRITE_TAC[x]) >>
+              rw[rich_listTheory.LASTN_APPEND1,LENGTH_LASTN,LESS_IMP_LESS_OR_EQ,SUC_SUB] >>
+              qpat_assum `LENGTH dys = xxx` (fn x => REWRITE_TAC[GSYM x]) >>
+              Q.PAT_ABBREV_TAC `Z = LASTN (LENGTH dys) dxs` >>
+              Q.PAT_ABBREV_TAC`X = BUTLASTN (LENGTH dys) dxs` >>
+              `LENGTH (LASTN 1 X) = 1` by METIS_TAC[LESS_IMP_LESS_OR_EQ,LENGTH_LASTN,LENGTH_BUTLASTN,Abbr`X`,SUB_LESS_0,LESS_EQ,ONE] >>
+              rw[mw2n_APPEND,dimwords_dimword] >>
+              `0 < mw2n dys` by DECIDE_TAC >>
+              `!a b. (a < b * mw2n dys ==> a DIV mw2n dys < b)` by METIS_TAC[DIV_LT_X] >>
+              POP_ASSUM (fn x => MATCH_MP_TAC x) >>
+              MATCH_MP_TAC LESS_LESS_EQ_TRANS >> EXISTS_TAC ``dimword(:'a) * SUC (mw2n (Z:'a word list))`` >>
+              REWRITE_TAC[METIS_PROVE [MULT,MULT_COMM,ADD_COMM] ``a * SUC b = a + a * b``] >>
+              `!(x:num). x ** 1 = x` by
+                         (GEN_TAC >> REWRITE_TAC[ONE,Q.SPECL [`x`,`0`] (CONJUNCT2 EXP)] >>
+                         RW_TAC arith_ss[]) >>
+              METIS_TAC[mw2n_lt,dimwords_dimword,LESS_MONO_ADD,LESS_EQ,LESS_MONO_MULT,MULT_COMM,MULT,ADD_COMM]),
+              `mw2n (REVERSE (TAKE (SUC (LENGTH (dys:'a word list))) (REVERSE dxs))) DIV mw2n dys < dimword (:'a)` by
+              (`0 < mw2n dys` by METIS_TAC[Abbr`dys`,mw_mul_by_single_lemma,mw2n_mw_trailing,ZERO_LESS_MULT] >>
+              `!a b. (a < b * mw2n dys ==> a DIV mw2n dys < b)` by METIS_TAC[DIV_LT_X] >>
+              POP_ASSUM (fn x => MATCH_MP_TAC x) >>
+              markerLib.UNABBREV_TAC "dxs" >>
+              rw[REVERSE_SNOC,REVERSE_APPEND,mw2n_APPEND,dimwords_dimword,word_0_n2w,mw2n_def] >>
+              Q.PAT_ABBREV_TAC `Z = REVERSE (mw_mul_by_single d txs)` >>
+              `LENGTH tys <= LENGTH (Z:'a word list)` by METIS_TAC[NOT_LESS,mw_mul_by_single_lemma,LENGTH_REVERSE,LESS_EQ_TRANS,DECIDE ``x <= x + 1``,Abbr`Z`] >>
+              MATCH_MP_TAC LESS_LESS_EQ_TRANS >> EXISTS_TAC ``dimword(:'a) ** LENGTH (tys:'a word list)``  >>
+              strip_tac THEN1 METIS_TAC[LENGTH_TAKE,LENGTH_REVERSE,mw2n_lt,dimwords_dimword] >>
+              rw[mw_mul_by_single_lemma] >>
+              `mw2n tys = mw2n (FRONT tys ++ [LAST tys])` by METIS_TAC[APPEND_FRONT_LAST] >>
+              POP_ASSUM (fn x => REWRITE_TAC[x,Once (DECIDE ``a * (b * c) = b * (a * c)``)]) >>
+              REWRITE_TAC[mw2n_msf,dimwords_dimword,DECIDE ``d * (m + d ** l * w) = d * d ** l * w + d * m``,GSYM EXP] >>
+              rw[LENGTH_BUTLAST] >>
+              `SUC (PRE (LENGTH tys)) = LENGTH tys` by METIS_TAC[SUC_PRE,NOT_NIL_EQ_LENGTH_NOT_0] >>
+              POP_ASSUM (fn x => REWRITE_TAC[x]) >>
+              METIS_TAC[LE_MULT_CANCEL_LBARE,LESS_EQ_ADD,MULT_COMM,LESS_EQ_TRANS]) >>
+              `LENGTH dys < LENGTH dxs` by METIS_TAC[NOT_LESS,LENGTH_SNOC,Abbr`dxs`,ADD1,LESS_TRANS,LESS_EQ_LESS_TRANS,DECIDE ``x < SUC x``,mw_mul_by_single_lemma]] >>
+        `mw2n (REVERSE (BUTLASTN (LENGTH (dys:'a word list)) rslt'')) * mw2n dys + mw2n (REVERSE (LASTN (LENGTH dys) rslt'')) = mw2n dxs`
+                by METIS_TAC[LENGTH_REVERSE,REVERSE_REVERSE,mw_div_loop_thm,Abbr`rslt''`] >>
+        `LENGTH dys <= LENGTH rslt''` by METIS_TAC[LENGTH_REVERSE,mw_div_loop_LENGTH,Abbr`rslt''`,LESS_IMP_LESS_OR_EQ] >>
+        rw[rich_listTheory.BUTFIRSTN_REVERSE] >>
+        qpat_assum `LENGTH dys = xxx` (fn x => REWRITE_TAC[GSYM x] THEN ASSUME_TAC x) >>
+        Cases_on `w2n d` THENL[DECIDE_TAC,ALL_TAC,DECIDE_TAC,ALL_TAC] >> POP_ASSUM (fn x => ASSUME_TAC (GSYM x)) >>
+        MATCH_MP_TAC ((fn (x,y) => x) (EQ_IMP_RULE (Q.SPECL [`n`,`a`,`b`] MULT_SUC_EQ))) >>
+        `!(z:'a word list). mw2n (SNOC 0w z) = mw2n z` by METIS_TAC[SNOC_APPEND,mw2n_msf,dimwords_dimword,DECIDE``x + y*0 = x``,word_0_n2w] >>
+        `(mw2n ys * SUC n = mw2n (dys:'a word list)) /\
+         (mw2n xs * SUC n = mw2n dxs)` by METIS_TAC[mw_mul_by_single_lemma,Abbr`dxs`,MULT_COMM,mw2n_mw_trailing,Abbr`txs`,Abbr`tys`] >>
+        POP_ASSUM (fn x => REWRITE_TAC[x]) >>
+        REWRITE_TAC[RIGHT_ADD_DISTRIB] >>
+        ONCE_REWRITE_TAC[GSYM MULT_ASSOC] >>
+        POP_ASSUM (fn x => REWRITE_TAC[x]) >>
+        qpat_assum `xxx = mw2n dxs` (fn x => ONCE_REWRITE_TAC[GSYM x]) >> RW_TAC arith_ss[] >>
+        `0 < w2n d` by DECIDE_TAC >>
+        IMP_RES_TAC mw_div_by_single_thm_bis >>
+        POP_ASSUM (K ALL_TAC) >> POP_ASSUM (K ALL_TAC) >> POP_ASSUM (K ALL_TAC) >>
+        POP_ASSUM (fn x =>ASM_REWRITE_TAC [Q.SPECL [`LASTN (LENGTH (dys:'a word list)) rslt'':'a word list`] x]) >>
+        Q.PAT_ABBREV_TAC `X = mw2n (REVERSE (LASTN (LENGTH tys) rslt''))` >>
+        `X = X DIV w2n d * w2n d + X MOD w2n d` by METIS_TAC[DIVISION] >>
+        POP_ASSUM (fn x => CONV_TAC (RATOR_CONV (REWRITE_CONV [Once x]))) >>
+        RW_TAC arith_ss[] >> markerLib.UNABBREV_TAC "X" >>
+        `mw2n (REVERSE (LASTN (LENGTH tys) rslt'')) = (mw2n dxs) MOD (mw2n dys)`
+        by METIS_TAC[mw_div_loop_thm_bis,LENGTH_REVERSE,REVERSE_REVERSE,Abbr`rslt''`] >>
+        POP_ASSUM (fn x => REWRITE_TAC[x]) >>
+        rw[Abbr`dxs`,Abbr`dys`,mw_mul_by_single_lemma] >>
+        `0 < mw2n tys` by METIS_TAC[mw2n_mw_trailing,Abbr`tys`] >>
+        rw[GSYM MOD_COMMON_FACTOR] >>
+        METIS_TAC[MULT_COMM,MOD_EQ_0]) >>
+markerLib.UNABBREV_TAC "rslt" >>
+rw[mw_div_def]>>
+rw[]
+THEN1( `mw2n ys = mw2n tys` by METIS_TAC[mw2n_mw_trailing,Abbr`tys`] >> POP_ASSUM (fn x => REWRITE_TAC[x]) >>
+       `tys <> []` by METIS_TAC[mw2n_def,NOT_ZERO_LT_ZERO,mw2n_mw_trailing] >>
+       `tys = FRONT tys ++ [LAST tys]` by METIS_TAC[APPEND_FRONT_LAST] >>
+       POP_ASSUM (fn x => REWRITE_TAC[Once x,mw2n_msf]) >>
+       MATCH_MP_TAC LESS_LESS_EQ_TRANS >> EXISTS_TAC ``dimwords (LENGTH (FRONT (tys:'a word list))) (:'a)`` >> strip_tac
+       THEN1( rw[rich_listTheory.LENGTH_BUTLAST] >>
+              `LENGTH txs <= PRE (LENGTH tys)` by METIS_TAC[NOT_NIL_EQ_LENGTH_NOT_0,INV_PRE_LESS_EQ,LESS_EQ,prim_recTheory.PRE] >>
+              METIS_TAC[mw2n_lt,dimwords_dimword,logrootTheory.LE_EXP_ISO,ONE_LT_dimword,LESS_LESS_EQ_TRANS]) >>
+       `0 < w2n (LAST tys)` by METIS_TAC[mw2n_def,NOT_ZERO_LT_ZERO,mw2n_mw_trailing,mw_ok_def,mw_ok_mw_trailing,Abbr`tys`,w2n_eq_0] >>
+       METIS_TAC[LESS_EQ_ADD,ADD_COMM,LE_MULT_CANCEL_LBARE,LESS_EQ_TRANS])
+THEN1( markerLib.UNABBREV_TAC "rslt" >>
+       `0 < w2n (LAST tys)` by METIS_TAC[mw2n_def,NOT_ZERO_LT_ZERO,mw2n_mw_trailing,mw_ok_def,mw_ok_mw_trailing,Abbr`tys`,w2n_eq_0] >>
+       rw[mw2n_def,mw_div_by_single_thm_bis] >>
+       `mw2n ys = mw2n tys` by METIS_TAC[mw2n_mw_trailing,Abbr`tys`] >> POP_ASSUM (fn x => REWRITE_TAC[x]) >>
+       `tys <> []` by METIS_TAC[mw2n_def,NOT_ZERO_LT_ZERO,mw2n_mw_trailing] >>
+       `mw2n tys = mw2n (FRONT tys ++ [LAST tys])` by METIS_TAC[APPEND_FRONT_LAST] >>
+       POP_ASSUM (fn x => REWRITE_TAC[Once x,mw2n_msf]) >>
+       METIS_TAC[MOD_LESS,LESS_LESS_EQ_TRANS,LESS_EQ_ADD,ADD_COMM,LESS_EQ_TRANS,LE_MULT_CANCEL_LBARE,MULT_COMM,bitTheory.ZERO_LT_TWOEXP,dimwords_def]) >>
+`0 < w2n (LAST tys)` by METIS_TAC[mw2n_def,NOT_ZERO_LT_ZERO,mw2n_mw_trailing,mw_ok_def,mw_ok_mw_trailing,Abbr`tys`,w2n_eq_0] >>
+`0 < w2n d` by METIS_TAC[d_clauses,Abbr`d`] >>
+rw[mw_div_by_single_thm_bis] >>
+markerLib.UNABBREV_TAC "rslt''" >>
+markerLib.UNABBREV_TAC "rslt'" >>
+`1 < LENGTH tys` by
+     (Cases_on `LENGTH tys = 0` THEN1 METIS_TAC[mw2n_mw_trailing,Abbr`tys`,NOT_ZERO_LT_ZERO,LENGTH_NIL,mw2n_def] >>
+      DECIDE_TAC) >>
+`tys <> []` by METIS_TAC[mw2n_mw_trailing,Abbr`tys`,mw2n_def,DECIDE ``~(0<0)``] >>
+`0 < w2n (LAST tys)` by METIS_TAC[mw_ok_mw_trailing,Abbr`tys`,mw_ok_def,NOT_0w_bis] >>
+`LENGTH dys = LENGTH tys` by
+      (markerLib.UNABBREV_TAC "dys" >>
+      `(mw_mul_by_single d tys <> []) /\ (LENGTH (mw_mul_by_single d tys) = SUC(LENGTH tys))` by METIS_TAC[mw_mul_by_single_lemma,DECIDE ``0<1 /\ (n < SUC n)``,LESS_TRANS,NOT_NIL_EQ_LENGTH_NOT_0,ADD1] >>
+       rw[rich_listTheory.LENGTH_BUTLAST,prim_recTheory.PRE])>>
+`(dimword(:'a) DIV 2 <= w2n (HD (REVERSE dys))) /\
+ (mw2n dys = mw2n (mw_mul_by_single d tys))` by
+      (`dys <> []` by METIS_TAC[NOT_NIL_EQ_LENGTH_NOT_0] >>
+      markerLib.UNABBREV_TAC "dys" >>
+      `REVERSE tys = (LAST tys)::(REVERSE (FRONT tys))` by ALL_TAC
+      THEN1(`tys = FRONT tys ++ [LAST tys]` by METIS_TAC[APPEND_FRONT_LAST] >>
+            POP_ASSUM (fn x => CONV_TAC (RATOR_CONV (REWRITE_CONV [Once x]))) >>
+            lrw[]) >>
+      METIS_TAC[d_clauses,REVERSE_REVERSE,Abbr`d`,HD_REVERSE]) >>
+markerLib.UNABBREV_TAC "dxs"
+THENL[Q.PAT_ABBREV_TAC `dxs = mw_mul_by_single d txs`, Q.PAT_ABBREV_TAC `dxs = SNOC 0w (mw_mul_by_single d txs)`] >>
+Q.PAT_ABBREV_TAC`rslt'' = mw_div_loop (REVERSE dxs) (REVERSE dys)` >>
+`0 < w2n d` by METIS_TAC[NOT_0w_bis,d_lemma2_bis,FST,Abbr`d`]
+THENL[`mw2n (REVERSE (TAKE (SUC (LENGTH (dys:'a word list))) (REVERSE dxs))) DIV mw2n dys < dimword (:'a)` by
+              (`SUC (LENGTH dys) <= LENGTH dxs` by METIS_TAC[LESS_EQ] >>
+              qpat_assum `mw2n dys = xxx` (K ALL_TAC) >>
+              rw[REVERSE_REVERSE,rich_listTheory.FIRSTN_REVERSE] >>
+              `mw2n (LASTN (LENGTH dys) dxs) < mw2n dys` by FULL_SIMP_TAC std_ss [LESS_IMP_LESS_OR_EQ,LENGTH_LASTN,mw_cmp_thm] >>
+              `dxs = BUTLASTN (LENGTH dys) dxs ++ LASTN (LENGTH dys) dxs` by METIS_TAC[APPEND_BUTLASTN_LASTN,LESS_IMP_LESS_OR_EQ] >>
+              POP_ASSUM (fn x => ONCE_REWRITE_TAC[x]) >>
+              rw[rich_listTheory.LASTN_APPEND1,LENGTH_LASTN,LESS_IMP_LESS_OR_EQ,SUC_SUB] >>
+              qpat_assum `LENGTH dys = xxx` (fn x => REWRITE_TAC[GSYM x]) >>
+              Q.PAT_ABBREV_TAC `Z = LASTN (LENGTH dys) dxs` >>
+              Q.PAT_ABBREV_TAC`X = BUTLASTN (LENGTH dys) dxs` >>
+              `LENGTH (LASTN 1 X) = 1` by METIS_TAC[LESS_IMP_LESS_OR_EQ,LENGTH_LASTN,LENGTH_BUTLASTN,Abbr`X`,SUB_LESS_0,LESS_EQ,ONE] >>
+              rw[mw2n_APPEND,dimwords_dimword] >>
+              `0 < mw2n dys` by DECIDE_TAC >>
+              `!a b. (a < b * mw2n dys ==> a DIV mw2n dys < b)` by METIS_TAC[DIV_LT_X] >>
+              POP_ASSUM (fn x => MATCH_MP_TAC x) >>
+              MATCH_MP_TAC LESS_LESS_EQ_TRANS >> EXISTS_TAC ``dimword(:'a) * SUC (mw2n (Z:'a word list))`` >>
+              REWRITE_TAC[METIS_PROVE [MULT,MULT_COMM,ADD_COMM] ``a * SUC b = a + a * b``] >>
+              `!(x:num). x ** 1 = x` by
+                         (GEN_TAC >> REWRITE_TAC[ONE,Q.SPECL [`x`,`0`] (CONJUNCT2 EXP)] >>
+                         RW_TAC arith_ss[]) >>
+              METIS_TAC[mw2n_lt,dimwords_dimword,LESS_MONO_ADD,LESS_EQ,LESS_MONO_MULT,MULT_COMM,MULT,ADD_COMM]),
+      `mw2n (REVERSE (TAKE (SUC (LENGTH (dys:'a word list))) (REVERSE dxs))) DIV mw2n dys < dimword (:'a)` by
+              (`0 < mw2n dys` by METIS_TAC[Abbr`dys`,mw_mul_by_single_lemma,mw2n_mw_trailing,ZERO_LESS_MULT] >>
+              `!a b. (a < b * mw2n dys ==> a DIV mw2n dys < b)` by METIS_TAC[DIV_LT_X] >>
+              POP_ASSUM (fn x => MATCH_MP_TAC x) >>
+              markerLib.UNABBREV_TAC "dxs" >>
+              rw[REVERSE_SNOC,REVERSE_APPEND,mw2n_APPEND,dimwords_dimword,word_0_n2w,mw2n_def] >>
+              Q.PAT_ABBREV_TAC `Z = REVERSE (mw_mul_by_single d txs)` >>
+              `LENGTH tys <= LENGTH (Z:'a word list)` by METIS_TAC[NOT_LESS,mw_mul_by_single_lemma,LENGTH_REVERSE,LESS_EQ_TRANS,DECIDE ``x <= x + 1``,Abbr`Z`] >>
+              MATCH_MP_TAC LESS_LESS_EQ_TRANS >> EXISTS_TAC ``dimword(:'a) ** LENGTH (tys:'a word list)``  >>
+              strip_tac THEN1 METIS_TAC[LENGTH_TAKE,LENGTH_REVERSE,mw2n_lt,dimwords_dimword] >>
+              rw[mw_mul_by_single_lemma] >>
+              `mw2n tys = mw2n (FRONT tys ++ [LAST tys])` by METIS_TAC[APPEND_FRONT_LAST] >>
+              POP_ASSUM (fn x => REWRITE_TAC[x,Once (DECIDE ``a * (b * c) = b * (a * c)``)]) >>
+              REWRITE_TAC[mw2n_msf,dimwords_dimword,DECIDE ``d * (m + d ** l * w) = d * d ** l * w + d * m``,GSYM EXP] >>
+              rw[LENGTH_BUTLAST] >>
+              `SUC (PRE (LENGTH tys)) = LENGTH tys` by METIS_TAC[SUC_PRE,NOT_NIL_EQ_LENGTH_NOT_0] >>
+              POP_ASSUM (fn x => REWRITE_TAC[x]) >>
+              METIS_TAC[LE_MULT_CANCEL_LBARE,LESS_EQ_ADD,MULT_COMM,LESS_EQ_TRANS]) >>
+              `LENGTH dys < LENGTH dxs` by METIS_TAC[NOT_LESS,LENGTH_SNOC,Abbr`dxs`,ADD1,LESS_TRANS,LESS_EQ_LESS_TRANS,DECIDE ``x < SUC x``,mw_mul_by_single_lemma]] >>
+        `mw2n (REVERSE (LASTN (LENGTH (dys:'a word list)) rslt'')) = mw2n dxs MOD mw2n dys` by METIS_TAC[REVERSE_REVERSE,mw_div_loop_thm_bis,LENGTH_REVERSE] >>
+        POP_ASSUM (fn x => REWRITE_TAC[x]) >>
+        rw[mw_mul_by_single_lemma] >>
+        `0 < mw2n tys` by METIS_TAC[mw2n_mw_trailing,Abbr`tys`] >>
+        rw[GSYM DIV_MOD_MOD_DIV] >>
+        METIS_TAC[MOD_LESS,mw2n_mw_trailing,Abbr`tys`]);
+
+(* converting into decimal form *)
+
+val num_to_dec_string_unroll = prove(
+  ``!n. num_to_dec_string n =
+          SNOC (CHR (48 + n MOD 10))
+               (if n < 10 then [] else num_to_dec_string (n DIV 10))``,
+  SIMP_TAC std_ss [num_to_dec_string_def,n2s_def]
+  \\ SIMP_TAC std_ss [Once numposrepTheory.n2l_def] \\ SRW_TAC [] []
+  THEN1 (Cases_on `(n=0) \/ (n=1) \/ (n=2) \/ (n=3) \/ (n=4) \/
+                   (n=5) \/ (n=6) \/ (n=7) \/ (n=8) \/ (n=9)`
+         \\ FULL_SIMP_TAC std_ss [] \\ EVAL_TAC \\ `F` by DECIDE_TAC)
+  \\ `n MOD 10 < 10` by FULL_SIMP_TAC std_ss []
+  \\ Q.ABBREV_TAC `k = n MOD 10`
+  THEN1 (Cases_on `(k=0) \/ (k=1) \/ (k=2) \/ (k=3) \/ (k=4) \/
+                   (k=5) \/ (k=6) \/ (k=7) \/ (k=8) \/ (k=9)`
+         \\ FULL_SIMP_TAC std_ss [] \\ EVAL_TAC \\ `F` by DECIDE_TAC));
+
+val mw_to_dec_def = tDefine "mw_to_dec" `
+  mw_to_dec (xs:'a word list) =
+    if dimword (:'a) <= 10 then ([],F) else
+      let (qs,r,c1) = mw_simple_div 0w (REVERSE xs) 10w in
+      let qs = mw_trailing (REVERSE qs) in
+        if LENGTH qs = 0 then
+          ([r + 48w],c1)
+        else
+          let (result,c2) = mw_to_dec qs in
+            (result ++ [r + 48w],c1 /\ c2)`
+ (WF_REL_TAC `measure (mw2n)` \\ REPEAT STRIP_TAC
+  \\ Q.PAT_ASSUM `(xx,yy) = zz` (ASSUME_TAC o GSYM)
+  \\ FULL_SIMP_TAC std_ss [GSYM NOT_LESS]
+  \\ `0x0w <+ 10w` by FULL_SIMP_TAC (srw_ss()) [WORD_LO]
+  \\ IMP_RES_TAC mw_simple_div_thm
+  \\ FULL_SIMP_TAC (srw_ss()) [REVERSE_REVERSE,mw2n_mw_trailing]
+  \\ FULL_SIMP_TAC std_ss [DIV_LT_X,mw_trailing_LENGTH_ZERO]
+  \\ Q.PAT_ASSUM `10 < dimword (:'a)` ASSUME_TAC
+  \\ FULL_SIMP_TAC std_ss [DIV_EQ_X,NOT_LESS]
+  \\ DECIDE_TAC);
+
+val mw_to_dec_thm = store_thm("mw_to_dec_thm",
+  ``!(xs:'a word list).
+      10 < dimword (:'a) ==>
+      (mw_to_dec xs = (MAP (n2w o ORD) (num_to_dec_string (mw2n xs)),T))``,
+  STRIP_TAC \\ STRIP_ASSUME_TAC (SPEC_ALL n2mw_EXISTS)
+  \\ Q.PAT_ASSUM `xs = bb` (fn th => ONCE_REWRITE_TAC [th])
+  \\ POP_ASSUM MP_TAC \\ Q.SPEC_TAC (`xs`,`xs`)
+  \\ completeInduct_on `k` \\ ONCE_REWRITE_TAC [mw_to_dec_def]
+  \\ FULL_SIMP_TAC std_ss [GSYM NOT_LESS,LET_DEF] \\ STRIP_TAC
+  \\ `?x1 x2 x3. mw_simple_div 0x0w (REVERSE (n2mw (LENGTH (xs:'a word list)) k)) 0xAw = (x1,x2:'a word,x3)` by METIS_TAC [PAIR]
+  \\ FULL_SIMP_TAC std_ss [] \\ REPEAT STRIP_TAC
+  \\ `0x0w <+ 10w` by FULL_SIMP_TAC (srw_ss()) [WORD_LO]
+  \\ IMP_RES_TAC mw_simple_div_thm
+  \\ FULL_SIMP_TAC std_ss [REVERSE_REVERSE]
+  \\ IMP_RES_TAC mw2n_n2mw \\ FULL_SIMP_TAC (srw_ss()) [w2n_n2w]
+  \\ Q.PAT_ASSUM `10 < dimword (:'a)` ASSUME_TAC \\ FULL_SIMP_TAC std_ss []
+  \\ FULL_SIMP_TAC std_ss [PULL_FORALL,AND_IMP_INTRO]
+  \\ FULL_SIMP_TAC std_ss [mw_trailing_LENGTH_ZERO]
+  \\ ONCE_REWRITE_TAC [num_to_dec_string_unroll]
+  \\ `(k DIV 10 = 0) = k < 10` by ALL_TAC
+  THEN1 FULL_SIMP_TAC std_ss [DIV_EQ_X,NOT_LESS]
+  \\ FULL_SIMP_TAC std_ss []
+  \\ Cases_on `k < 10` \\ FULL_SIMP_TAC std_ss [] THEN1
+   (EVAL_TAC \\ `48 + k < 256` by DECIDE_TAC
+    \\ Cases_on `x2` \\ FULL_SIMP_TAC (srw_ss()) [SNOC,MAP,word_add_n2w]
+    \\ FULL_SIMP_TAC std_ss [AC ADD_COMM ADD_ASSOC])
+  \\ Q.PAT_ASSUM `!m. bbb` (MP_TAC o Q.SPECL [`k DIV 10`,`(mw_trailing (REVERSE x1))`])
+  \\ MATCH_MP_TAC (METIS_PROVE [] ``b /\ (c ==> d) ==> ((b ==> c) ==> d)``)
+  \\ STRIP_TAC THEN1
+   (FULL_SIMP_TAC std_ss [DIV_LT_X,NOT_LESS]
+    \\ `0 < dimwords (LENGTH x1) (:'a)` by FULL_SIMP_TAC std_ss [ZERO_LT_dimwords]
+    \\ STRIP_TAC THEN1 DECIDE_TAC
+    \\ MP_TAC (Q.SPEC `(mw_trailing (REVERSE x1))` mw2n_lt)
+    \\ FULL_SIMP_TAC std_ss [mw2n_mw_trailing,DIV_LT_X])
+  \\ REPEAT STRIP_TAC \\ FULL_SIMP_TAC std_ss []
+  \\ `(n2mw (LENGTH (mw_trailing (REVERSE x1))) (k DIV 10)) =
+      (mw_trailing (REVERSE x1))` by ALL_TAC THEN1
+   (MP_TAC (Q.SPEC `mw_trailing (REVERSE x1)` n2mw_mw2n)
+    \\ FULL_SIMP_TAC std_ss [mw2n_mw_trailing])
+  \\ FULL_SIMP_TAC std_ss []
+  \\ Cases_on `x2` \\ FULL_SIMP_TAC std_ss [mw2n_mw_trailing]
+  \\ FULL_SIMP_TAC (srw_ss()) [word_add_n2w]
+  \\ `k MOD 10 < 10` by FULL_SIMP_TAC (srw_ss()) []
+  \\ `48 + k MOD 10 < 256` by DECIDE_TAC
+  \\ FULL_SIMP_TAC (srw_ss()) []
+  \\ FULL_SIMP_TAC std_ss [AC ADD_COMM ADD_ASSOC]);
+
+
+(* extra *)
+
+val LESS_EQ_LENGTH = store_thm("LESS_EQ_LENGTH",
+  ``!xs n. n <= LENGTH xs ==> ?xs1 xs2. (xs = xs1 ++ xs2) /\ (LENGTH xs1 = n)``,
+  Induct \\ FULL_SIMP_TAC (srw_ss()) [LENGTH,LENGTH_NIL]
+  \\ Cases_on `n` \\ FULL_SIMP_TAC (srw_ss()) [LENGTH_NIL]
+  \\ REPEAT STRIP_TAC \\ RES_TAC \\ FULL_SIMP_TAC std_ss []
+  \\ Q.LIST_EXISTS_TAC [`h::xs1`,`xs2`] \\ FULL_SIMP_TAC (srw_ss()) []);
+
+val LENGTH_mw_add = store_thm("LENGTH_mw_add",
+  ``!xs1 ys c qs1 c1. (mw_add xs1 ys c = (qs1,c1)) ==> (LENGTH xs1 = LENGTH qs1)``,
+  Induct \\ FULL_SIMP_TAC std_ss [mw_add_def,LET_DEF,single_add_def]
+  \\ CONV_TAC (DEPTH_CONV PairRules.PBETA_CONV) \\ REPEAT STRIP_TAC
+  \\ Q.ABBREV_TAC `t = (dimword (:'a) <= w2n h + w2n (HD ys) + b2n c)`
+  \\ `?x1 x2. mw_add xs1 (TL ys) t = (x1,x2)` by METIS_TAC [PAIR]
+  \\ RES_TAC \\ Cases_on `qs1` \\ FULL_SIMP_TAC (srw_ss()) []);
+
+val LENGTH_mw_sub = store_thm("LENGTH_mw_sub",
+  ``!xs1 ys c qs1 c1. (mw_sub xs1 ys c = (qs1,c1)) ==> (LENGTH xs1 = LENGTH qs1)``,
+  Induct \\ FULL_SIMP_TAC std_ss [mw_sub_def,LET_DEF,single_add_def,single_sub_def]
+  \\ CONV_TAC (DEPTH_CONV PairRules.PBETA_CONV) \\ REPEAT STRIP_TAC
+  \\ Q.ABBREV_TAC `t = (dimword (:'a) <= w2n h + w2n (~HD ys) + b2n c)`
+  \\ `?x1 x2. mw_sub xs1 (TL ys) t = (x1,x2)` by METIS_TAC [PAIR]
+  \\ RES_TAC \\ Cases_on `qs1` \\ FULL_SIMP_TAC (srw_ss()) []);
+
+val LENGTH_mw_trailing = store_thm("LENGTH_mw_trailing",
+  ``!xs. LENGTH (mw_trailing xs) <= LENGTH xs``,
+  HO_MATCH_MP_TAC SNOC_INDUCT \\ REPEAT STRIP_TAC
+  \\ SIMP_TAC (srw_ss()) [Once mw_trailing_def] \\ SRW_TAC [] []
+  \\ DECIDE_TAC);
+
+val LENGTH_mw_trailing_IMP = store_thm("LENGTH_mw_trailing_IMP",
+  ``(LENGTH xs = LENGTH ys) ==>
+    LENGTH (mw_trailing xs) <= LENGTH ys``,
+  METIS_TAC [LENGTH_mw_trailing]);
+
+val LENGTH_mw_subv = store_thm("LENGTH_mw_subv",
+  ``!ys xs. LENGTH xs <= LENGTH ys ==> (LENGTH (mw_subv ys xs) <= LENGTH ys)``,
+  REPEAT STRIP_TAC \\ FULL_SIMP_TAC std_ss [mw_subv_def,mw_sub2_def,LET_DEF]
+  \\ MATCH_MP_TAC LENGTH_mw_trailing_IMP \\ IMP_RES_TAC LESS_EQ_LENGTH
+  \\ POP_ASSUM (ASSUME_TAC o GSYM) \\ FULL_SIMP_TAC (srw_ss()) [
+       rich_listTheory.DROP_LENGTH_APPEND,
+       rich_listTheory.TAKE_LENGTH_APPEND]
+  \\ `?ts1 t1. mw_sub xs1 xs T = (ts1,t1)` by METIS_TAC [PAIR]
+  \\ `?ts2 t2. mw_sub xs2 (MAP (\x. 0x0w) xs2) t1 = (ts2,t2)` by METIS_TAC [PAIR]
+  \\ IMP_RES_TAC LENGTH_mw_sub \\ FULL_SIMP_TAC std_ss [LENGTH_APPEND]);
+
+val mw_add_F = store_thm("mw_add_F",
+  ``!xs2. (mw_add xs2 (MAP (\x. 0x0w) xs2) F = (xs2,F))``,
+  Induct \\ FULL_SIMP_TAC (srw_ss()) [mw_add_def,MAP,single_add_def,
+    LET_DEF,b2w_def,b2n_def,GSYM NOT_LESS,w2n_lt]);
+
+val LENGTH_mw_addv = store_thm("LENGTH_mw_addv",
+  ``LENGTH ys <= LENGTH xs ==>
+    LENGTH (mw_addv xs ys F) <= LENGTH xs + LENGTH ys``,
+  REPEAT STRIP_TAC \\ IMP_RES_TAC LESS_EQ_LENGTH
+  \\ FULL_SIMP_TAC std_ss [mw_addv_EQ_mw_add,LET_DEF]
+  \\ `?ts1 t1. mw_add xs1 ys F = (ts1,t1)` by METIS_TAC [PAIR]
+  \\ `?ts2 t2. mw_add xs2 (MAP (\x. 0x0w) xs2) t1 = (ts2,t2)` by METIS_TAC [PAIR]
+  \\ FULL_SIMP_TAC std_ss []
+  \\ Cases_on `ys` \\ FULL_SIMP_TAC std_ss [] THEN1
+   (Cases_on `xs1` \\ FULL_SIMP_TAC std_ss [LENGTH,ADD1,mw_add_def]
+    \\ Cases_on `t1` \\ FULL_SIMP_TAC std_ss [mw_add_F,LENGTH_APPEND]
+    \\ Cases_on `ts1` \\ FULL_SIMP_TAC (srw_ss()) [LENGTH])
+  \\ IMP_RES_TAC LENGTH_mw_add
+  \\ Cases_on `t2` \\ FULL_SIMP_TAC std_ss [LENGTH_APPEND,LENGTH] \\ DECIDE_TAC);
+
+val LENGTH_mw_mul_pass = store_thm("LENGTH_mw_mul_pass",
+  ``!ys zs (x:'a word) k.
+      (LENGTH (mw_mul_pass x ys zs k) = LENGTH ys + 1)``,
+  Induct \\ Cases_on `zs`
+  \\ FULL_SIMP_TAC (srw_ss()) [mw_mul_pass_def,single_mul_add_def,LET_DEF,
+       single_mul_def,mw_add_def,single_add_def] \\ DECIDE_TAC);
+
+val LENGTH_mw_mul = store_thm("LENGTH_mw_mul",
+  ``!xs ys zs.
+      (LENGTH zs = LENGTH ys) ==>
+      (LENGTH (mw_mul xs ys zs) = LENGTH xs + LENGTH ys)``,
+  Induct \\ FULL_SIMP_TAC std_ss [mw_mul_def,LENGTH,LET_DEF]
+  \\ REPEAT STRIP_TAC \\ FULL_SIMP_TAC std_ss []
+  \\ `LENGTH (mw_mul_pass h ys zs 0w) = LENGTH ys + 1` by
+       FULL_SIMP_TAC std_ss [LENGTH_mw_mul_pass]
+  \\ Cases_on `mw_mul_pass h ys zs 0x0w`
+  \\ FULL_SIMP_TAC std_ss [LENGTH,TL,ADD1] \\ DECIDE_TAC);
+
+val _ = export_theory();
