examples/machine-code/multiword/x64_multiwordScript.sml
@@ -1,0 +1,1476 @@
+
+open HolKernel Parse boolLib bossLib;
+val _ = new_theory "x64_multiword";
+
+infix \\ val op \\ = op THEN;
+open multiwordTheory;
+
+open progTheory;
+open decompilerLib x64_codegenLib prog_x64Lib x64_encodeLib x64_compilerLib;
+open wordsTheory wordsLib addressTheory arithmeticTheory listTheory pairSyntax;
+open addressTheory pairTheory set_sepTheory rich_listTheory integerTheory;
+
+val REV = Tactical.REVERSE;
+
+fun x64_decompile name asm =
+  decompile_strings x64_tools_64 name (assemble asm);
+
+fun x64_decompile_no_status name asm =
+  decompile_strings x64_tools_64_no_status name (assemble asm);
+
+(*
+
+  This file produces a single blob of x64 machine code that is able to
+  do any of the following arithmetic functions over arbitrary size
+  integer inputs.
+
+    + - * div mod < = dec
+
+  This blob of machine code takes to bignum integers as input. Each
+  bignum is represented as a pointer to the payload in memory (an
+  unsigned natural number) and a word containing the length of the
+  payload and the sign of the integer.
+
+    input 1: R13 hold pointer, R0 holds length with sign
+    input 2: R14 hold pointer, R1 holds length with sign
+
+  The name of the operation to perform is held in R2 and a pointer to
+  free space is given in R15. Output is produced where at the location
+  given in R15 and the length of this output is returned in R0 with
+  sign --- the exception is comparison which returns its full result
+  in R0.
+
+*)
+
+(*
+
+  All of the functions in this file operate over three arrays (bignum
+  payloads): two read-only that may alias and one which is the result
+  of the arithemtic operation. In order to make it easy to write
+  functions that operate over these we will provide an abstraction
+  which makes it clear that we are operating over such arrays. We
+  provide two indexes into each array.
+
+*)
+
+val array64_def = Define `
+  (array64 a [] = emp) /\
+  (array64 a (x::xs) = one (a:word64,x:word64) * array64 (a+8w) xs)`;
+
+val bignum_mem_def = Define `
+  bignum_mem p dm m xa xs ya ys za zs =
+    (xa && 7w = 0w) /\ (ya && 7w = 0w) /\ (za && 7w = 0w) /\
+    if xa = ya then
+      (xs = ys) /\ (array64 xa xs * array64 za zs * p) (fun2set (m,dm))
+    else
+      (array64 xa xs * array64 ya ys * array64 za zs * p) (fun2set (m,dm))`
+
+val zBIGNUMS_def = Define `
+  zBIGNUMS (xa,xs,ya,ys,za,zs,p) =
+    SEP_EXISTS dm m.
+      zMEMORY64 dm m * zR 13w xa * zR 14w ya * zR 15w za *
+      cond (bignum_mem p dm m xa xs ya ys za zs)`;
+
+(* read xs, ys, zs *)
+
+val LESS_LENGTH_IMP = prove(
+  ``!xs n. n < LENGTH xs ==>
+           ?ys1 ys2. (xs = ys1 ++ EL n xs :: ys2) /\ (LENGTH ys1 = n)``,
+  Induct \\ FULL_SIMP_TAC (srw_ss()) []
+  \\ Cases_on `n` \\ FULL_SIMP_TAC (srw_ss()) [LENGTH_NIL]
+  \\ REPEAT STRIP_TAC \\ RES_TAC
+  \\ Q.LIST_EXISTS_TAC [`h::ys1`,`ys2`]
+  \\ FULL_SIMP_TAC std_ss [APPEND,LENGTH] \\ METIS_TAC []);
+
+val array64_APPEND = prove(
+  ``!xs a ys.
+      array64 a (xs ++ ys) = array64 a xs * array64 (a + n2w (8 * LENGTH xs)) ys``,
+  Induct \\ FULL_SIMP_TAC (srw_ss()) [array64_def,SEP_CLAUSES,STAR_ASSOC,
+      MULT_CLAUSES,word_arith_lemma1,AC ADD_COMM ADD_ASSOC]);
+
+val ALIGNED64_IMP = prove(
+  ``(x && 7w = 0w:word64) ==> (x + 8w * w && 7w = 0w) /\
+                              (8w * w + x && 7w = 0w)``,
+  blastLib.BBLAST_TAC);
+
+val FINISH_TAC =
+  FULL_SIMP_TAC std_ss [array64_APPEND,array64_def]
+  \\ Cases_on `xa = ya` \\ FULL_SIMP_TAC std_ss [GSYM word_mul_n2w,
+        AC WORD_ADD_COMM WORD_ADD_ASSOC,GSYM w2w_def,
+        AC WORD_MULT_COMM WORD_MULT_ASSOC,w2w_id]
+  \\ SEP_R_TAC
+
+val x0 = ("r0",``0w:word4``,``r0:word64``);
+val x1 = ("r1",``1w:word4``,``r1:word64``);
+val x2 = ("r2",``2w:word4``,``r2:word64``);
+val x3 = ("r3",``3w:word4``,``r3:word64``);
+val x8 = ("r8",``8w:word4``,``r8:word64``);
+val x9 = ("r9",``9w:word4``,``r9:word64``);
+val x10 = ("r10",``10w:word4``,``r10:word64``);
+val x11 = ("r11",``11w:word4``,``r11:word64``);
+val x12 = ("r12",``12w:word4``,``r12:word64``);
+
+fun READ_XS (at,wt,rt) (a,w,r) = let
+  val ((th,_,_),_) = x64_spec_memory64 (x64_encode ("mov "^at^",[8*"^a^"+r13]"))
+  val th = SPEC_FRAME_RULE th ``zR 14w ya * zR 15w za *
+                 cond (bignum_mem p df f xa xs ya ys za zs /\
+                       w2n (^r:word64) < LENGTH xs)``
+  val th = Q.INST [`r13`|->`xa`] th
+  val (th,goal) = SPEC_WEAKEN_RULE th
+    ``let ^rt = (EL (w2n ^r) xs) in zPC (rip + 0x5w) * zR ^wt ^rt * zR ^w ^r *
+      zBIGNUMS (xa,xs,ya,ys,za,zs,p)``
+  val lemma = prove(goal,
+    FULL_SIMP_TAC (std_ss++sep_cond_ss) [zBIGNUMS_def,SEP_CLAUSES,
+      cond_STAR,SEP_IMP_def,SEP_EXISTS_THM,LET_DEF] \\ REPEAT STRIP_TAC
+    \\ Q.LIST_EXISTS_TAC [`df`,`f`] \\ FULL_SIMP_TAC std_ss []
+    \\ `f (8w * ^r + xa) = EL (w2n (^r:word64)) xs` by ALL_TAC
+    \\ FULL_SIMP_TAC (std_ss++star_ss) []
+    \\ FULL_SIMP_TAC std_ss [bignum_mem_def]
+    \\ IMP_RES_TAC LESS_LENGTH_IMP
+    \\ Q.ABBREV_TAC `y = EL (w2n (^r:word64)) xs` \\ POP_ASSUM (K ALL_TAC)
+    \\ FINISH_TAC)
+  val th = MP th lemma
+  val th = th |> Q.GEN `df` |> Q.GEN `f` |> SIMP_RULE std_ss [SPEC_PRE_EXISTS]
+  val (th,goal) = SPEC_STRENGTHEN_RULE th
+    ``zPC rip * zR ^wt ^rt * zR ^w ^r *
+      zBIGNUMS (xa,xs,ya,ys,za,zs,p) * cond (w2n ^r < LENGTH xs)``
+  val lemma = prove(goal,
+    FULL_SIMP_TAC (std_ss++sep_cond_ss) [zBIGNUMS_def,SEP_CLAUSES,
+      cond_STAR,SEP_IMP_def,SEP_EXISTS_THM] \\ REPEAT STRIP_TAC
+    \\ Q.LIST_EXISTS_TAC [`m`,`dm`] \\ FULL_SIMP_TAC (std_ss++star_ss) []
+    \\ FULL_SIMP_TAC std_ss [bignum_mem_def]
+    \\ IMP_RES_TAC ALIGNED64_IMP \\ FULL_SIMP_TAC std_ss [GSYM word_mul_n2w]
+    \\ IMP_RES_TAC LESS_LENGTH_IMP
+    \\ Q.ABBREV_TAC `y = EL (w2n (^r:word64)) xs` \\ POP_ASSUM (K ALL_TAC)
+    \\ FINISH_TAC)
+  val th = MP th lemma
+  val th = th |> INST [``rip:word64``|->``p:word64``]
+  val _ = add_compiled [SIMP_RULE std_ss [LET_DEF] th]
+  in th end;
+
+val mov_r10_xs = READ_XS x0 x10;
+val mov_r10_xs = READ_XS x8 x10;
+val mov_r11_xs = READ_XS x8 x11;
+val mov_r12_xs = READ_XS x8 x12;
+
+val _ = add_decompiled("r8_el_r10_xs",mov_r10_xs,5,SOME 5);
+
+fun READ_YS (at,wt,rt) (a,w,r) = let
+  val ((th,_,_),_) = x64_spec_memory64 (x64_encode ("mov "^at^",[8*"^a^"+r14]"))
+  val th = SPEC_FRAME_RULE th ``zR 13w xa * zR 15w za *
+                 cond (bignum_mem p df f xa xs ya ys za zs /\
+                       w2n (^r:word64) < LENGTH ys)``
+  val th = Q.INST [`r14`|->`ya`] th
+  val (th,goal) = SPEC_WEAKEN_RULE th
+    ``let ^rt = (EL (w2n ^r) ys) in zPC (rip + 0x4w) * zR ^wt ^rt * zR ^w ^r *
+      zBIGNUMS (xa,xs,ya,ys,za,zs,p)``
+  val lemma = prove(goal,
+    FULL_SIMP_TAC (std_ss++sep_cond_ss) [zBIGNUMS_def,SEP_CLAUSES,
+      cond_STAR,SEP_IMP_def,SEP_EXISTS_THM,LET_DEF] \\ REPEAT STRIP_TAC
+    \\ Q.LIST_EXISTS_TAC [`df`,`f`] \\ FULL_SIMP_TAC std_ss []
+    \\ `f (8w * ^r + ya) = EL (w2n (^r:word64)) ys` by ALL_TAC
+    \\ FULL_SIMP_TAC (std_ss++star_ss) []
+    \\ FULL_SIMP_TAC std_ss [bignum_mem_def]
+    \\ IMP_RES_TAC LESS_LENGTH_IMP
+    \\ Q.ABBREV_TAC `y = EL (w2n (^r:word64)) ys` \\ POP_ASSUM (K ALL_TAC)
+    \\ Cases_on `xs = ys` \\ FULL_SIMP_TAC std_ss []
+    \\ FINISH_TAC)
+  val th = MP th lemma
+  val th = th |> Q.GEN `df` |> Q.GEN `f` |> SIMP_RULE std_ss [SPEC_PRE_EXISTS]
+  val (th,goal) = SPEC_STRENGTHEN_RULE th
+    ``zPC rip * zR ^wt ^rt * zR ^w ^r *
+      zBIGNUMS (xa,xs,ya,ys,za,zs,p) * cond (w2n ^r < LENGTH ys)``
+  val lemma = prove(goal,
+    FULL_SIMP_TAC (std_ss++sep_cond_ss) [zBIGNUMS_def,SEP_CLAUSES,
+      cond_STAR,SEP_IMP_def,SEP_EXISTS_THM] \\ REPEAT STRIP_TAC
+    \\ Q.LIST_EXISTS_TAC [`m`,`dm`] \\ FULL_SIMP_TAC (std_ss++star_ss) []
+    \\ FULL_SIMP_TAC std_ss [bignum_mem_def]
+    \\ IMP_RES_TAC ALIGNED64_IMP \\ FULL_SIMP_TAC std_ss [GSYM word_mul_n2w]
+    \\ IMP_RES_TAC LESS_LENGTH_IMP
+    \\ Q.ABBREV_TAC `y = EL (w2n (^r:word64)) ys` \\ POP_ASSUM (K ALL_TAC)
+    \\ Cases_on `xs = ys` \\ FULL_SIMP_TAC std_ss []
+    \\ FINISH_TAC)
+  val th = MP th lemma
+  val th = th |> INST [``rip:word64``|->``p:word64``]
+  val _ = add_compiled [SIMP_RULE std_ss [LET_DEF] th]
+  in th end;
+
+val mov_r10_ys = READ_YS x2 x10;
+val mov_r11_ys = READ_YS x2 x11;
+val mov_r12_ys = READ_YS x2 x12;
+val mov_r10_ys = READ_YS x8 x10;
+val mov_r11_ys = READ_YS x8 x11;
+val mov_r12_ys = READ_YS x8 x12;
+val mov_r10_ys = READ_YS x9 x10;
+val mov_r11_ys = READ_YS x9 x11;
+val mov_r12_ys = READ_YS x9 x12;
+
+val _ = add_decompiled("r9_el_r10_ys",mov_r10_ys,4,SOME 4);
+
+fun READ_ZS (at,wt,rt) (a,w,r) = let
+  val ((th,_,_),_) = x64_spec_memory64 (x64_encode ("mov "^at^",[8*"^a^"+r15]"))
+  val th = SPEC_FRAME_RULE th ``zR 13w xa * zR 14w ya *
+                 cond (bignum_mem p df f xa xs ya ys za zs /\
+                       w2n (^r:word64) < LENGTH zs)``
+  val th = Q.INST [`r15`|->`za`] th
+  val (th,goal) = SPEC_WEAKEN_RULE th
+    ``let ^rt = (EL (w2n ^r) zs) in zPC (rip + 0x4w) * zR ^wt ^rt * zR ^w ^r *
+      zBIGNUMS (xa,xs,ya,ys,za,zs,p)``
+  val lemma = prove(goal,
+    FULL_SIMP_TAC (std_ss++sep_cond_ss) [zBIGNUMS_def,SEP_CLAUSES,
+      cond_STAR,SEP_IMP_def,SEP_EXISTS_THM,LET_DEF] \\ REPEAT STRIP_TAC
+    \\ Q.LIST_EXISTS_TAC [`df`,`f`] \\ FULL_SIMP_TAC std_ss []
+    \\ `f (8w * ^r + za) = EL (w2n (^r:word64)) zs` by ALL_TAC
+    \\ FULL_SIMP_TAC (std_ss++star_ss) []
+    \\ FULL_SIMP_TAC std_ss [bignum_mem_def]
+    \\ IMP_RES_TAC LESS_LENGTH_IMP
+    \\ Q.ABBREV_TAC `y = EL (w2n (^r:word64)) zs` \\ POP_ASSUM (K ALL_TAC)
+    \\ FINISH_TAC)
+  val th = MP th lemma
+  val th = th |> Q.GEN `df` |> Q.GEN `f` |> SIMP_RULE std_ss [SPEC_PRE_EXISTS]
+  val (th,goal) = SPEC_STRENGTHEN_RULE th
+    ``zPC rip * zR ^wt ^rt * zR ^w ^r *
+      zBIGNUMS (xa,xs,ya,ys,za,zs,p) * cond (w2n ^r < LENGTH zs)``
+  val lemma = prove(goal,
+    FULL_SIMP_TAC (std_ss++sep_cond_ss) [zBIGNUMS_def,SEP_CLAUSES,
+      cond_STAR,SEP_IMP_def,SEP_EXISTS_THM] \\ REPEAT STRIP_TAC
+    \\ Q.LIST_EXISTS_TAC [`m`,`dm`] \\ FULL_SIMP_TAC (std_ss++star_ss) []
+    \\ FULL_SIMP_TAC std_ss [bignum_mem_def]
+    \\ IMP_RES_TAC ALIGNED64_IMP \\ FULL_SIMP_TAC std_ss [GSYM word_mul_n2w]
+    \\ IMP_RES_TAC LESS_LENGTH_IMP
+    \\ Q.ABBREV_TAC `y = EL (w2n (^r:word64)) zs` \\ POP_ASSUM (K ALL_TAC)
+    \\ FINISH_TAC)
+  val th = MP th lemma
+  val th = th |> INST [``rip:word64``|->``p:word64``]
+  val _ = add_compiled [SIMP_RULE std_ss [LET_DEF] th]
+  in th end;
+
+val mov_r10_zs = READ_ZS x3 x10;
+val mov_r11_zs = READ_ZS x3 x11;
+val mov_r12_zs = READ_ZS x3 x12;
+val mov_r10_zs = READ_ZS x8 x10;
+val mov_r11_zs = READ_ZS x8 x11;
+val mov_r12_zs = READ_ZS x8 x12;
+
+val _ = add_decompiled("r8_el_r10_zs",mov_r10_zs,4,SOME 4);
+
+(* write zs *)
+
+fun WRITE_ZS (at,wt,rt) (a,w,r) = let
+  val ((th,_,_),_) = x64_spec_memory64 (x64_encode ("mov [8*"^a^"+r15],"^at))
+  val th = SPEC_FRAME_RULE th ``zR 13w xa * zR 14w ya *
+                 cond (bignum_mem p df f xa xs ya ys za zs /\
+                       w2n (^r:word64) < LENGTH zs)``
+  val th = Q.INST [`r15`|->`za`] th
+  val (th,goal) = SPEC_WEAKEN_RULE th
+    ``let zs = LUPDATE ^rt (w2n ^r) zs in
+        zPC (rip + 0x4w) * zR ^wt ^rt * zR ^w ^r *
+        zBIGNUMS (xa,xs,ya,ys,za,zs,p)``
+  val lemma = prove(goal,
+    FULL_SIMP_TAC (std_ss++sep_cond_ss) [zBIGNUMS_def,SEP_CLAUSES,
+      cond_STAR,SEP_IMP_def,SEP_EXISTS_THM,LET_DEF] \\ REPEAT STRIP_TAC
+    \\ Q.LIST_EXISTS_TAC [`df`,`(0x8w * ^r + za =+ ^rt) f`]
+    \\ FULL_SIMP_TAC (std_ss++star_ss) []
+    \\ FULL_SIMP_TAC std_ss [bignum_mem_def]
+    \\ IMP_RES_TAC LESS_LENGTH_IMP
+    \\ POP_ASSUM (ASSUME_TAC o GSYM)
+    \\ Q.ABBREV_TAC `y = EL (w2n ^r) zs` \\ POP_ASSUM (K ALL_TAC)
+    \\ FULL_SIMP_TAC std_ss [APPEND,GSYM APPEND_ASSOC,LUPDATE_LENGTH]
+    \\ FULL_SIMP_TAC std_ss [array64_APPEND,array64_def]
+    \\ `za + n2w (8 * LENGTH ys1) = 0x8w * ^r + za` by ALL_TAC THEN1
+      (Cases_on `^r` \\ FULL_SIMP_TAC (srw_ss()) [word_mul_n2w])
+    \\ FULL_SIMP_TAC std_ss []
+    \\ Cases_on `xa = ya` \\ FULL_SIMP_TAC std_ss [] \\ SEP_WRITE_TAC
+    \\ FULL_SIMP_TAC (std_ss++star_ss) [])
+  val th = MP th lemma
+  val th = th |> Q.GEN `df` |> Q.GEN `f` |> SIMP_RULE std_ss [SPEC_PRE_EXISTS]
+  val (th,goal) = SPEC_STRENGTHEN_RULE th
+    ``zPC rip * zR ^wt ^rt * zR ^w ^r *
+      zBIGNUMS (xa,xs,ya,ys,za,zs,p) * cond (w2n ^r < LENGTH zs)``
+  val lemma = prove(goal,
+    FULL_SIMP_TAC (std_ss++sep_cond_ss) [zBIGNUMS_def,SEP_CLAUSES,
+      cond_STAR,SEP_IMP_def,SEP_EXISTS_THM] \\ REPEAT STRIP_TAC
+    \\ Q.LIST_EXISTS_TAC [`m`,`dm`] \\ FULL_SIMP_TAC (std_ss++star_ss) []
+    \\ FULL_SIMP_TAC std_ss [bignum_mem_def]
+    \\ IMP_RES_TAC ALIGNED64_IMP \\ FULL_SIMP_TAC std_ss [GSYM word_mul_n2w]
+    \\ IMP_RES_TAC LESS_LENGTH_IMP
+    \\ Q.ABBREV_TAC `y = EL (w2n (^r:word64)) zs` \\ POP_ASSUM (K ALL_TAC)
+    \\ FINISH_TAC)
+  val th = MP th lemma
+  val th = th |> INST [``rip:word64``|->``p:word64``]
+  val _ = add_compiled [SIMP_RULE std_ss [LET_DEF] th]
+  in th end;
+
+val mov_zs_r10 = WRITE_ZS x0 x10;
+val mov_zs_r11 = WRITE_ZS x0 x11;
+val mov_zs_r12 = WRITE_ZS x0 x12;
+val mov_zs_r10 = WRITE_ZS x1 x10;
+val mov_zs_r11 = WRITE_ZS x1 x11;
+val mov_zs_r12 = WRITE_ZS x1 x12;
+val mov_zs_r10 = WRITE_ZS x8 x10;
+val mov_zs_r11 = WRITE_ZS x8 x11;
+val mov_zs_r12 = WRITE_ZS x8 x12;
+
+val _ = add_decompiled("lupdate_r10_zs_with_r8",mov_zs_r10,4,SOME 4);
+
+(* swap xs ys *)
+
+val SWAP_XS_YS = let
+  val ((th,_,_),_) = x64_spec_memory64 (x64_encode ("xchg r13,r14"))
+  val th = SPEC_FRAME_RULE th ``zR 15w za * zMEMORY64 df f *
+                 cond (bignum_mem p df f xa xs ya ys za zs)``
+  val th = Q.INST [`r13`|->`xa`,`r14`|->`ya`] th
+  val (th,goal) = SPEC_WEAKEN_RULE th
+    ``zPC (rip + 0x3w) * zBIGNUMS (ya,ys,xa,xs,za,zs,p)``
+  val lemma = prove(goal,
+    FULL_SIMP_TAC (std_ss++sep_cond_ss) [zBIGNUMS_def,SEP_CLAUSES,
+      cond_STAR,SEP_IMP_def,SEP_EXISTS_THM,LET_DEF] \\ REPEAT STRIP_TAC
+    \\ Q.LIST_EXISTS_TAC [`df`,`f`]
+    \\ FULL_SIMP_TAC (std_ss++star_ss) []
+    \\ FULL_SIMP_TAC std_ss [bignum_mem_def]
+    \\ SRW_TAC [] [] \\ FULL_SIMP_TAC (std_ss++star_ss) []);
+  val th = MP th lemma
+  val th = th |> Q.GEN `df` |> Q.GEN `f` |> SIMP_RULE std_ss [SPEC_PRE_EXISTS]
+  val (th,goal) = SPEC_STRENGTHEN_RULE th
+    ``zPC rip * zBIGNUMS (xa,xs,ya,ys,za,zs,p)``
+  val lemma = prove(goal,
+    FULL_SIMP_TAC (std_ss++sep_cond_ss) [zBIGNUMS_def,SEP_CLAUSES,
+      cond_STAR,SEP_IMP_def,SEP_EXISTS_THM] \\ REPEAT STRIP_TAC
+    \\ Q.LIST_EXISTS_TAC [`m`,`dm`] \\ FULL_SIMP_TAC (std_ss++star_ss) [])
+  val th = MP th lemma
+  val th = th |> INST [``rip:word64``|->``p:word64``]
+  val _ = add_compiled [SIMP_RULE std_ss [LET_DEF] th]
+  in th end;
+
+val _ = print_compiler_grammar ();
+
+(* compare *)
+
+val (res,x64_cmp_def,x64_cmp_pre_def) = x64_compile `
+  x64_cmp (r10:word64,xs:word64 list,ys:word64 list) =
+    if r10 = 0w then (r10,xs,ys) else
+      let r10 = r10 - 1w in
+      let r8 = EL (w2n r10) xs in
+      let r9 = EL (w2n r10) ys in
+        if r8 = r9 then
+          x64_cmp (r10,xs,ys)
+        else if r8 <+ r9 then let r10 = 1w in (r10,xs,ys)
+                         else let r10 = 2w in (r10,xs,ys)`
+
+val (res,x64_compare_def,x64_compare_pre_def) = x64_compile `
+  x64_compare (r10:word64,r11,xs:word64 list,ys:word64 list) =
+    if r10 <+ r11 then let r10 = 1w in (r10,xs,ys) else
+    if r11 <+ r10 then let r10 = 2w in (r10,xs,ys) else
+      let (r10,xs,ys) = x64_cmp (r10,xs,ys) in
+        (r10,xs,ys)`
+
+val x64_header_def = Define `
+  x64_header (s,xs:word64 list) = n2w (LENGTH xs * 2) + if s then 1w else 0w:word64`;
+
+val (res,x64_icompare_def,x64_icompare_pre_def) = x64_compile `
+  x64_icompare (r10:word64,r11,xs:word64 list,ys:word64 list) =
+    if r10 && 1w = 0w then
+      if ~(r11 && 1w = 0w) then let r10 = 2w in (r10,xs,ys) else
+        let r10 = r10 >>> 1 in
+        let r11 = r11 >>> 1 in
+        let (r10,xs,ys) = x64_compare (r10,r11,xs,ys) in
+          (r10,xs,ys)
+    else
+      if r11 && 1w = 0w then let r10 = 1w in (r10,xs,ys) else
+        let r10 = r10 >>> 1 in
+        let r11 = r11 >>> 1 in
+        let (r10,xs,ys) = x64_compare (r10,r11,xs,ys) in
+          if r10 = 0w then (r10,xs,ys) else
+            let r10 = r10 ?? 3w in (r10,xs,ys)`
+
+val cmp2w_def = Define `
+  (cmp2w NONE = 0w:word64) /\
+  (cmp2w (SOME T) = 1w) /\
+  (cmp2w (SOME F) = 2w)`;
+
+val x64_cmp_thm = prove(
+  ``!xs ys xs1 ys1.
+      (LENGTH ys = LENGTH xs) /\ LENGTH xs < dimword(:64) ==>
+      x64_cmp_pre (n2w (LENGTH xs),xs++xs1,ys++ys1) /\
+      (x64_cmp (n2w (LENGTH xs),xs++xs1,ys++ys1) =
+       (cmp2w (mw_cmp xs ys),xs++xs1,ys++ys1))``,
+  HO_MATCH_MP_TAC SNOC_INDUCT \\ FULL_SIMP_TAC std_ss [LENGTH,LENGTH_NIL]
+  \\ STRIP_TAC THEN1
+   (REPEAT STRIP_TAC \\ ONCE_REWRITE_TAC [x64_cmp_def,Once x64_cmp_pre_def]
+    \\ FULL_SIMP_TAC std_ss [Once mw_cmp_def,cmp2w_def,APPEND])
+  \\ NTAC 7 STRIP_TAC
+  \\ `(ys = []) \/ ?y ys2. ys = SNOC y ys2` by METIS_TAC [SNOC_CASES]
+  \\ FULL_SIMP_TAC (srw_ss()) [] \\ FULL_SIMP_TAC std_ss [GSYM SNOC_APPEND,ADD1]
+  \\ `LENGTH xs < dimword (:64)` by (FULL_SIMP_TAC (srw_ss()) [] \\ DECIDE_TAC)
+  \\ RES_TAC \\ ONCE_REWRITE_TAC [x64_cmp_def,x64_cmp_pre_def]
+  \\ SIMP_TAC std_ss [GSYM word_add_n2w,WORD_ADD_SUB]
+  \\ FULL_SIMP_TAC (srw_ss()) [n2w_11,word_add_n2w,LET_DEF]
+  \\ FULL_SIMP_TAC std_ss [SNOC_APPEND,GSYM APPEND_ASSOC,APPEND]
+  \\ STRIP_TAC THEN1 DECIDE_TAC
+  \\ FULL_SIMP_TAC (srw_ss()) [rich_listTheory.EL_LENGTH_APPEND]
+  \\ Q.PAT_ASSUM `LENGTH ys2 = LENGTH xs` (ASSUME_TAC o GSYM)
+  \\ FULL_SIMP_TAC (srw_ss()) [rich_listTheory.EL_LENGTH_APPEND]
+  \\ ONCE_REWRITE_TAC [EQ_SYM_EQ]
+  \\ SIMP_TAC std_ss [Once mw_cmp_def]
+  \\ FULL_SIMP_TAC (srw_ss()) []
+  \\ FULL_SIMP_TAC std_ss [GSYM SNOC_APPEND,FRONT_SNOC]
+  \\ SRW_TAC [] [cmp2w_def])
+  |> Q.SPECL [`xs`,`ys`,`[]`,`[]`]
+  |> SIMP_RULE std_ss [APPEND_NIL];
+
+val x64_compare_thm = prove(
+  ``LENGTH xs < dimword (:64) /\ LENGTH ys < dimword (:64) ==>
+    x64_compare_pre (n2w (LENGTH xs),n2w (LENGTH ys),xs,ys) /\
+    (x64_compare (n2w (LENGTH xs),n2w (LENGTH ys),xs,ys) =
+     (cmp2w (mw_compare xs ys),xs,ys))``,
+  SIMP_TAC (srw_ss()) [x64_compare_def,x64_compare_pre_def,
+    n2w_11,WORD_LO,LET_DEF,mw_compare_def] \\ SRW_TAC [] [cmp2w_def]
+  \\ `LENGTH xs = LENGTH ys` by DECIDE_TAC
+  \\ MP_TAC x64_cmp_thm \\ FULL_SIMP_TAC (srw_ss()) []);
+
+val x64_header_sign = prove(
+  ``(x64_header (s,xs) && 1w = 0w) = ~s``,
+  SIMP_TAC std_ss [x64_header_def,GSYM word_mul_n2w]
+  \\ Q.SPEC_TAC (`n2w (LENGTH xs)`,`w`) \\ Cases_on `s`
+  \\ FULL_SIMP_TAC std_ss [] \\ blastLib.BBLAST_TAC);
+
+val x64_length_lemma = prove(
+  ``(w * 2w + if s then 0x1w else 0x0w) >>> 1 = (w * 2w:word64) >>> 1``,
+  Cases_on `s` \\ FULL_SIMP_TAC std_ss [] \\ blastLib.BBLAST_TAC);
+
+val x64_length = prove(
+  ``LENGTH xs < dimword (:63) ==>
+    (x64_header (s,xs) >>> 1 = n2w (LENGTH xs))``,
+  FULL_SIMP_TAC std_ss [x64_header_def,GSYM word_mul_n2w,x64_length_lemma]
+  \\ SIMP_TAC std_ss [GSYM w2n_11,w2n_lsr,w2n_n2w,word_mul_n2w]
+  \\ FULL_SIMP_TAC (srw_ss()) [] \\ REPEAT STRIP_TAC
+  \\ `(LENGTH xs * 2) < 18446744073709551616` by DECIDE_TAC
+  \\ `LENGTH xs < 18446744073709551616` by DECIDE_TAC
+  \\ FULL_SIMP_TAC (srw_ss()) [MULT_DIV]);
+
+val dim63_IMP_dim64 = prove(
+  ``n < dimword (:63) ==> n < dimword (:64)``,
+  FULL_SIMP_TAC (srw_ss()) [] \\ DECIDE_TAC);
+
+val x64_icompare_thm = prove(
+  ``LENGTH xs < dimword (:63) /\ LENGTH ys < dimword (:63) ==>
+    x64_icompare_pre (x64_header (s,xs),x64_header (t,ys),xs,ys) /\
+    (x64_icompare (x64_header (s,xs),x64_header (t,ys),xs,ys) =
+     (cmp2w (mwi_compare (s,xs) (t,ys)),xs,ys))``,
+  FULL_SIMP_TAC std_ss [x64_icompare_def,x64_icompare_pre_def,x64_header_sign,
+    x64_length,LET_DEF] \\ STRIP_TAC \\ IMP_RES_TAC dim63_IMP_dim64
+  \\ FULL_SIMP_TAC std_ss [x64_compare_thm,mwi_compare_def]
+  \\ Cases_on `s` \\ Cases_on `t` \\ FULL_SIMP_TAC std_ss [cmp2w_def]
+  \\ Cases_on `mw_compare xs ys` \\ FULL_SIMP_TAC std_ss [cmp2w_def,option_eq_def]
+  \\ Cases_on `x` \\ FULL_SIMP_TAC (srw_ss()) [cmp2w_def,option_eq_def,n2w_11]);
+
+(* addition *)
+
+val (res,x64_add_loop_def) = x64_decompile_no_status "x64_add_loop" `
+      inc r1
+      inc r2
+      add r1,0
+      jmp L2
+  L1: insert r8_el_r10_xs
+      insert r9_el_r10_ys
+      adc r8,r9
+      insert lupdate_r10_zs_with_r8
+      lea r10,[r10+1]
+  L2: loop L1
+      mov r1,r2
+      mov r9,0
+      jmp L4
+  L3: insert r8_el_r10_xs
+      adc r8,r9
+      insert lupdate_r10_zs_with_r8
+      lea r10,[r10+1]
+  L4: loop L3
+      jnb L5
+      mov r8,1
+      insert lupdate_r10_zs_with_r8
+      lea r10,[r10+1]
+  L5:`
+
+val (x64_add_res,x64_add_def) = x64_decompile "x64_add" `
+  sub r2,r1
+  insert x64_add_loop`;
+
+val _ = add_compiled [x64_add_res]
+
+val SNOC_INTRO = prove(
+  ``xs1 ++ x::(xs ++ xs2) = SNOC x xs1 ++ (xs ++ xs2)``,
+  FULL_SIMP_TAC std_ss [SNOC_APPEND,GSYM APPEND_ASSOC,APPEND]);
+
+val LUPDATE_SNOC = prove(
+  ``(LENGTH zs1 = LENGTH xs1) ==>
+    (LUPDATE x (LENGTH xs1) (SNOC y zs1 ++ (t ++ zs2)) =
+     (SNOC x zs1 ++ (t ++ zs2)))``,
+  ONCE_REWRITE_TAC [EQ_SYM_EQ]
+  \\ FULL_SIMP_TAC std_ss [SNOC_APPEND,GSYM APPEND_ASSOC,APPEND,LUPDATE_LENGTH]);
+
+val bool2num_thm = prove(``!b. bool2num b = b2n b``,Cases \\ EVAL_TAC)
+
+val x64_add_loop1_thm = prove(
+  ``!xs ys zs xs1 ys1 zs1 xs2 ys2 zs2
+     z_af z_of c z_pf z_sf z_zf r8 r9.
+      (LENGTH ys1 = LENGTH xs1) /\ (LENGTH zs1 = LENGTH xs1) /\
+      (LENGTH ys = LENGTH xs) /\ (LENGTH zs = LENGTH xs) /\
+      LENGTH (xs1 ++ xs) + 1 < 18446744073709551616 ==>
+      ?r8' r9' z_af' z_of' z_pf' z_sf' z_zf'.
+        x64_add_loop1_pre (n2w (LENGTH xs + 1),r8,r9,n2w (LENGTH xs1),
+          xs1 ++ xs ++ xs2, ys1 ++ ys ++ ys2,z_af,SOME c,
+          z_of,z_pf,z_sf,z_zf,zs1 ++ zs ++ zs2) /\
+        (x64_add_loop1 (n2w (LENGTH xs + 1),r8,r9,n2w (LENGTH xs1),
+          xs1 ++ xs ++ xs2, ys1 ++ ys ++ ys2,z_af,SOME c,
+          z_of,z_pf,z_sf,z_zf,zs1 ++ zs ++ zs2) =
+          (0w,r8',r9',n2w (LENGTH (xs1++xs)),xs1 ++ xs ++ xs2,ys1 ++ ys ++ ys2,z_af',
+             SOME (SND (mw_add xs ys c)),z_of',z_pf',z_sf',z_zf',
+                        zs1 ++ FST (mw_add xs ys c) ++ zs2))``,
+  Induct THEN1
+   (FULL_SIMP_TAC (srw_ss()) [LENGTH,LENGTH_NIL,mw_add_def]
+    \\ ONCE_REWRITE_TAC [x64_add_loop_def]
+    \\ FULL_SIMP_TAC (srw_ss()) [LENGTH,LENGTH_NIL,mw_add_def,LET_DEF])
+  \\ Cases_on `ys` \\ FULL_SIMP_TAC std_ss [LENGTH,ADD1]
+  \\ ONCE_REWRITE_TAC [x64_add_loop_def]
+  \\ FULL_SIMP_TAC (srw_ss()) [LET_DEF]
+  \\ REPEAT STRIP_TAC
+  \\ `LENGTH xs < 18446744073709551616 /\
+      LENGTH xs + 1 < 18446744073709551616 /\
+      LENGTH xs + 1 + 1 < 18446744073709551616` by DECIDE_TAC
+  \\ `LENGTH xs1 < 18446744073709551616 /\
+      LENGTH xs1 + 1 < 18446744073709551616` by DECIDE_TAC
+  \\ FULL_SIMP_TAC std_ss []
+  \\ FULL_SIMP_TAC std_ss [GSYM APPEND_ASSOC,APPEND,
+        rich_listTheory.EL_LENGTH_APPEND,NULL_DEF,HD,TL]
+  \\ Q.PAT_ASSUM `LENGTH ys1 = LENGTH xs1` (ASSUME_TAC o GSYM)
+  \\ FULL_SIMP_TAC std_ss [GSYM APPEND_ASSOC,APPEND,
+        rich_listTheory.EL_LENGTH_APPEND,NULL_DEF,HD,TL]
+  \\ SIMP_TAC std_ss [GSYM word_sub_def,GSYM word_add_n2w,WORD_ADD_SUB]
+  \\ SIMP_TAC std_ss [word_add_n2w]
+  \\ Cases_on `zs` \\ FULL_SIMP_TAC std_ss [LENGTH,ADD1,APPEND]
+  \\ SIMP_TAC std_ss [SNOC_INTRO]
+  \\ POP_ASSUM (ASSUME_TAC o GSYM) \\ FULL_SIMP_TAC std_ss []
+  \\ `LENGTH xs1 + 1 = LENGTH (SNOC h' xs1)` by
+    FULL_SIMP_TAC std_ss [LENGTH_SNOC,ADD1] \\ ASM_SIMP_TAC std_ss []
+  \\ ASM_SIMP_TAC std_ss [LUPDATE_SNOC]
+  \\ SEP_I_TAC "x64_add_loop1" \\ POP_ASSUM MP_TAC
+  \\ MATCH_MP_TAC IMP_IMP \\ STRIP_TAC
+  THEN1 (FULL_SIMP_TAC (srw_ss()) [] \\ DECIDE_TAC)
+  \\ STRIP_TAC \\ ASM_SIMP_TAC std_ss []
+  \\ FULL_SIMP_TAC (srw_ss()) [LENGTH_SNOC,ADD1,AC ADD_COMM ADD_ASSOC,mw_add_def,
+       LET_DEF,single_add_def,bool2num_thm]
+  \\ CONV_TAC (DEPTH_CONV PairRules.PBETA_CONV)
+  \\ FULL_SIMP_TAC (srw_ss()) [b2w_def] \\ DECIDE_TAC)
+
+val x64_add_loop2_thm = prove(
+  ``!xs zs xs1 zs1 xs2 zs2
+     z_af z_of c z_pf z_sf z_zf r8.
+      (LENGTH zs1 = LENGTH xs1) /\ (LENGTH zs = LENGTH xs) /\
+      LENGTH (xs1 ++ xs) + 1 < 18446744073709551616 ==>
+      ?r8' r9' z_af' z_of' z_pf' z_sf' z_zf'.
+        x64_add_loop2_pre (n2w (LENGTH xs + 1),r8,0w,n2w (LENGTH xs1),
+          xs1 ++ xs ++ xs2,z_af,SOME c,
+          z_of,z_pf,z_sf,z_zf,zs1 ++ zs ++ zs2) /\
+        (x64_add_loop2 (n2w (LENGTH xs + 1),r8,0w,n2w (LENGTH xs1),
+          xs1 ++ xs ++ xs2,z_af,SOME c,
+          z_of,z_pf,z_sf,z_zf,zs1 ++ zs ++ zs2) =
+          (0w,r8',r9',n2w (LENGTH (xs1++xs)),xs1 ++ xs ++ xs2,z_af',
+             SOME (SND (mw_add xs (MAP (\x.0w) xs) c)),z_of',z_pf',z_sf',z_zf',
+                        zs1 ++ FST (mw_add xs (MAP (\x.0w) xs) c) ++ zs2))``,
+  Induct THEN1
+   (FULL_SIMP_TAC (srw_ss()) [LENGTH,LENGTH_NIL,mw_add_def]
+    \\ ONCE_REWRITE_TAC [x64_add_loop_def]
+    \\ FULL_SIMP_TAC (srw_ss()) [LENGTH,LENGTH_NIL,mw_add_def,LET_DEF])
+  \\ FULL_SIMP_TAC std_ss [LENGTH,ADD1]
+  \\ ONCE_REWRITE_TAC [x64_add_loop_def]
+  \\ FULL_SIMP_TAC (srw_ss()) [LET_DEF]
+  \\ REPEAT STRIP_TAC
+  \\ `LENGTH xs < 18446744073709551616 /\
+      LENGTH xs + 1 < 18446744073709551616 /\
+      LENGTH xs + 1 + 1 < 18446744073709551616` by DECIDE_TAC
+  \\ `LENGTH xs1 < 18446744073709551616 /\
+      LENGTH xs1 + 1 < 18446744073709551616` by DECIDE_TAC
+  \\ FULL_SIMP_TAC std_ss []
+  \\ FULL_SIMP_TAC std_ss [GSYM APPEND_ASSOC,APPEND,
+        rich_listTheory.EL_LENGTH_APPEND,NULL_DEF,HD,TL]
+  \\ SIMP_TAC std_ss [GSYM word_sub_def,GSYM word_add_n2w,WORD_ADD_SUB]
+  \\ SIMP_TAC std_ss [word_add_n2w]
+  \\ Cases_on `zs` \\ FULL_SIMP_TAC std_ss [LENGTH,ADD1,APPEND]
+  \\ SIMP_TAC std_ss [SNOC_INTRO]
+  \\ POP_ASSUM (ASSUME_TAC o GSYM) \\ FULL_SIMP_TAC std_ss []
+  \\ `LENGTH xs1 + 1 = LENGTH (SNOC h xs1)` by
+    FULL_SIMP_TAC std_ss [LENGTH_SNOC,ADD1] \\ ASM_SIMP_TAC std_ss []
+  \\ ASM_SIMP_TAC std_ss [LUPDATE_SNOC]
+  \\ SEP_I_TAC "x64_add_loop2" \\ POP_ASSUM MP_TAC
+  \\ MATCH_MP_TAC IMP_IMP \\ STRIP_TAC
+  THEN1 (FULL_SIMP_TAC (srw_ss()) [] \\ DECIDE_TAC)
+  \\ STRIP_TAC \\ ASM_SIMP_TAC std_ss []
+  \\ FULL_SIMP_TAC (srw_ss()) [LENGTH_SNOC,ADD1,AC ADD_COMM ADD_ASSOC,mw_add_def,
+       LET_DEF,single_add_def,bool2num_thm]
+  \\ CONV_TAC (DEPTH_CONV PairRules.PBETA_CONV)
+  \\ FULL_SIMP_TAC (srw_ss()) [b2w_def]
+  \\ DECIDE_TAC)
+
+val x64_add_thm = prove(
+  ``!xs ys zs zs2.
+      LENGTH ys <= LENGTH xs /\ (LENGTH zs = LENGTH (mw_addv xs ys F)) /\
+      LENGTH xs + 1 < 18446744073709551616 ==>
+      ?r1' r2' r8' r9' r10'.
+        x64_add_pre (n2w (LENGTH ys),n2w (LENGTH xs),0w,0w,0w,xs,ys,zs++zs2) /\
+        (x64_add (n2w (LENGTH ys),n2w (LENGTH xs),0w,0w,0w,xs,ys,zs++zs2) =
+          (r1',r2',r8',r9',n2w (LENGTH (mw_addv xs ys F)),xs,ys,mw_addv xs ys F ++ zs2))``,
+  REPEAT STRIP_TAC \\ IMP_RES_TAC LESS_EQ_LENGTH
+  \\ FULL_SIMP_TAC std_ss [LENGTH_APPEND,x64_add_def,LET_DEF]
+  \\ ONCE_REWRITE_TAC [ADD_COMM]
+  \\ SIMP_TAC std_ss [GSYM word_add_n2w,WORD_ADD_SUB]
+  \\ ONCE_REWRITE_TAC [x64_add_loop_def]
+  \\ SIMP_TAC (srw_ss()) [LET_DEF,w2n_n2w,word_add_n2w]
+  \\ `~((18446744073709551616 <= (LENGTH ys + 1) MOD 18446744073709551616))` by ALL_TAC
+  THEN1 (FULL_SIMP_TAC std_ss [DECIDE ``~(n <= m) = m < n:num``])
+  \\ FULL_SIMP_TAC std_ss []
+  \\ (x64_add_loop1_thm |> Q.SPECL [`xs1`,`ys`,`zs`,`[]`,`[]`,`[]`,`xs2`,`[]`,`zs2`]
+      |> GEN_ALL |> MP_TAC)
+  \\ FULL_SIMP_TAC std_ss [LENGTH,APPEND,APPEND_NIL] \\ STRIP_TAC
+  \\ Q.PAT_ASSUM `LENGTH xs1 = LENGTH ys` (ASSUME_TAC o GSYM)
+  \\ FULL_SIMP_TAC std_ss [mw_addv_EQ_mw_add,LET_DEF]
+  \\ `?qs1 c1. mw_add xs1 ys F = (qs1,c1)` by METIS_TAC [PAIR]
+  \\ `?qs2 c2. mw_add xs2 (MAP (\x.0w) xs2) c1 = (qs2,c2)` by METIS_TAC [PAIR]
+  \\ FULL_SIMP_TAC std_ss []
+  \\ Q.ABBREV_TAC `qs3 = if c2 then [0x1w] else []:word64 list`
+  \\ `?zs1 zs3 zs4. (zs = zs1 ++ zs3 ++ zs4) /\
+        (LENGTH zs1 = LENGTH xs1) /\
+        (LENGTH zs3 = LENGTH xs2) /\
+        (LENGTH zs4 = LENGTH qs3)` by ALL_TAC THEN1
+   (IMP_RES_TAC LENGTH_mw_add
+    \\ `LENGTH xs1 <= LENGTH zs` by ALL_TAC THEN1
+          (FULL_SIMP_TAC std_ss [LENGTH_APPEND] \\ DECIDE_TAC)
+    \\ IMP_RES_TAC LESS_EQ_LENGTH \\ FULL_SIMP_TAC std_ss []
+    \\ Q.EXISTS_TAC `xs1'` \\ FULL_SIMP_TAC std_ss [LENGTH_APPEND]
+    \\ `LENGTH xs2 <= LENGTH xs2'` by ALL_TAC THEN1
+          (FULL_SIMP_TAC std_ss [LENGTH_APPEND] \\ DECIDE_TAC)
+    \\ IMP_RES_TAC LESS_EQ_LENGTH \\ FULL_SIMP_TAC std_ss []
+    \\ Q.LIST_EXISTS_TAC [`xs1''`,`xs2''`]
+    \\ FULL_SIMP_TAC std_ss [APPEND_ASSOC,LENGTH_APPEND]
+    \\ DECIDE_TAC)
+  \\ FULL_SIMP_TAC std_ss [GSYM APPEND_ASSOC]
+  \\ SEP_I_TAC "x64_add_loop1" \\ POP_ASSUM MP_TAC
+  \\ MATCH_MP_TAC IMP_IMP \\ STRIP_TAC
+  THEN1 (FULL_SIMP_TAC (srw_ss()) [] \\ DECIDE_TAC)
+  \\ STRIP_TAC \\ ASM_SIMP_TAC std_ss []
+  \\ (x64_add_loop2_thm |> Q.SPECL [`xs`,`ys`,`xs1`,`zs1`,`[]`] |> GEN_ALL
+       |> SIMP_RULE std_ss [GSYM APPEND_ASSOC,APPEND_NIL] |> ASSUME_TAC)
+  \\ SEP_I_TAC "x64_add_loop2" \\ POP_ASSUM MP_TAC
+  \\ MATCH_MP_TAC IMP_IMP \\ STRIP_TAC
+  THEN1 (IMP_RES_TAC LENGTH_mw_add \\ FULL_SIMP_TAC (srw_ss()) [] \\ DECIDE_TAC)
+  \\ STRIP_TAC \\ ASM_SIMP_TAC std_ss []
+  \\ REV (Cases_on `c2`) \\ FULL_SIMP_TAC std_ss []
+  THEN1 (Q.UNABBREV_TAC `qs3`
+         \\ FULL_SIMP_TAC std_ss [LENGTH,LENGTH_NIL,APPEND_NIL,LENGTH_APPEND])
+  \\ `LENGTH xs1 + LENGTH xs2 < 18446744073709551616` by DECIDE_TAC
+  \\ FULL_SIMP_TAC (srw_ss()) []
+  \\ IMP_RES_TAC LENGTH_mw_add
+  \\ Q.UNABBREV_TAC `qs3` \\ FULL_SIMP_TAC std_ss [LENGTH]
+  \\ STRIP_TAC THEN1 DECIDE_TAC
+  \\ Cases_on `zs4` \\ FULL_SIMP_TAC std_ss [LENGTH]
+  \\ Cases_on `t` \\ FULL_SIMP_TAC std_ss [LENGTH,ADD1]
+  \\ FULL_SIMP_TAC std_ss [GSYM APPEND_ASSOC,APPEND,word_add_n2w,ADD_ASSOC]
+  \\ FULL_SIMP_TAC std_ss [APPEND_ASSOC,GSYM LENGTH_APPEND,LUPDATE_LENGTH]);
+
+(* subtraction *)
+
+val (res,x64_sub_loop_def) = x64_decompile_no_status "x64_sub_loop" `
+      inc r1
+      inc r2
+      sub r8,0
+      jmp L2
+  L1: insert r8_el_r10_xs
+      insert r9_el_r10_ys
+      sbb r8,r9
+      insert lupdate_r10_zs_with_r8
+      lea r10,[r10+1]
+  L2: loop L1
+      mov r1,r2
+      mov r9,0
+      jmp L4
+  L3: insert r8_el_r10_xs
+      sbb r8,r9
+      insert lupdate_r10_zs_with_r8
+      lea r10,[r10+1]
+  L4: loop L3`
+
+val (x64_trailing_res,x64_trailing_def) = x64_decompile "x64_trailing" `
+  L1: test r10,r10
+      je L2
+      dec r10
+      insert r8_el_r10_zs
+      test r8,r8
+      je L1
+      inc r10
+  L2: `
+
+val _ = add_compiled [x64_trailing_res];
+
+val (x64_sub_res,x64_sub_def) = x64_decompile "x64_sub" `
+      sub r2,r1
+      insert x64_sub_loop
+      insert x64_trailing`
+
+val _ = add_compiled [x64_sub_res]
+
+val REPLICATE_SNOC = prove(
+  ``!n x. REPLICATE (SUC n) x = SNOC x (REPLICATE n x)``,
+  Induct \\ FULL_SIMP_TAC (srw_ss()) [REPLICATE]);
+
+val x64_trailing_thm = prove(
+  ``!zs zs1 r8.
+      LENGTH zs < dimword(:64) ==>
+      ?r8'.
+        x64_trailing_pre (r8,n2w (LENGTH zs),zs++zs1) /\
+        (x64_trailing (r8,n2w (LENGTH zs),zs++zs1) =
+         (r8',n2w (LENGTH (mw_trailing zs)),
+          mw_trailing zs ++ REPLICATE (LENGTH zs - LENGTH (mw_trailing zs)) 0w ++ zs1))``,
+  HO_MATCH_MP_TAC SNOC_INDUCT \\ FULL_SIMP_TAC std_ss [LENGTH,LENGTH_NIL]
+  \\ REPEAT STRIP_TAC \\ ONCE_REWRITE_TAC [x64_trailing_def,mw_trailing_def]
+  \\ FULL_SIMP_TAC (srw_ss()) [rich_listTheory.REPLICATE,LET_DEF]
+  \\ FULL_SIMP_TAC std_ss [GSYM word_add_n2w,ADD1,GSYM word_sub_def,WORD_ADD_SUB]
+  \\ IMP_RES_TAC (DECIDE ``n + 1 < k ==> n < k:num``)
+  \\ FULL_SIMP_TAC (srw_ss()) [w2n_n2w]
+  \\ FULL_SIMP_TAC std_ss [SNOC_APPEND,GSYM APPEND_ASSOC,APPEND,
+       rich_listTheory.EL_LENGTH_APPEND,NULL,HD]
+  \\ REV (Cases_on `x = 0w`) \\ FULL_SIMP_TAC std_ss [] THEN1
+   (FULL_SIMP_TAC std_ss [LENGTH_APPEND,LENGTH,REPLICATE,APPEND,
+      GSYM APPEND_ASSOC,word_add_n2w] \\ DECIDE_TAC)
+  \\ SEP_I_TAC "x64_trailing" \\ FULL_SIMP_TAC std_ss []
+  \\ STRIP_TAC THEN1 DECIDE_TAC \\ AP_TERM_TAC
+  \\ `LENGTH (mw_trailing zs) <= LENGTH zs` by
+      FULL_SIMP_TAC std_ss [LENGTH_mw_trailing]
+  \\ `LENGTH zs + 1 - LENGTH (mw_trailing zs) =
+        SUC (LENGTH zs - LENGTH (mw_trailing zs))` by DECIDE_TAC
+  \\ FULL_SIMP_TAC std_ss [REPLICATE_SNOC]
+  \\ FULL_SIMP_TAC std_ss [SNOC_APPEND,GSYM APPEND_ASSOC,APPEND])
+
+val sub_borrow_lemma = prove(
+  ``!h:word64 h':word64 c.
+     (18446744073709551616 <= b2n ~c + (w2n h' + w2n (~h))) =
+      ~(w2n h' < b2n c + w2n h)``,
+  Cases \\ Cases \\ Cases
+  \\ `(18446744073709551615 - n) < 18446744073709551616` by DECIDE_TAC
+  \\ FULL_SIMP_TAC (srw_ss()) [b2n_def,word_1comp_n2w] \\ DECIDE_TAC);
+
+val x64_sub_loop1_thm = prove(
+  ``!xs ys zs xs1 ys1 zs1 xs2 ys2 zs2
+     z_af z_of c z_pf z_sf z_zf r8 r9.
+      (LENGTH ys1 = LENGTH xs1) /\ (LENGTH zs1 = LENGTH xs1) /\
+      (LENGTH ys = LENGTH xs) /\ (LENGTH zs = LENGTH xs) /\
+      LENGTH (xs1 ++ xs) + 1 < 18446744073709551616 ==>
+      ?r8' r9' z_af' z_of' z_pf' z_sf' z_zf'.
+        x64_sub_loop1_pre (n2w (LENGTH xs + 1),r8,r9,n2w (LENGTH xs1),
+          xs1 ++ xs ++ xs2, ys1 ++ ys ++ ys2,z_af,SOME c,
+          z_of,z_pf,z_sf,z_zf,zs1 ++ zs ++ zs2) /\
+        (x64_sub_loop1 (n2w (LENGTH xs + 1),r8,r9,n2w (LENGTH xs1),
+          xs1 ++ xs ++ xs2, ys1 ++ ys ++ ys2,z_af,SOME c,
+          z_of,z_pf,z_sf,z_zf,zs1 ++ zs ++ zs2) =
+          (0w,r8',r9',n2w (LENGTH (xs1++xs)),xs1 ++ xs ++ xs2,ys1 ++ ys ++ ys2,z_af',
+             SOME (~SND (mw_sub xs ys ~c)),z_of',z_pf',z_sf',z_zf',
+                        zs1 ++ FST (mw_sub xs ys ~c) ++ zs2))``,
+  Induct THEN1
+   (FULL_SIMP_TAC (srw_ss()) [LENGTH,LENGTH_NIL,mw_sub_def]
+    \\ ONCE_REWRITE_TAC [x64_sub_loop_def]
+    \\ FULL_SIMP_TAC (srw_ss()) [LENGTH,LENGTH_NIL,mw_sub_def,LET_DEF])
+  \\ Cases_on `ys` \\ FULL_SIMP_TAC std_ss [LENGTH,ADD1]
+  \\ ONCE_REWRITE_TAC [x64_sub_loop_def]
+  \\ FULL_SIMP_TAC (srw_ss()) [LET_DEF]
+  \\ REPEAT STRIP_TAC
+  \\ `LENGTH xs < 18446744073709551616 /\
+      LENGTH xs + 1 < 18446744073709551616 /\
+      LENGTH xs + 1 + 1 < 18446744073709551616` by DECIDE_TAC
+  \\ `LENGTH xs1 < 18446744073709551616 /\
+      LENGTH xs1 + 1 < 18446744073709551616` by DECIDE_TAC
+  \\ FULL_SIMP_TAC std_ss []
+  \\ FULL_SIMP_TAC std_ss [GSYM APPEND_ASSOC,APPEND,
+        rich_listTheory.EL_LENGTH_APPEND,NULL_DEF,HD,TL]
+  \\ Q.PAT_ASSUM `LENGTH ys1 = LENGTH xs1` (ASSUME_TAC o GSYM)
+  \\ FULL_SIMP_TAC std_ss [GSYM APPEND_ASSOC,APPEND,
+        rich_listTheory.EL_LENGTH_APPEND,NULL_DEF,HD,TL]
+  \\ SIMP_TAC std_ss [GSYM word_sub_def,GSYM word_add_n2w,WORD_ADD_SUB]
+  \\ SIMP_TAC std_ss [word_add_n2w]
+  \\ Cases_on `zs` \\ FULL_SIMP_TAC std_ss [LENGTH,ADD1,APPEND]
+  \\ SIMP_TAC std_ss [SNOC_INTRO]
+  \\ POP_ASSUM (ASSUME_TAC o GSYM) \\ FULL_SIMP_TAC std_ss []
+  \\ `LENGTH xs1 + 1 = LENGTH (SNOC h' xs1)` by
+    FULL_SIMP_TAC std_ss [LENGTH_SNOC,ADD1] \\ ASM_SIMP_TAC std_ss []
+  \\ ASM_SIMP_TAC std_ss [LUPDATE_SNOC]
+  \\ SEP_I_TAC "x64_sub_loop1" \\ POP_ASSUM MP_TAC
+  \\ MATCH_MP_TAC IMP_IMP \\ STRIP_TAC
+  THEN1 (FULL_SIMP_TAC (srw_ss()) [] \\ DECIDE_TAC)
+  \\ STRIP_TAC \\ ASM_SIMP_TAC std_ss []
+  \\ FULL_SIMP_TAC (srw_ss()) [LENGTH_SNOC,ADD1,AC ADD_COMM ADD_ASSOC,mw_sub_def,
+       LET_DEF,single_sub_def,bool2num_thm,single_add_def]
+  \\ CONV_TAC (DEPTH_CONV PairRules.PBETA_CONV)
+  \\ FULL_SIMP_TAC (srw_ss()) [b2w_def]
+  \\ `(18446744073709551616 <= b2n ~c + (w2n h' + w2n (~h))) =
+      ~(w2n h' < b2n c + w2n h)` by METIS_TAC [sub_borrow_lemma]
+  \\ FULL_SIMP_TAC std_ss [AC ADD_COMM ADD_ASSOC]
+  \\ REPEAT (STRIP_TAC THEN1 DECIDE_TAC)
+  \\ Cases_on `c` \\ FULL_SIMP_TAC std_ss [b2n_def]
+  \\ REPEAT (POP_ASSUM (K ALL_TAC))
+  \\ blastLib.BBLAST_TAC);
+
+val x64_sub_loop2_thm = prove(
+  ``!xs zs xs1 zs1 xs2 zs2
+     z_af z_of c z_pf z_sf z_zf r8.
+      (LENGTH zs1 = LENGTH xs1) /\ (LENGTH zs = LENGTH xs) /\
+      LENGTH (xs1 ++ xs) + 1 < 18446744073709551616 ==>
+      ?r8' r9' z_af' z_of' z_pf' z_sf' z_zf'.
+        x64_sub_loop2_pre (n2w (LENGTH xs + 1),r8,0w,n2w (LENGTH xs1),
+          xs1 ++ xs ++ xs2,z_af,SOME c,
+          z_of,z_pf,z_sf,z_zf,zs1 ++ zs ++ zs2) /\
+        (x64_sub_loop2 (n2w (LENGTH xs + 1),r8,0w,n2w (LENGTH xs1),
+          xs1 ++ xs ++ xs2,z_af,SOME c,
+          z_of,z_pf,z_sf,z_zf,zs1 ++ zs ++ zs2) =
+          (0w,r8',r9',n2w (LENGTH (xs1++xs)),xs1 ++ xs ++ xs2,z_af',
+             SOME (~SND (mw_sub xs (MAP (\x.0w) xs) ~c)),z_of',z_pf',z_sf',z_zf',
+                        zs1 ++ FST (mw_sub xs (MAP (\x.0w) xs) ~c) ++ zs2))``,
+  Induct THEN1
+   (FULL_SIMP_TAC (srw_ss()) [LENGTH,LENGTH_NIL,mw_sub_def]
+    \\ ONCE_REWRITE_TAC [x64_sub_loop_def]
+    \\ FULL_SIMP_TAC (srw_ss()) [LENGTH,LENGTH_NIL,mw_sub_def,LET_DEF])
+  \\ FULL_SIMP_TAC std_ss [LENGTH,ADD1]
+  \\ ONCE_REWRITE_TAC [x64_sub_loop_def]
+  \\ FULL_SIMP_TAC (srw_ss()) [LET_DEF]
+  \\ REPEAT STRIP_TAC
+  \\ `LENGTH xs < 18446744073709551616 /\
+      LENGTH xs + 1 < 18446744073709551616 /\
+      LENGTH xs + 1 + 1 < 18446744073709551616` by DECIDE_TAC
+  \\ `LENGTH xs1 < 18446744073709551616 /\
+      LENGTH xs1 + 1 < 18446744073709551616` by DECIDE_TAC
+  \\ FULL_SIMP_TAC std_ss []
+  \\ FULL_SIMP_TAC std_ss [GSYM APPEND_ASSOC,APPEND,
+        rich_listTheory.EL_LENGTH_APPEND,NULL_DEF,HD,TL]
+  \\ SIMP_TAC std_ss [GSYM word_sub_def,GSYM word_add_n2w,WORD_ADD_SUB]
+  \\ SIMP_TAC std_ss [word_add_n2w]
+  \\ Cases_on `zs` \\ FULL_SIMP_TAC std_ss [LENGTH,ADD1,APPEND]
+  \\ SIMP_TAC std_ss [SNOC_INTRO]
+  \\ POP_ASSUM (ASSUME_TAC o GSYM) \\ FULL_SIMP_TAC std_ss []
+  \\ `LENGTH xs1 + 1 = LENGTH (SNOC h xs1)` by
+    FULL_SIMP_TAC std_ss [LENGTH_SNOC,ADD1] \\ ASM_SIMP_TAC std_ss []
+  \\ ASM_SIMP_TAC std_ss [LUPDATE_SNOC]
+  \\ SEP_I_TAC "x64_sub_loop2" \\ POP_ASSUM MP_TAC
+  \\ MATCH_MP_TAC IMP_IMP \\ STRIP_TAC
+  THEN1 (FULL_SIMP_TAC (srw_ss()) [] \\ DECIDE_TAC)
+  \\ STRIP_TAC \\ ASM_SIMP_TAC std_ss []
+  \\ FULL_SIMP_TAC (srw_ss()) [LENGTH_SNOC,ADD1,AC ADD_COMM ADD_ASSOC,mw_sub_def,
+       LET_DEF,single_add_def,bool2num_thm,single_sub_def]
+  \\ CONV_TAC (DEPTH_CONV PairRules.PBETA_CONV)
+  \\ FULL_SIMP_TAC (srw_ss()) [b2w_def]
+  \\ `(18446744073709551616 <= b2n ~c + (w2n h + w2n (~(0w:word64)))) =
+      ~(w2n h < b2n c + w2n (0w:word64))` by METIS_TAC [sub_borrow_lemma]
+  \\ FULL_SIMP_TAC (srw_ss()) [AC ADD_COMM ADD_ASSOC]
+  \\ REPEAT (STRIP_TAC THEN1 DECIDE_TAC)
+  \\ Cases_on `c` \\ FULL_SIMP_TAC std_ss [b2n_def]
+  \\ REPEAT (POP_ASSUM (K ALL_TAC))
+  \\ blastLib.BBLAST_TAC);
+
+val x64_sub_thm = prove(
+  ``!xs ys zs zs2.
+      LENGTH ys <= LENGTH xs /\ (LENGTH zs = LENGTH xs) /\
+      LENGTH xs + 1 < 18446744073709551616 ==>
+      ?r1' r2' r8' r9' r10'.
+        x64_sub_pre (n2w (LENGTH ys),n2w (LENGTH xs),0w,0w,0w,xs,ys,zs++zs2) /\
+        (x64_sub (n2w (LENGTH ys),n2w (LENGTH xs),0w,0w,0w,xs,ys,zs++zs2) =
+          (r1',r2',r8',r9',n2w (LENGTH (mw_subv xs ys)),xs,ys,
+           mw_subv xs ys ++ REPLICATE (LENGTH xs - LENGTH (mw_subv xs ys)) 0w ++ zs2))``,
+  REPEAT STRIP_TAC \\ IMP_RES_TAC LESS_EQ_LENGTH
+  \\ FULL_SIMP_TAC std_ss [LENGTH_APPEND,x64_sub_def,LET_DEF]
+  \\ ONCE_REWRITE_TAC [ADD_COMM]
+  \\ SIMP_TAC std_ss [GSYM word_add_n2w,WORD_ADD_SUB]
+  \\ ONCE_REWRITE_TAC [x64_sub_loop_def]
+  \\ SIMP_TAC std_ss [LET_DEF,w2n_n2w,word_add_n2w,WORD_LO]
+  \\ FULL_SIMP_TAC (srw_ss()) []
+  \\ (x64_sub_loop1_thm |> Q.SPECL [`xs1`,`ys`,`zs`,`[]`,`[]`,`[]`,`xs2`,`[]`,`zs2`]
+      |> GEN_ALL |> MP_TAC)
+  \\ FULL_SIMP_TAC std_ss [LENGTH,APPEND,APPEND_NIL] \\ STRIP_TAC
+  \\ Q.PAT_ASSUM `LENGTH xs1 = LENGTH ys` (ASSUME_TAC o GSYM)
+  \\ FULL_SIMP_TAC std_ss [mw_subv_def,LET_DEF,mw_sub2_def,
+       rich_listTheory.DROP_LENGTH_APPEND,
+       rich_listTheory.TAKE_LENGTH_APPEND]
+  \\ `?qs1 c1. mw_sub xs1 ys T = (qs1,c1)` by METIS_TAC [PAIR]
+  \\ `?qs2 c2. mw_sub xs2 (MAP (\x.0w) xs2) c1 = (qs2,c2)` by METIS_TAC [PAIR]
+  \\ FULL_SIMP_TAC std_ss []
+  \\ `?zs1 zs3. (zs = zs1 ++ zs3) /\
+        (LENGTH zs1 = LENGTH xs1) /\
+        (LENGTH zs3 = LENGTH xs2)` by ALL_TAC THEN1
+     (IMP_RES_TAC LENGTH_mw_sub \\ FULL_SIMP_TAC std_ss []
+      \\ `LENGTH qs1 <= LENGTH zs` by DECIDE_TAC
+      \\ IMP_RES_TAC LESS_EQ_LENGTH \\ FULL_SIMP_TAC std_ss []
+      \\ Q.LIST_EXISTS_TAC [`xs1'`,`xs2'`] \\ FULL_SIMP_TAC std_ss []
+      \\ `LENGTH (xs1' ++ xs2') = LENGTH (qs1 ++ qs2)` by ALL_TAC
+      \\ FULL_SIMP_TAC std_ss [LENGTH_APPEND] \\ DECIDE_TAC)
+  \\ FULL_SIMP_TAC std_ss [GSYM APPEND_ASSOC]
+  \\ SEP_I_TAC "x64_sub_loop1" \\ POP_ASSUM MP_TAC
+  \\ MATCH_MP_TAC IMP_IMP \\ STRIP_TAC
+  THEN1 (FULL_SIMP_TAC (srw_ss()) [] \\ DECIDE_TAC)
+  \\ STRIP_TAC \\ ASM_SIMP_TAC std_ss []
+  \\ (x64_sub_loop2_thm |> Q.SPECL [`xs`,`ys`,`xs1`,`zs1`,`[]`] |> GEN_ALL
+       |> SIMP_RULE std_ss [GSYM APPEND_ASSOC,APPEND_NIL] |> ASSUME_TAC)
+  \\ SEP_I_TAC "x64_sub_loop2" \\ POP_ASSUM MP_TAC
+  \\ MATCH_MP_TAC IMP_IMP \\ STRIP_TAC
+  THEN1 (IMP_RES_TAC LENGTH_mw_sub \\ FULL_SIMP_TAC (srw_ss()) [] \\ DECIDE_TAC)
+  \\ STRIP_TAC \\ ASM_SIMP_TAC std_ss []
+  \\ FULL_SIMP_TAC std_ss [APPEND_ASSOC]
+  \\ IMP_RES_TAC LENGTH_mw_sub
+  \\ `LENGTH (xs1 ++ xs2) = LENGTH (qs1 ++ qs2)` by FULL_SIMP_TAC std_ss [LENGTH_APPEND]
+  \\ `LENGTH (qs1 ++ qs2) < dimword (:64)` by
+        (FULL_SIMP_TAC (srw_ss()) [] \\ DECIDE_TAC)
+  \\ FULL_SIMP_TAC std_ss []
+  \\ IMP_RES_TAC x64_trailing_thm \\ SEP_I_TAC "x64_trailing"
+  \\ FULL_SIMP_TAC std_ss []
+  \\ FULL_SIMP_TAC std_ss [LENGTH_APPEND,AC ADD_COMM ADD_ASSOC]);
+
+(* integer addition *)
+
+val (res,x64_iadd1_def,x64_iadd1_pre_def) = x64_compile `
+  x64_iadd1 (r1:word64,r2:word64,xs:word64 list,ys:word64 list,xa:word64,ya:word64) =
+    let r0 = 0w:word64 in
+      if r1 <+ r2 then
+        let (xa,xs,ya,ys) = (ya,ys,xa,xs) in
+        let r0 = 1w in
+          (r1,r2,r0,xs,ys,xa,ya)
+      else
+        let r8 = r1 in
+        let r1 = r2 in
+        let r2 = r8 in
+          (r1,r2,r0,xs,ys,xa,ya)`
+
+val (res,x64_iadd2_def,x64_iadd2_pre_def) = x64_compile `
+  x64_iadd2 (r1:word64,r2:word64,r10:word64,r12:word64,xs,ys,xa,ya) =
+    let r0 = 0w:word64 in
+      if r10 = 1w then
+        let (xa,xs,ya,ys) = (ya,ys,xa,xs) in
+        let r12 = r12 ?? 1w in
+        let r0 = 1w in
+          (r1,r2,r0,r12,xs,ys,xa,ya)
+      else
+        let r8 = r1 in
+        let r1 = r2 in
+        let r2 = r8 in
+          (r1,r2,r0,r12,xs:word64 list,ys:word64 list,xa:word64,ya:word64)`
+
+val (res,x64_iadd3_def,x64_iadd3_pre_def) = x64_compile `
+  x64_iadd3 (r0:word64,xs:word64 list,ys:word64 list,xa:word64,ya:word64) =
+      if r0 = 0w then (xs,ys,xa,ya) else
+        let (xa,xs,ya,ys) = (ya,ys,xa,xs) in
+          (xs,ys,xa,ya)`
+
+val (res,x64_iadd_def,x64_iadd_pre_def) = x64_compile `
+  x64_iadd (r1:word64,r2:word64,xs:word64 list,ys:word64 list,zs:word64 list,xa,ya) =
+    let r10 = r1 && 1w in
+    let r11 = r2 && 1w in
+      if r10 = r11 then (* same sign *)
+        let r1 = r1 >>> 1 in
+        let r2 = r2 >>> 1 in
+        let (r1,r2,r0,xs,ys,xa,ya) = x64_iadd1 (r1,r2,xs,ys,xa,ya) in
+        let r8 = 0w in
+        let r9 = r8 in
+        let r10 = r8 in
+        let (r1,r2,r8,r9,r10,xs,ys,zs) = x64_add (r1,r2,r8,r9,r10,xs,ys,zs) in
+        let (xs,ys,xa,ya) = x64_iadd3 (r0,xs,ys,xa,ya) in
+        let r10 = r10 << 1 in
+        let r10 = r10 + r11 in
+          (r10,xs,ys,zs,xa,ya)
+      else (* signs differ *)
+        let r12 = r10 in
+        let r10 = r1 >>> 1 in
+        let r11 = r2 >>> 1 in
+        let (r10,xs,ys) = x64_compare (r10,r11,xs,ys) in
+          if r10 = 0w then
+            (r10,xs,ys,zs,xa,ya)
+          else
+            let (r1,r2,r0,r12,xs,ys,xa,ya) = x64_iadd2 (r1,r2,r10,r12,xs,ys,xa,ya) in
+            let r8 = 0w in
+            let r9 = r8 in
+            let r10 = r8 in
+            let r1 = r1 >>> 1 in
+            let r2 = r2 >>> 1 in
+            let (r1,r2,r8,r9,r10,xs,ys,zs) = x64_sub (r1,r2,r8,r9,r10,xs,ys,zs) in
+            let (xs,ys,xa,ya) = x64_iadd3 (r0,xs,ys,xa,ya) in
+            let r10 = r10 << 1 in
+            let r10 = r10 + r12 in
+              (r10,xs,ys,zs,xa,ya)`
+
+val x64_header_AND_1 = prove(
+  ``x64_header (s,xs) && 0x1w = b2w s``,
+  FULL_SIMP_TAC std_ss [x64_header_def,GSYM word_mul_n2w]
+  \\ Cases_on `s` \\ FULL_SIMP_TAC std_ss [b2w_def,b2n_def]
+  \\ blastLib.BBLAST_TAC);
+
+val x64_header_EQ = prove(
+  ``(x64_header (s,xs) && 0x1w = x64_header (t,ys) && 0x1w) = (s = t)``,
+  FULL_SIMP_TAC std_ss [x64_header_AND_1]
+  \\ Cases_on `s` \\ Cases_on `t` \\ EVAL_TAC);
+
+val b2w_NOT = prove(
+  ``!s. b2w s ?? 0x1w = b2w (~s):word64``,
+  Cases \\ EVAL_TAC);
+
+val x64_iadd_thm = prove(
+  ``LENGTH xs < dimword (:63) /\ LENGTH ys < dimword (:63) /\
+    LENGTH xs + LENGTH ys <= LENGTH zs /\ mw_ok xs /\ mw_ok ys ==>
+    ?zs1.
+      x64_iadd_pre (x64_header (s,xs),x64_header (t,ys),xs,ys,zs,xa,ya) /\
+      (x64_iadd (x64_header (s,xs),x64_header (t,ys),xs,ys,zs,xa,ya) =
+        (x64_header (mwi_add (s,xs) (t,ys)),xs,ys,
+         SND (mwi_add (s,xs) (t,ys))++zs1,xa,ya)) /\
+      (LENGTH (SND (mwi_add (s,xs) (t,ys))++zs1) = LENGTH zs) ``,
+  FULL_SIMP_TAC std_ss [x64_iadd_def,x64_iadd_pre_def,LET_DEF]
+  \\ FULL_SIMP_TAC std_ss [x64_header_EQ,mwi_add_def,x64_length]
+  \\ Cases_on `s <=> t` \\ FULL_SIMP_TAC std_ss []
+  \\ REPEAT STRIP_TAC \\ IMP_RES_TAC dim63_IMP_dim64 THEN1
+   (Cases_on `LENGTH ys <= LENGTH xs` \\ FULL_SIMP_TAC std_ss []
+    \\ FULL_SIMP_TAC (srw_ss()) [x64_iadd1_def,WORD_LO,GSYM NOT_LESS,LET_DEF]
+    THEN1
+     (ASSUME_TAC x64_add_thm
+      \\ `LENGTH (mw_addv xs ys F) <= LENGTH xs + LENGTH ys` by
+            FULL_SIMP_TAC std_ss [LENGTH_mw_addv,NOT_LESS]
+      \\ `LENGTH (mw_addv xs ys F) <= LENGTH zs` by DECIDE_TAC
+      \\ IMP_RES_TAC LESS_EQ_LENGTH
+      \\ FULL_SIMP_TAC std_ss []
+      \\ SEP_I_TAC "x64_add" \\ POP_ASSUM MP_TAC
+      \\ MATCH_MP_TAC IMP_IMP \\ STRIP_TAC
+      THEN1 (FULL_SIMP_TAC std_ss [] \\ DECIDE_TAC)
+      \\ REPEAT STRIP_TAC \\ FULL_SIMP_TAC std_ss [LENGTH_APPEND]
+      \\ FULL_SIMP_TAC (srw_ss()) [LENGTH_APPEND,x64_iadd3_def,x64_iadd3_pre_def,LET_DEF]
+      \\ FULL_SIMP_TAC std_ss [WORD_MUL_LSL,word_mul_n2w]
+      \\ ONCE_REWRITE_TAC [WORD_AND_COMM]
+      \\ FULL_SIMP_TAC std_ss [x64_header_AND_1]
+      \\ FULL_SIMP_TAC std_ss [x64_header_def,AC MULT_COMM MULT_ASSOC]
+      \\ Cases_on `t` \\ FULL_SIMP_TAC (srw_ss()) [b2w_def,b2n_def,
+           AC ADD_COMM ADD_ASSOC,word_add_n2w])
+    THEN1
+     (ASSUME_TAC x64_add_thm
+      \\ `LENGTH (mw_addv ys xs F) <= LENGTH ys + LENGTH xs` by
+         (`LENGTH xs <= LENGTH ys` by DECIDE_TAC
+          \\ FULL_SIMP_TAC std_ss [LENGTH_mw_addv])
+      \\ `LENGTH (mw_addv ys xs F) <= LENGTH zs` by DECIDE_TAC
+      \\ IMP_RES_TAC LESS_EQ_LENGTH
+      \\ FULL_SIMP_TAC std_ss []
+      \\ SEP_I_TAC "x64_add" \\ POP_ASSUM MP_TAC
+      \\ MATCH_MP_TAC IMP_IMP \\ STRIP_TAC
+      THEN1 (FULL_SIMP_TAC std_ss [] \\ DECIDE_TAC)
+      \\ REPEAT STRIP_TAC \\ FULL_SIMP_TAC std_ss [LENGTH_APPEND]
+      \\ FULL_SIMP_TAC (srw_ss()) [LENGTH_APPEND,x64_iadd3_def,x64_iadd3_pre_def,LET_DEF]
+      \\ FULL_SIMP_TAC std_ss [WORD_MUL_LSL,word_mul_n2w]
+      \\ ONCE_REWRITE_TAC [WORD_AND_COMM]
+      \\ FULL_SIMP_TAC std_ss [x64_header_AND_1]
+      \\ FULL_SIMP_TAC std_ss [x64_header_def,AC MULT_COMM MULT_ASSOC]
+      \\ Cases_on `t` \\ FULL_SIMP_TAC (srw_ss()) [b2w_def,b2n_def,
+           AC ADD_COMM ADD_ASSOC,word_add_n2w]))
+  \\ FULL_SIMP_TAC std_ss [x64_compare_thm,mw_compare_thm]
+  \\ Cases_on `mw2n ys = mw2n xs` \\ FULL_SIMP_TAC std_ss [cmp2w_def]
+  THEN1 (FULL_SIMP_TAC (srw_ss()) [x64_header_def,APPEND,LENGTH])
+  \\ Cases_on `mw2n xs < mw2n ys` \\ FULL_SIMP_TAC std_ss [GSYM NOT_LESS]
+  \\ FULL_SIMP_TAC (srw_ss()) [cmp2w_def,x64_iadd2_def,LET_DEF]
+  THEN1
+   (`LENGTH ys <= LENGTH zs` by DECIDE_TAC
+    \\ IMP_RES_TAC LESS_EQ_LENGTH
+    \\ FULL_SIMP_TAC std_ss []
+    \\ ASSUME_TAC x64_sub_thm
+    \\ FULL_SIMP_TAC (srw_ss()) [x64_length]
+    \\ SEP_I_TAC "x64_sub" \\ POP_ASSUM MP_TAC
+    \\ MATCH_MP_TAC IMP_IMP \\ STRIP_TAC
+    \\ `mw2n xs <= mw2n ys` by DECIDE_TAC
+    \\ IMP_RES_TAC mw2n_LESS
+    THEN1 (FULL_SIMP_TAC std_ss [] \\ DECIDE_TAC)
+    \\ REPEAT STRIP_TAC
+    \\ FULL_SIMP_TAC std_ss [LENGTH_APPEND,x64_iadd3_def,
+         x64_iadd3_pre_def,LET_DEF,EVAL ``1w=0w:word64``]
+    \\ SIMP_TAC (srw_ss()) [GSYM APPEND_ASSOC,LENGTH_REPLICATE]
+    \\ STRIP_TAC THEN1
+     (FULL_SIMP_TAC std_ss [WORD_MUL_LSL,word_mul_n2w]
+      \\ ONCE_REWRITE_TAC [WORD_AND_COMM]
+      \\ FULL_SIMP_TAC std_ss [x64_header_AND_1]
+      \\ FULL_SIMP_TAC std_ss [x64_header_def,AC MULT_COMM MULT_ASSOC]
+      \\ FULL_SIMP_TAC std_ss [b2w_NOT]
+      \\ Cases_on `s` \\ FULL_SIMP_TAC (srw_ss()) [b2w_def,b2n_def,
+           AC ADD_COMM ADD_ASSOC,word_add_n2w])
+    \\ `LENGTH (mw_subv ys xs) <= LENGTH ys` by ASM_SIMP_TAC std_ss [LENGTH_mw_subv]
+    \\ DECIDE_TAC)
+  THEN1
+   (`LENGTH xs <= LENGTH zs` by DECIDE_TAC
+    \\ IMP_RES_TAC LESS_EQ_LENGTH
+    \\ FULL_SIMP_TAC std_ss []
+    \\ ASSUME_TAC x64_sub_thm
+    \\ FULL_SIMP_TAC (srw_ss()) [x64_length]
+    \\ SEP_I_TAC "x64_sub" \\ POP_ASSUM MP_TAC
+    \\ MATCH_MP_TAC IMP_IMP \\ STRIP_TAC
+    \\ `mw2n ys <= mw2n xs` by DECIDE_TAC
+    \\ IMP_RES_TAC mw2n_LESS
+    THEN1 (FULL_SIMP_TAC std_ss [] \\ DECIDE_TAC)
+    \\ REPEAT STRIP_TAC
+    \\ FULL_SIMP_TAC std_ss [LENGTH_APPEND,x64_iadd3_def,x64_iadd3_pre_def,LET_DEF]
+    \\ SIMP_TAC (srw_ss()) [GSYM APPEND_ASSOC,LENGTH_REPLICATE]
+    \\ STRIP_TAC THEN1
+     (FULL_SIMP_TAC std_ss [WORD_MUL_LSL,word_mul_n2w]
+      \\ ONCE_REWRITE_TAC [WORD_AND_COMM]
+      \\ FULL_SIMP_TAC std_ss [x64_header_AND_1]
+      \\ FULL_SIMP_TAC std_ss [x64_header_def,AC MULT_COMM MULT_ASSOC]
+      \\ FULL_SIMP_TAC std_ss [b2w_NOT]
+      \\ Cases_on `s` \\ FULL_SIMP_TAC (srw_ss()) [b2w_def,b2n_def,
+           AC ADD_COMM ADD_ASSOC,word_add_n2w])
+    \\ `LENGTH (mw_subv xs ys) <= LENGTH xs` by ASM_SIMP_TAC std_ss [LENGTH_mw_subv]
+    \\ DECIDE_TAC));
+
+
+(* multiplication *)
+
+val (x64_single_mul_add_res,
+     x64_single_mul_add_def) = x64_decompile "x64_single_mul_add" `
+  mul r2
+  add r0,r1
+  adc r2,0
+  add r0,r3
+  adc r2,0`
+
+val _ = add_compiled [x64_single_mul_add_res]
+
+val x64_single_mul_add_thm = prove(
+  ``x64_single_mul_add_pre (p,k,q,s) /\
+    (x64_single_mul_add (p,k,q,s) =
+      let (x1,x2) = single_mul_add p q k s in (x1,k,x2,s))``,
+  FULL_SIMP_TAC (srw_ss()) [x64_single_mul_add_def,LET_DEF]
+  \\ Cases_on `k` \\ Cases_on `s` \\ Cases_on `p` \\ Cases_on `q`
+  \\ FULL_SIMP_TAC (srw_ss()) [single_mul_add_def,LET_DEF,single_mul_def,bool2num_thm,
+       mw_add_def,single_add_def,b2n_def,b2w_def,word_add_n2w,word_mul_n2w]
+  \\ FULL_SIMP_TAC std_ss [AC ADD_COMM ADD_ASSOC, AC MULT_COMM MULT_ASSOC]
+  \\ `10 < 18446744073709551616` by DECIDE_TAC
+  \\ Q.ABBREV_TAC `k = 18446744073709551616` \\ POP_ASSUM (K ALL_TAC)
+  \\ FULL_SIMP_TAC std_ss [ADD_ASSOC]
+  \\ `n'' * n''' DIV k + b2n (k <= n + (n'' * n''') MOD k) =
+      (n + n'' * n''') DIV k` by ALL_TAC \\ FULL_SIMP_TAC std_ss []
+  \\ Q.SPEC_TAC (`n'' * n'''`,`l`) \\ STRIP_TAC
+  \\ `0 < k` by DECIDE_TAC
+  \\ `(n + l) DIV k = l DIV k + (n + l MOD k) DIV k` by ALL_TAC THEN1
+   (SIMP_TAC std_ss [Once ADD_COMM]
+    \\ STRIP_ASSUME_TAC (SIMP_RULE bool_ss [PULL_FORALL] DIVISION
+         |> Q.SPECL [`k`,`l`] |> UNDISCH_ALL |> ONCE_REWRITE_RULE [CONJ_COMM])
+    \\ POP_ASSUM (fn th => SIMP_TAC std_ss [Once th])
+    \\ FULL_SIMP_TAC std_ss [GSYM ADD_ASSOC,ADD_DIV_ADD_DIV]
+    \\ FULL_SIMP_TAC std_ss [AC ADD_ASSOC ADD_COMM])
+  \\ FULL_SIMP_TAC std_ss []
+  \\ Cases_on `k <= n + l MOD k` \\ FULL_SIMP_TAC std_ss [b2n_def]
+  \\ SIMP_TAC std_ss [Once EQ_SYM_EQ]
+  \\ `l MOD k < k` by FULL_SIMP_TAC std_ss []
+  \\ ASM_SIMP_TAC std_ss [DIV_EQ_X] \\ DECIDE_TAC);
+
+val (res,x64_mul_pass_def,x64_mul_pass_pre_def) = x64_compile `
+  x64_mul_pass (r1:word64,r8:word64,r9:word64,r10:word64,r11:word64,ys:word64 list,zs:word64 list) =
+    if r9 = r11 then
+      let zs = LUPDATE r1 (w2n r10) zs in
+      let r10 = r10 + 1w in
+        (r1,r9,r10,ys,zs)
+    else
+      let r3 = EL (w2n r10) zs in
+      let r2 = EL (w2n r11) ys in
+      let r0 = r8 in
+      let (r0,r1,r2,r3) = x64_single_mul_add (r0,r1,r2,r3) in
+      let zs = LUPDATE r0 (w2n r10) zs in
+      let r1 = r2 in
+      let r10 = r10 + 1w in
+      let r11 = r11 + 1w in
+        x64_mul_pass (r1,r8,r9,r10,r11,ys,zs)`
+
+val (res,x64_mul_def,x64_mul_pre_def) = x64_compile `
+  x64_mul (r7:word64,r9,r10:word64,r12:word64,xs:word64 list,ys,zs) =
+    if r7 = 0w then let r10 = r10 + r9 in (r10,xs,ys,zs) else
+      let r7 = r7 - 1w in
+      let r8 = EL (w2n r12) xs in
+      let r12 = r12 + 1w in
+      let r11 = 0w in
+      let r1 = r11 in
+      let (r1,r9,r10,ys,zs) = x64_mul_pass (r1,r8,r9,r10,r11,ys,zs) in
+      let r10 = r10 - r9 in
+        x64_mul (r7,r9,r10,r12,xs,ys,zs)`
+
+val (res,x64_mul_zero_def,x64_mul_zero_pre_def) = x64_compile `
+  x64_mul_zero (r0:word64,r10:word64,zs:word64 list) =
+    if r10 = 0w then (r10,zs) else
+      let r10 = r10 - 1w in
+      let zs = LUPDATE r0 (w2n r10) zs in
+        x64_mul_zero (r0,r10,zs)`;
+
+val (res,x64_imul_def,x64_imul_pre_def) = x64_compile `
+  x64_imul (r1:word64,r2:word64,xs:word64 list,ys:word64 list,zs:word64 list) =
+    let r10 = 0w in
+      if r1 = 0w then (r10,xs,ys,zs) else
+      if r2 = 0w then (r10,xs,ys,zs) else
+        let r0 = 0w in
+        let r10 = r2 >>> 1 in
+        let (r10,zs) = x64_mul_zero (r0,r10,zs) in
+        let r10 = r1 && 1w in
+        let r11 = r2 && 1w in
+          if r10 = r11 then
+            let r7 = r1 >>> 1 in
+            let r9 = r2 >>> 1 in
+            let r10 = 0w in
+            let r12 = r10 in
+            let (r10,xs,ys,zs) = x64_mul (r7,r9,r10,r12,xs,ys,zs) in
+            let r8 = 0w in
+            let (r8,r10,zs) = x64_trailing (r8,r10,zs) in
+            let r10 = r10 << 1 in
+              (r10,xs,ys,zs)
+          else
+            let r7 = r1 >>> 1 in
+            let r9 = r2 >>> 1 in
+            let r10 = 0w in
+            let r12 = r10 in
+            let (r10,xs,ys,zs) = x64_mul (r7,r9,r10,r12,xs,ys,zs) in
+            let r8 = 0w in
+            let (r8,r10,zs) = x64_trailing (r8,r10,zs) in
+            let r10 = r10 << 1 in
+            let r10 = r10 + 1w in
+              (r10,xs,ys,zs)`;
+
+val x64_mul_pass_thm = prove(
+  ``!ys ys1 x zs k zs1 zs2 z2.
+      LENGTH (ys1++ys) < dimword (:64) /\  (LENGTH zs = LENGTH ys) /\
+      LENGTH (zs1++zs) < dimword (:64) ==>
+      ?r1.
+        x64_mul_pass_pre (k,x,n2w (LENGTH (ys1++ys)),n2w (LENGTH zs1),
+                          n2w (LENGTH ys1),ys1++ys,zs1++zs++z2::zs2) /\
+        (x64_mul_pass (k,x,n2w (LENGTH (ys1++ys)),n2w (LENGTH zs1),
+                       n2w (LENGTH ys1),ys1++ys,zs1++zs++z2::zs2) =
+           (r1,n2w (LENGTH (ys1++ys)),n2w (LENGTH (zs1++zs)+1),ys1++ys,
+            zs1++(mw_mul_pass x ys zs k)++zs2))``,
+  Induct \\ Cases_on `zs`
+  \\ FULL_SIMP_TAC std_ss [LENGTH,APPEND_NIL,mw_mul_pass_def,ADD1]
+  \\ ONCE_REWRITE_TAC [x64_mul_pass_def,x64_mul_pass_pre_def]
+  \\ FULL_SIMP_TAC std_ss [LET_DEF,n2w_11,w2n_n2w,LUPDATE_LENGTH]
+  \\ FULL_SIMP_TAC std_ss [GSYM APPEND_ASSOC,APPEND,word_add_n2w,LENGTH_APPEND]
+  \\ FULL_SIMP_TAC std_ss [LENGTH]
+  \\ REPEAT STRIP_TAC
+  \\ IMP_RES_TAC (DECIDE ``m+n<k ==> m < k /\ n<k:num``)
+  \\ FULL_SIMP_TAC std_ss [ADD1,x64_single_mul_add_thm]
+  \\ FULL_SIMP_TAC std_ss [rich_listTheory.EL_LENGTH_APPEND,LUPDATE_LENGTH,NULL,HD]
+  \\ Cases_on `single_mul_add x h' k h` \\ FULL_SIMP_TAC std_ss [LET_DEF,TL]
+  \\ ONCE_REWRITE_TAC [SNOC_INTRO |> Q.INST [`xs2`|->`[]`] |> REWRITE_RULE [APPEND_NIL]]
+  \\ `((LENGTH ys1 + (LENGTH ys + 1)) = (LENGTH (SNOC h' ys1) + LENGTH ys)) /\
+      ((LENGTH ys1 + 1) = (LENGTH (SNOC h' ys1))) /\
+      ((LENGTH zs1 + 1) = LENGTH (SNOC q zs1))` by ALL_TAC
+  THEN1 (FULL_SIMP_TAC std_ss [LENGTH_SNOC] \\ DECIDE_TAC)
+  \\ FULL_SIMP_TAC std_ss []
+  \\ SEP_I_TAC "x64_mul_pass" \\ POP_ASSUM MP_TAC
+  \\ MATCH_MP_TAC IMP_IMP \\ STRIP_TAC
+  THEN1 (FULL_SIMP_TAC (srw_ss()) [] \\ DECIDE_TAC)
+  \\ REPEAT STRIP_TAC \\ FULL_SIMP_TAC std_ss []
+  \\ FULL_SIMP_TAC std_ss [SNOC_APPEND,GSYM APPEND_ASSOC,APPEND,
+       LENGTH_APPEND,LENGTH,AC ADD_COMM ADD_ASSOC] \\ DECIDE_TAC)
+  |> Q.SPECL [`ys`,`[]`] |> SIMP_RULE std_ss [APPEND,LENGTH] |> GEN_ALL;
+
+val WORD_SUB_LEMMA = prove(
+  ``v + -1w * w = v - w``,
+  FULL_SIMP_TAC (srw_ss()) []);
+
+val x64_mul_thm = prove(
+  ``!xs ys zs xs1 zs1 zs2.
+      LENGTH (xs1 ++ xs) < dimword (:64) /\ LENGTH ys < dimword (:64) /\
+      (LENGTH zs = LENGTH ys) /\ LENGTH (zs1++zs++zs2) < dimword (:64) /\
+      LENGTH xs <= LENGTH zs2 /\ ys <> [] ==>
+      ?zs3.
+        x64_mul_pre (n2w (LENGTH xs),n2w (LENGTH ys),n2w (LENGTH zs1),n2w (LENGTH xs1),
+                 xs1 ++ xs,ys,zs1 ++ zs ++ zs2) /\
+       (x64_mul (n2w (LENGTH xs),n2w (LENGTH ys),n2w (LENGTH zs1),n2w (LENGTH xs1),
+                 xs1 ++ xs,ys,zs1 ++ zs ++ zs2) =
+          (n2w (LENGTH (zs1 ++ mw_mul xs ys zs)),xs1++xs,ys,zs1 ++ mw_mul xs ys zs ++ zs3)) /\
+       (LENGTH (zs1 ++ zs ++ zs2) = LENGTH (zs1 ++ mw_mul xs ys zs ++ zs3))``,
+  Induct \\ ONCE_REWRITE_TAC [x64_mul_def,x64_mul_pre_def]
+  \\ FULL_SIMP_TAC std_ss [LENGTH,mw_mul_def,APPEND_NIL,LET_DEF]
+  \\ FULL_SIMP_TAC std_ss [LENGTH_APPEND,word_add_n2w]
+  THEN1 (METIS_TAC [])
+  \\ NTAC 7 STRIP_TAC
+  \\ IMP_RES_TAC (DECIDE ``m+n<k ==> m < k /\ n<k:num``)
+  \\ IMP_RES_TAC (DECIDE ``SUC n < k ==> n < k``)
+  \\ FULL_SIMP_TAC (srw_ss()) []
+  \\ FULL_SIMP_TAC std_ss [rich_listTheory.EL_LENGTH_APPEND,LUPDATE_LENGTH,NULL,HD]
+  \\ FULL_SIMP_TAC std_ss [GSYM word_sub_def,ADD1,GSYM word_add_n2w,WORD_ADD_SUB]
+  \\ Cases_on `zs2` \\ FULL_SIMP_TAC std_ss [LENGTH]
+  \\ ASSUME_TAC x64_mul_pass_thm
+  \\ SEP_I_TAC "x64_mul_pass" \\ POP_ASSUM MP_TAC
+  \\ MATCH_MP_TAC IMP_IMP \\ STRIP_TAC
+  THEN1 (FULL_SIMP_TAC (srw_ss()) [] \\ DECIDE_TAC)
+  \\ STRIP_TAC \\ FULL_SIMP_TAC std_ss []
+  \\ `LENGTH (mw_mul_pass h ys zs 0x0w) = LENGTH ys + 1` by ALL_TAC
+  THEN1 (FULL_SIMP_TAC std_ss [LENGTH_mw_mul_pass])
+  \\ Cases_on `mw_mul_pass h ys zs 0x0w`
+  \\ FULL_SIMP_TAC std_ss [LENGTH,ADD1]
+  \\ `n2w (LENGTH (zs1 ++ zs:word64 list) + 1) + -0x1w * n2w (LENGTH (ys:word64 list)) =
+      n2w (LENGTH (SNOC h'' zs1)):word64` by ALL_TAC THEN1
+   (FULL_SIMP_TAC std_ss [WORD_SUB_LEMMA,LENGTH,LENGTH_APPEND]
+    \\ `LENGTH zs1 + LENGTH ys + 1 = (LENGTH zs1 + 1) + LENGTH ys` by DECIDE_TAC
+    \\ ASM_SIMP_TAC std_ss []
+    \\ FULL_SIMP_TAC std_ss [GSYM word_add_n2w,WORD_ADD_SUB]
+    \\ FULL_SIMP_TAC std_ss [word_add_n2w,LENGTH_SNOC,ADD1])
+  \\ `n2w (LENGTH xs1) + 0x1w = n2w (LENGTH (SNOC h xs1)):word64` by ALL_TAC
+  THEN1 (FULL_SIMP_TAC std_ss [word_add_n2w,LENGTH_SNOC,ADD1])
+  \\ FULL_SIMP_TAC std_ss []
+  \\ FULL_SIMP_TAC std_ss [GSYM APPEND_ASSOC,APPEND]
+  \\ ONCE_REWRITE_TAC [SNOC_INTRO |> Q.INST [`xs2`|->`[]`] |> REWRITE_RULE [APPEND_NIL]]
+  \\ SEP_I_TAC "x64_mul" \\ POP_ASSUM MP_TAC
+  \\ MATCH_MP_TAC IMP_IMP \\ STRIP_TAC
+  THEN1 (FULL_SIMP_TAC (srw_ss()) [] \\ REPEAT STRIP_TAC \\ DECIDE_TAC)
+  \\ STRIP_TAC \\ FULL_SIMP_TAC std_ss []
+  \\ SIMP_TAC std_ss [word_add_n2w,TL,LENGTH_SNOC,ADD1,HD,AC ADD_COMM ADD_ASSOC]
+  \\ POP_ASSUM MP_TAC \\ FULL_SIMP_TAC std_ss [LENGTH_mw_mul] \\ STRIP_TAC
+  \\ Q.EXISTS_TAC `zs3` \\ DECIDE_TAC)
+  |> Q.SPECL [`xs`,`ys`,`zs`,`[]`,`[]`,`zs2`]
+  |> SIMP_RULE std_ss [LENGTH,APPEND] |> GEN_ALL;
+
+val x64_mul_zero_thm = prove(
+  ``!zs zs1.
+      LENGTH zs < dimword(:64) ==>
+        x64_mul_zero_pre (0w,n2w (LENGTH zs),zs++zs1) /\
+        (x64_mul_zero (0w,n2w (LENGTH zs),zs++zs1) = (0w,MAP (\x.0w) zs ++ zs1))``,
+  HO_MATCH_MP_TAC SNOC_INDUCT \\ FULL_SIMP_TAC std_ss [LENGTH,LENGTH_NIL]
+  \\ NTAC 3 STRIP_TAC
+  \\ ONCE_REWRITE_TAC [x64_mul_zero_def,x64_mul_zero_pre_def]
+  \\ FULL_SIMP_TAC (srw_ss()) [rich_listTheory.REPLICATE,LET_DEF]
+  \\ NTAC 3 STRIP_TAC
+  \\ FULL_SIMP_TAC std_ss [GSYM word_add_n2w,ADD1,GSYM word_sub_def,WORD_ADD_SUB]
+  \\ IMP_RES_TAC (DECIDE ``n+1<k ==> n<k``)
+  \\ FULL_SIMP_TAC (srw_ss()) [w2n_n2w]
+  \\ FULL_SIMP_TAC std_ss [SNOC_APPEND,GSYM APPEND_ASSOC,
+       APPEND,LUPDATE_LENGTH,MAP_APPEND,MAP] \\ DECIDE_TAC);
+
+val MAP_EQ_MAP_EQ = prove(
+  ``!xs ys. (MAP (\x.0w) xs = MAP (\x.0w) ys) = (LENGTH xs = LENGTH ys)``,
+  Induct \\ Cases_on `ys` \\ FULL_SIMP_TAC (srw_ss()) []);
+
+val x64_imul_thm = prove(
+  ``((x64_header (s,xs) = 0w) = (xs = [])) /\
+    ((x64_header (t,ys) = 0w) = (ys = [])) /\
+    LENGTH xs < dimword (:63) /\ LENGTH ys < dimword (:63) /\
+    LENGTH xs + LENGTH ys <= LENGTH zs /\ LENGTH zs < dimword (:63) ==>
+    ?zs1.
+      x64_imul_pre (x64_header (s,xs),x64_header (t,ys),xs,ys,zs) /\
+      (x64_imul (x64_header (s,xs),x64_header (t,ys),xs,ys,zs) =
+        (x64_header (mwi_mul_simple (s,xs) (t,ys)),xs,ys,
+         SND (mwi_mul_simple (s,xs) (t,ys))++zs1)) /\
+      (LENGTH (SND (mwi_mul_simple (s,xs) (t,ys))++zs1) = LENGTH zs) ``,
+  FULL_SIMP_TAC std_ss [x64_imul_def,x64_imul_pre_def,LET_DEF]
+  \\ FULL_SIMP_TAC std_ss [x64_header_EQ,mwi_mul_simple_def,x64_length]
+  \\ Cases_on `xs = []` \\ FULL_SIMP_TAC std_ss [APPEND]
+  THEN1 (REPEAT STRIP_TAC \\ EVAL_TAC)
+  \\ Cases_on `ys = []` \\ FULL_SIMP_TAC std_ss [APPEND]
+  THEN1 (REPEAT STRIP_TAC \\ EVAL_TAC)
+  \\ REPEAT STRIP_TAC
+  \\ `LENGTH ys <= LENGTH zs` by DECIDE_TAC
+  \\ `?qs1 qs2. (zs = qs1 ++ qs2) /\ (LENGTH ys = LENGTH qs1)` by
+       METIS_TAC [LESS_EQ_LENGTH]
+  \\ `LENGTH qs1 < dimword (:64)` by (FULL_SIMP_TAC (srw_ss()) [] \\ DECIDE_TAC)
+  \\ FULL_SIMP_TAC std_ss [x64_mul_zero_thm]
+  \\ ASSUME_TAC x64_mul_thm
+  \\ Q.PAT_ASSUM `LENGTH ys = LENGTH qs1` (ASSUME_TAC o GSYM)
+  \\ `MAP (\x. 0x0w:word64) qs1 = MAP (\x. 0x0w) ys` by
+       ASM_SIMP_TAC std_ss [MAP_EQ_MAP_EQ]
+  \\ FULL_SIMP_TAC std_ss []
+  \\ SEP_I_TAC "x64_mul" \\ POP_ASSUM MP_TAC
+  \\ MATCH_MP_TAC IMP_IMP \\ STRIP_TAC
+  THEN1 (FULL_SIMP_TAC (srw_ss()) [LENGTH_APPEND] \\ DECIDE_TAC)
+  \\ STRIP_TAC \\ FULL_SIMP_TAC std_ss []
+  \\ `LENGTH qs1 < dimword (:64)` by (FULL_SIMP_TAC (srw_ss()) [] \\ DECIDE_TAC)
+  \\ `LENGTH (mw_mul xs ys (MAP (\x. 0x0w) ys)) < dimword (:64)` by ALL_TAC
+  THEN1 (FULL_SIMP_TAC (srw_ss()) [LENGTH_mw_mul,LENGTH_MAP] \\ DECIDE_TAC)
+  \\ ASSUME_TAC x64_trailing_thm \\ SEP_I_TAC "x64_trailing" \\ POP_ASSUM MP_TAC
+  \\ MATCH_MP_TAC IMP_IMP \\ STRIP_TAC
+  THEN1 (FULL_SIMP_TAC (srw_ss()) [LENGTH_APPEND] \\ DECIDE_TAC)
+  \\ STRIP_TAC \\ FULL_SIMP_TAC std_ss []
+  \\ Cases_on `s = t` \\ FULL_SIMP_TAC std_ss []
+  \\ FULL_SIMP_TAC std_ss [x64_header_def,GSYM APPEND_ASSOC]
+  \\ FULL_SIMP_TAC (srw_ss()) [LENGTH_REPLICATE,WORD_MUL_LSL,word_mul_n2w]
+  \\ FULL_SIMP_TAC std_ss [AC MULT_COMM MULT_ASSOC]
+  \\ Q.ABBREV_TAC `ts = mw_mul xs ys (MAP (\x. 0x0w) ys)`
+  \\ `LENGTH (mw_trailing ts) <= LENGTH ts` by FULL_SIMP_TAC std_ss [LENGTH_mw_trailing]
+  \\ DECIDE_TAC);
+
+
+(* simple div xs into zs and zs into zs *)
+
+val (x64_single_div_res,x64_single_div_def) = x64_decompile "x64_single_div" `
+  div r9`
+
+val _ = add_compiled [x64_single_div_res]
+
+val MULT_LEMMA_LEMMA = prove(
+  ``!m n. l < k /\ l + k * m < k + k * n ==> m <= n:num``,
+  Induct \\ Cases_on `n` \\ FULL_SIMP_TAC std_ss [MULT_CLAUSES]
+  THEN1 (REPEAT STRIP_TAC \\ CCONTR_TAC \\ FULL_SIMP_TAC std_ss [] \\ DECIDE_TAC)
+  \\ REPEAT STRIP_TAC \\ Q.PAT_ASSUM `!x.bbb` MATCH_MP_TAC
+  \\ FULL_SIMP_TAC std_ss [] \\ DECIDE_TAC);
+
+val MULT_LEMMA = prove(
+  ``l < k ==> (l + k * m < k + k * n = m <= n:num)``,
+  REPEAT STRIP_TAC \\ REV EQ_TAC \\ REPEAT STRIP_TAC THEN1
+   (SUFF_TAC ``k * m <= k * n:num`` \\ REPEAT STRIP_TAC THEN1 DECIDE_TAC
+    \\ MATCH_MP_TAC LESS_MONO_MULT2 \\ FULL_SIMP_TAC std_ss [])
+  \\ CCONTR_TAC \\ FULL_SIMP_TAC std_ss [GSYM NOT_LESS]
+  \\ IMP_RES_TAC MULT_LEMMA_LEMMA \\ DECIDE_TAC);
+
+val x64_single_div_thm = prove(
+  ``(x64_single_div_pre (x2,x1,y) = x1 <+ y) /\
+    (x64_single_div (x2,x1,y) = let (q,r) = single_div x1 x2 y in (q,r,y))``,
+  FULL_SIMP_TAC (srw_ss()) [x64_single_div_def,single_div_def,LET_DEF]
+  \\ Cases_on `y` \\ Cases_on `n` \\ FULL_SIMP_TAC (srw_ss()) [WORD_LO,DIV_LT_X]
+  \\ FULL_SIMP_TAC std_ss [MULT_CLAUSES]
+  \\ SIMP_TAC std_ss [Once ADD_COMM] \\ SIMP_TAC std_ss [Once MULT_COMM]
+  \\ `w2n x2 < 18446744073709551616` by ALL_TAC THEN1
+   (ASSUME_TAC (w2n_lt |> INST_TYPE [``:'a``|->``:64``] |> Q.SPEC `x2`)
+    \\ FULL_SIMP_TAC (srw_ss()) [])
+  \\ FULL_SIMP_TAC std_ss [MULT_LEMMA]
+  \\ DECIDE_TAC);
+
+val (res,x64_simple_div_def,x64_simple_div_pre_def) = x64_compile `
+  x64_simple_div (r2:word64,r9:word64,r10:word64,xs:word64 list,zs:word64 list) =
+    if r10 = 0w then (r2,r9,r10,xs,zs) else
+      let r10 = r10 - 1w in
+      let r0 = EL (w2n r10) xs in
+      let (r0,r2,r9) = x64_single_div (r0,r2,r9) in
+      let zs = LUPDATE r0 (w2n r10) zs in
+        x64_simple_div (r2,r9,r10,xs,zs)`
+
+val x64_simple_div_thm = prove(
+  ``!xs xs1 zs zs1 r2 r9 qs r.
+      LENGTH xs < dimword(:64) /\ (LENGTH zs = LENGTH xs) /\
+      (mw_simple_div r2 (REVERSE xs) r9 = (qs,r,T)) ==>
+      x64_simple_div_pre (r2,r9,n2w (LENGTH xs),xs++xs1,zs++zs1) /\
+      (x64_simple_div (r2,r9,n2w (LENGTH xs),xs++xs1,zs++zs1) =
+         (r,r9,0w,xs++xs1,REVERSE qs++zs1))``,
+  HO_MATCH_MP_TAC SNOC_INDUCT \\ STRIP_TAC THEN1
+   (REPEAT STRIP_TAC \\ POP_ASSUM MP_TAC
+    \\ FULL_SIMP_TAC std_ss [LENGTH,Once x64_simple_div_pre_def,
+         Once x64_simple_div_def,REVERSE,mw_simple_div_def]
+    \\ Q.SPEC_TAC (`qs`,`qs`)
+    \\ Cases_on `zs` \\ FULL_SIMP_TAC (srw_ss()) [LENGTH,ADD1])
+  \\ NTAC 11 STRIP_TAC
+  \\ FULL_SIMP_TAC std_ss [REVERSE_SNOC,mw_simple_div_def,LET_DEF]
+  \\ `(zs = []) \/ ?z zs2. zs = SNOC z zs2` by METIS_TAC [SNOC_CASES]
+  THEN1 (FULL_SIMP_TAC (srw_ss()) [LENGTH])
+  \\ FULL_SIMP_TAC std_ss [LENGTH_SNOC]
+  \\ SIMP_TAC std_ss [LENGTH,Once x64_simple_div_pre_def,
+         Once x64_simple_div_def,REVERSE,mw_simple_div_def]
+  \\ FULL_SIMP_TAC (srw_ss()) [n2w_11,LET_DEF]
+  \\ FULL_SIMP_TAC std_ss [ADD1,GSYM word_add_n2w,GSYM word_sub_def,WORD_ADD_SUB]
+  \\ IMP_RES_TAC (DECIDE ``n+1<k ==> n<k``)
+  \\ FULL_SIMP_TAC (srw_ss()) []
+  \\ FULL_SIMP_TAC std_ss [SNOC_APPEND,GSYM APPEND_ASSOC,APPEND,LUPDATE_LENGTH]
+  \\ FULL_SIMP_TAC std_ss [rich_listTheory.EL_LENGTH_APPEND,NULL,HD]
+  \\ Q.PAT_ASSUM `LENGTH zs2 = LENGTH xs` (ASSUME_TAC o GSYM)
+  \\ FULL_SIMP_TAC std_ss [LUPDATE_LENGTH,x64_single_div_thm]
+  \\ `?q1 r1. single_div r2 x r9 = (q1,r1)` by METIS_TAC [PAIR]
+  \\ `?qs2 r2 c2. mw_simple_div r1 (REVERSE xs) r9 = (qs2,r2,c2)` by METIS_TAC [PAIR]
+  \\ FULL_SIMP_TAC std_ss [LET_DEF]
+  \\ Q.PAT_ASSUM `q1::qs2 = qs` (ASSUME_TAC o GSYM)
+  \\ FULL_SIMP_TAC std_ss [REVERSE,SNOC_APPEND,GSYM APPEND_ASSOC,APPEND]
+  \\ DECIDE_TAC);
+
+
+val _ = export_theory();
+
